Rename x64_ to mc_ and any_ to mc_

examples/machine-code/multiword/mc_multiwordScript.sml
@@ -4,7 +4,7 @@ open wordsTheory wordsLib addressTheory arithmeticTheory listTheory pairSyntax;
 open addressTheory pairTheory set_sepTheory rich_listTheory integerTheory;
 local open tailrecLib blastLib intLib in end
 
-val _ = new_theory "any_multiword";
+val _ = new_theory "mc_multiword";
 
 val REV = Tactical.REVERSE;
 
@@ -77,9 +77,9 @@ val one_neq_zero_word = SIMP_CONV(srw_ss())[]``1w = 0w``
 
 (* compare *)
 
-val (x64_cmp_def, _,
-     x64_cmp_pre_def, _) =
-  tailrec_define "x64_cmp" ``
+val (mc_cmp_def, _,
+     mc_cmp_pre_def, _) =
+  tailrec_define "mc_cmp" ``
     (\(l,r10,xs,ys).
       if r10 = 0x0w then (INR (l,r10,xs,ys),T)
       else
@@ -96,34 +96,34 @@ val (x64_cmp_def, _,
     :num # α word # α word list # α word list -> (num # α word # α word list # α
      word list + num # α word # α word list # α word list) # bool``;
 
-val (x64_compare_def, _,
-     x64_compare_pre_def, _) =
-  tailrec_define "x64_compare" ``
+val (mc_compare_def, _,
+     mc_compare_pre_def, _) =
+  tailrec_define "mc_compare" ``
     (\(l,r10,r11,xs,ys).
       if r10 <+ r11 then (let r10 = 0x1w in (INR (l,r10,xs,ys),T))
       else if r11 <+ r10 then (let r10 = 0x2w in (INR (l,r10,xs,ys),T))
       else
-        (let cond = x64_cmp_pre (l-1,r10,xs,ys) /\ l <> 0 in
-         let (l,r10,xs,ys) = x64_cmp (l-1,r10,xs,ys)
+        (let cond = mc_cmp_pre (l-1,r10,xs,ys) /\ l <> 0 in
+         let (l,r10,xs,ys) = mc_cmp (l-1,r10,xs,ys)
          in
            (INR (l,r10,xs,ys),cond)))
     :num # α word # α word # α word list # α word list -> (num # α
      word # α word # α word list # α word list + num # α word # α word
      list # α word list) # bool``;
 
-val x64_header_def = Define `
-  x64_header (s,xs:α word list) = n2w (LENGTH xs * 2) + if s then 1w else 0w:α word`;
+val mc_header_def = Define `
+  mc_header (s,xs:α word list) = n2w (LENGTH xs * 2) + if s then 1w else 0w:α word`;
 
-val (x64_icompare_def, _,
-     x64_icompare_pre_def, _) =
-  tailrec_define "x64_icompare" ``
+val (mc_icompare_def, _,
+     mc_icompare_pre_def, _) =
+  tailrec_define "mc_icompare" ``
     (\(l,r10,r11,xs,ys).
       if r10 && 0x1w = 0x0w then
         if r11 && 0x1w = 0x0w then
           (let r10 = r10 >>> 1 in
            let r11 = r11 >>> 1 in
-           let cond = x64_compare_pre (l,r10,r11,xs,ys) in
-           let (l,r10,xs,ys) = x64_compare (l,r10,r11,xs,ys)
+           let cond = mc_compare_pre (l,r10,r11,xs,ys) in
+           let (l,r10,xs,ys) = mc_compare (l,r10,r11,xs,ys)
            in
              (INR (l,r10,xs,ys),cond))
         else (let r10 = 0x2w in (INR (l,r10,xs,ys),T))
@@ -132,8 +132,8 @@ val (x64_icompare_def, _,
       else
         (let r10 = r10 >>> 1 in
          let r11 = r11 >>> 1 in
-         let cond = x64_compare_pre (l,r10,r11,xs,ys) in
-         let (l,r10,xs,ys) = x64_compare (l,r10,r11,xs,ys)
+         let cond = mc_compare_pre (l,r10,r11,xs,ys) in
+         let (l,r10,xs,ys) = mc_compare (l,r10,r11,xs,ys)
          in
            if r10 = 0x0w then (INR (l,r10,xs,ys),cond)
            else (let r10 = r10 ?? 0x3w in (INR (l,r10,xs,ys),cond))))
@@ -146,24 +146,24 @@ val cmp2w_def = Define `
   (cmp2w (SOME T) = 1w) /\
   (cmp2w (SOME F) = 2w)`;
 
-val x64_cmp_thm = prove(
+val mc_cmp_thm = prove(
   ``!xs ys xs1 ys1 l.
       (LENGTH ys = LENGTH xs) /\ LENGTH (xs:α word list) < dimword(:α) /\
       LENGTH xs <= l ==>
-      x64_cmp_pre (l,n2w (LENGTH xs),xs++xs1,ys++ys1) /\
+      mc_cmp_pre (l,n2w (LENGTH xs),xs++xs1,ys++ys1) /\
       ?l2.
-        (x64_cmp (l,n2w (LENGTH xs),xs++xs1,ys++ys1) =
+        (mc_cmp (l,n2w (LENGTH xs),xs++xs1,ys++ys1) =
           (l2,cmp2w (mw_cmp xs ys),xs++xs1,ys++ys1)) /\
         l <= l2 + LENGTH xs``,
   HO_MATCH_MP_TAC SNOC_INDUCT \\ FULL_SIMP_TAC std_ss [LENGTH,LENGTH_NIL]
   \\ STRIP_TAC THEN1
-   (REPEAT STRIP_TAC \\ ONCE_REWRITE_TAC [x64_cmp_def,Once x64_cmp_pre_def]
+   (REPEAT STRIP_TAC \\ ONCE_REWRITE_TAC [mc_cmp_def,Once mc_cmp_pre_def]
     \\ FULL_SIMP_TAC std_ss [Once mw_cmp_def,cmp2w_def,APPEND])
   \\ NTAC 8 STRIP_TAC
   \\ `(ys = []) \/ ?y ys2. ys = SNOC y ys2` by METIS_TAC [SNOC_CASES]
   \\ FULL_SIMP_TAC (srw_ss()) [] \\ FULL_SIMP_TAC std_ss [GSYM SNOC_APPEND,ADD1]
   \\ `LENGTH xs < dimword (:α)` by (FULL_SIMP_TAC (srw_ss()) [] \\ DECIDE_TAC)
-  \\ RES_TAC \\ ONCE_REWRITE_TAC [x64_cmp_def,x64_cmp_pre_def]
+  \\ RES_TAC \\ ONCE_REWRITE_TAC [mc_cmp_def,mc_cmp_pre_def]
   \\ SIMP_TAC std_ss [GSYM word_add_n2w,WORD_ADD_SUB]
   \\ FULL_SIMP_TAC (srw_ss()) [n2w_11,word_add_n2w,LET_DEF]
   \\ FULL_SIMP_TAC std_ss [SNOC_APPEND,GSYM APPEND_ASSOC,APPEND]
@@ -187,25 +187,25 @@ val x64_cmp_thm = prove(
   |> Q.SPECL [`xs`,`ys`,`[]`,`[]`]
   |> SIMP_RULE std_ss [APPEND_NIL];
 
-val x64_compare_thm = prove(
+val mc_compare_thm = prove(
   ``LENGTH (xs:α word list) < dimword (:α) /\ LENGTH ys < dimword (:α) /\
     LENGTH xs + 1 <= l ==>
-    ?l2. x64_compare_pre (l,n2w (LENGTH xs),n2w (LENGTH ys),xs,ys) /\
-         (x64_compare (l,n2w (LENGTH xs),n2w (LENGTH ys),xs,ys) =
+    ?l2. mc_compare_pre (l,n2w (LENGTH xs),n2w (LENGTH ys),xs,ys) /\
+         (mc_compare (l,n2w (LENGTH xs),n2w (LENGTH ys),xs,ys) =
            (l2,cmp2w (mw_compare xs ys),xs,ys)) /\
          l <= l2 + LENGTH xs + 1``,
-  SIMP_TAC (srw_ss()) [x64_compare_def,x64_compare_pre_def,
+  SIMP_TAC (srw_ss()) [mc_compare_def,mc_compare_pre_def,
     n2w_11,WORD_LO,LET_DEF,mw_compare_def]
   \\ SRW_TAC [] [cmp2w_def]
   \\ fs []
   \\ `LENGTH xs = LENGTH ys` by DECIDE_TAC
-  \\ MP_TAC x64_cmp_thm \\ FULL_SIMP_TAC (srw_ss()) []
+  \\ MP_TAC mc_cmp_thm \\ FULL_SIMP_TAC (srw_ss()) []
   \\ disch_then (qspec_then `l-1` mp_tac) \\ fs []
   \\ strip_tac \\ fs []);
 
-val x64_header_AND_1 = prove(
-  ``x64_header (s,xs) && (0x1w:'a word) = b2w s``,
-  rw[x64_header_def,GSYM word_mul_n2w,b2w_def,b2n_def]
+val mc_header_AND_1 = prove(
+  ``mc_header (s,xs) && (0x1w:'a word) = b2w s``,
+  rw[mc_header_def,GSYM word_mul_n2w,b2w_def,b2n_def]
   \\ Q.SPEC_TAC (`n2w (LENGTH xs) :α word`,`w`)
   \\ rw[fcpTheory.CART_EQ]
   \\ rw[word_and_def,WORD_ADD_BIT0,fcpTheory.FCP_BETA]
@@ -220,12 +220,12 @@ val x64_header_AND_1 = prove(
   by ( simp[Abbr`m`,Abbr`n`,EVEN_EXP] )
   \\ simp[EVEN_MOD,Abbr`n`]);
 
-val x64_header_sign = prove(
-  ``(x64_header (s,xs) && 1w = (0w:'a word)) = ~s``,
-  Cases_on`s` \\ rw[x64_header_AND_1]
+val mc_header_sign = prove(
+  ``(mc_header (s,xs) && 1w = (0w:'a word)) = ~s``,
+  Cases_on`s` \\ rw[mc_header_AND_1]
   \\ EVAL_TAC \\ simp[]);
 
-val x64_length_lemma = prove(
+val mc_length_lemma = prove(
   ``(w * 2w + if s then 0x1w else 0x0w) >>> 1 = (w * 2w:'a word) >>> 1``,
   Cases_on `s` \\ FULL_SIMP_TAC std_ss [] \\ blastLib.BBLAST_TAC
   \\ Cases_on`w` \\ fs[WORD_MUL_LSL,word_mul_n2w,word_add_n2w]
@@ -238,10 +238,10 @@ val x64_length_lemma = prove(
   \\ once_rewrite_tac[MULT_COMM]
   \\ simp[DIV_MULT,MULT_DIV]);
 
-val x64_length = prove(
+val mc_length = prove(
   ``LENGTH (xs:'a word list) < dimword (:'a) DIV 2 ==>
-    (x64_header (s,xs) >>> 1 = n2w (LENGTH xs))``,
-  FULL_SIMP_TAC std_ss [x64_header_def,GSYM word_mul_n2w,x64_length_lemma]
+    (mc_header (s,xs) >>> 1 = n2w (LENGTH xs))``,
+  FULL_SIMP_TAC std_ss [mc_header_def,GSYM word_mul_n2w,mc_length_lemma]
   \\ SIMP_TAC std_ss [GSYM w2n_11,w2n_lsr,w2n_n2w,word_mul_n2w]
   \\ FULL_SIMP_TAC (srw_ss()) [] \\ REPEAT STRIP_TAC
   \\ fs[X_LT_DIV]
@@ -252,18 +252,18 @@ val dim63_IMP_dim64 = prove(
   ``n < dimword (:'a) DIV 2 ==> n < dimword (:'a)``,
   fs[X_LT_DIV]);
 
-val x64_icompare_thm = prove(
+val mc_icompare_thm = prove(
   ``LENGTH (xs:'a word list) < dimword (:'a) DIV 2 /\
     LENGTH ys < dimword (:'a) DIV 2 /\
     LENGTH xs + 1 <= l ==>
-    ?l2. x64_icompare_pre (l,x64_header (s,xs),x64_header (t,ys),xs,ys) /\
-        (x64_icompare (l,x64_header (s,xs),x64_header (t,ys),xs,ys) =
+    ?l2. mc_icompare_pre (l,mc_header (s,xs),mc_header (t,ys),xs,ys) /\
+        (mc_icompare (l,mc_header (s,xs),mc_header (t,ys),xs,ys) =
           (l2,cmp2w (mwi_compare (s,xs) (t,ys)),xs,ys)) /\
         l <= l2 + LENGTH xs + 1``,
   strip_tac \\
-  FULL_SIMP_TAC std_ss [x64_icompare_def,x64_icompare_pre_def,x64_header_sign,
-    x64_length,LET_DEF] \\ IMP_RES_TAC dim63_IMP_dim64
-  \\ mp_tac x64_compare_thm \\ fs [] \\ strip_tac \\ fs []
+  FULL_SIMP_TAC std_ss [mc_icompare_def,mc_icompare_pre_def,mc_header_sign,
+    mc_length,LET_DEF] \\ IMP_RES_TAC dim63_IMP_dim64
+  \\ mp_tac mc_compare_thm \\ fs [] \\ strip_tac \\ fs []
   \\ FULL_SIMP_TAC std_ss [mwi_compare_def]
   \\ Cases_on `s` \\ Cases_on `t` \\ FULL_SIMP_TAC std_ss [cmp2w_def] \\ fs []
   \\ Cases_on `mw_compare xs ys` \\ FULL_SIMP_TAC std_ss [cmp2w_def,option_eq_def]
@@ -297,9 +297,9 @@ val single_add_word_thm =
   |> SIMP_RULE std_ss [LET_DEF]
   |> CONV_RULE (DEPTH_CONV PairRules.PBETA_CONV);
 
-val (x64_add_loop2_def, _,
-     x64_add_loop2_pre_def, _) =
-  tailrec_define "x64_add_loop2" ``
+val (mc_add_loop2_def, _,
+     mc_add_loop2_pre_def, _) =
+  tailrec_define "mc_add_loop2" ``
     (\(l,r1:'a word,r3:'a word,r8:'a word,r9:'a word,r10:'a word,xs,zs).
       if r1 = 0x1w then
         (let r1 = 0x0w
@@ -317,9 +317,9 @@ val (x64_add_loop2_def, _,
          in
            (INL (l,r1,r3,r8,r9,r10,xs,zs),cond /\ l <> 0n)))``;
 
-val (x64_add_loop1_def, _,
-     x64_add_loop1_pre_def, _) =
-  tailrec_define "x64_add_loop1" ``
+val (mc_add_loop1_def, _,
+     mc_add_loop1_pre_def, _) =
+  tailrec_define "mc_add_loop1" ``
     (\(l,r1:'a word,r3:'a word,r8:'a word,r9:'a word,r10:'a word,xs,ys,zs).
       if r1 = 0x1w then
         (let r1 = 0x0w:'a word
@@ -339,19 +339,19 @@ val (x64_add_loop1_def, _,
          in
            (INL (l,r1,r3,r8,r9,r10,xs,ys,zs),cond /\ l <> 0n)))``;
 
-val (x64_add_loop_def, _,
-     x64_add_loop_pre_def, _) =
-  tailrec_define "x64_add_loop" ``
+val (mc_add_loop_def, _,
+     mc_add_loop_pre_def, _) =
+  tailrec_define "mc_add_loop" ``
     (\(l,r1,r2,r8,r9,r10,xs,ys,zs).
       (let r1 = r1 + 0x1w in
        let r2 = r2 + 0x1w in
        let r3 = 0w in
-       let cond = x64_add_loop1_pre (l-1,r1,r3,r8,r9,r10,xs,ys,zs) /\ l <> 0 in
-       let (l,r1,r3,r8,r9,r10,xs,ys,zs) = x64_add_loop1 (l-1,r1,r3,r8,r9,r10,xs,ys,zs) in
+       let cond = mc_add_loop1_pre (l-1,r1,r3,r8,r9,r10,xs,ys,zs) /\ l <> 0 in
+       let (l,r1,r3,r8,r9,r10,xs,ys,zs) = mc_add_loop1 (l-1,r1,r3,r8,r9,r10,xs,ys,zs) in
        let r1 = r2 in
        let r9 = 0x0w in
-       let cond = cond /\ x64_add_loop2_pre (l-1,r1,r3,r8,r9,r10,xs,zs) /\ l <> 0 in
-       let (l,r1,r3,r8,r9,r10,xs,zs) = x64_add_loop2 (l-1,r1,r3,r8,r9,r10,xs,zs)
+       let cond = cond /\ mc_add_loop2_pre (l-1,r1,r3,r8,r9,r10,xs,zs) /\ l <> 0 in
+       let (l,r1,r3,r8,r9,r10,xs,zs) = mc_add_loop2 (l-1,r1,r3,r8,r9,r10,xs,zs)
        in
          if r3 = 0w then
            (INR (l,r1,r2,r8,r9,r10,xs,ys,zs),cond)
@@ -368,19 +368,19 @@ val (x64_add_loop_def, _,
      word list + num # 'a word # 'a word # 'a word # 'a word # 'a word
      # 'a word list # 'a word list # 'a word list) # bool``;
 
-val x64_add_loop_def =
-  LIST_CONJ [x64_add_loop_def,x64_add_loop_pre_def,
-             x64_add_loop1_def,x64_add_loop1_pre_def,
-             x64_add_loop2_def,x64_add_loop2_pre_def]
+val mc_add_loop_def =
+  LIST_CONJ [mc_add_loop_def,mc_add_loop_pre_def,
+             mc_add_loop1_def,mc_add_loop1_pre_def,
+             mc_add_loop2_def,mc_add_loop2_pre_def]
 
-val (x64_add_def, _,
-     x64_add_pre_def, _) =
-  tailrec_define "x64_add" ``
+val (mc_add_def, _,
+     mc_add_pre_def, _) =
+  tailrec_define "mc_add" ``
     (\(l,r1,r2,r8,r9,r10,xs,ys,zs).
       (let r2 = r2 - r1 in
-       let cond = x64_add_loop_pre (l,r1,r2,r8,r9,r10,xs,ys,zs) in
+       let cond = mc_add_loop_pre (l,r1,r2,r8,r9,r10,xs,ys,zs) in
        let (l,r1,r2,r8,r9,r10,xs,ys,zs) =
-             x64_add_loop (l,r1,r2,r8,r9,r10,xs,ys,zs)
+             mc_add_loop (l,r1,r2,r8,r9,r10,xs,ys,zs)
        in
          (INR (l,r1,r2,r8,r9,r10,xs,ys,zs),cond)))
     :num # 'a word # 'a word # 'a word # 'a word # 'a word # 'a word
@@ -406,16 +406,16 @@ val b2w_eq = store_thm("b2w_eq[simp]",
   ``((b2w b = 0w) <=> ~b) /\ ((b2w b = 1w) <=> b)``,
   Cases_on `b` \\ EVAL_TAC \\ fs[]);
 
-val x64_add_loop1_thm = prove(
+val mc_add_loop1_thm = prove(
   ``!(xs:'a word list) ys zs xs1 ys1 zs1 xs2 ys2 zs2 r8 r9 c l.
       (LENGTH ys1 = LENGTH xs1) /\ (LENGTH zs1 = LENGTH xs1) /\
       (LENGTH ys = LENGTH xs) /\ (LENGTH zs = LENGTH xs) /\
       LENGTH (xs1 ++ xs) + 1 < dimword(:'a) /\
       LENGTH xs <= l ==>
       ?r8' r9' l2.
-        x64_add_loop1_pre (l,n2w (LENGTH xs + 1),b2w c,r8,r9,n2w (LENGTH xs1),
+        mc_add_loop1_pre (l,n2w (LENGTH xs + 1),b2w c,r8,r9,n2w (LENGTH xs1),
           xs1 ++ xs ++ xs2, ys1 ++ ys ++ ys2,zs1 ++ zs ++ zs2) /\
-        (x64_add_loop1 (l,n2w (LENGTH xs + 1),b2w c,r8,r9,n2w (LENGTH xs1),
+        (mc_add_loop1 (l,n2w (LENGTH xs + 1),b2w c,r8,r9,n2w (LENGTH xs1),
           xs1 ++ xs ++ xs2, ys1 ++ ys ++ ys2,zs1 ++ zs ++ zs2) =
           (l2,0w,b2w (SND (mw_add xs ys c)),r8',r9',n2w (LENGTH (xs1++xs)),
            xs1 ++ xs ++ xs2,ys1 ++ ys ++ ys2,
@@ -423,10 +423,10 @@ val x64_add_loop1_thm = prove(
         l <= l2 + LENGTH xs``,
   Induct THEN1
    (FULL_SIMP_TAC (srw_ss()) [LENGTH,LENGTH_NIL,mw_add_def]
-    \\ ONCE_REWRITE_TAC [x64_add_loop_def]
+    \\ ONCE_REWRITE_TAC [mc_add_loop_def]
     \\ FULL_SIMP_TAC (srw_ss()) [LENGTH,LENGTH_NIL,mw_add_def,LET_DEF])
   \\ Cases_on `ys` \\ FULL_SIMP_TAC std_ss [LENGTH,ADD1]
-  \\ ONCE_REWRITE_TAC [x64_add_loop_def]
+  \\ ONCE_REWRITE_TAC [mc_add_loop_def]
   \\ FULL_SIMP_TAC (srw_ss()) [LET_DEF,single_add_word_thm]
   \\ REPEAT STRIP_TAC
   \\ `LENGTH xs < dimword(:'a) /\
@@ -448,7 +448,7 @@ val x64_add_loop1_thm = prove(
   \\ `LENGTH xs1 + 1 = LENGTH (SNOC h' xs1)` by
     FULL_SIMP_TAC std_ss [LENGTH_SNOC,ADD1] \\ ASM_SIMP_TAC std_ss []
   \\ ASM_SIMP_TAC std_ss [LUPDATE_SNOC]
-  \\ SEP_I_TAC "x64_add_loop1" \\ POP_ASSUM MP_TAC
+  \\ SEP_I_TAC "mc_add_loop1" \\ POP_ASSUM MP_TAC
   \\ MATCH_MP_TAC IMP_IMP \\ STRIP_TAC
   THEN1 (FULL_SIMP_TAC (srw_ss()) [] \\ DECIDE_TAC)
   \\ STRIP_TAC \\ ASM_SIMP_TAC std_ss []
@@ -457,15 +457,15 @@ val x64_add_loop1_thm = prove(
   \\ CONV_TAC (DEPTH_CONV PairRules.PBETA_CONV)
   \\ FULL_SIMP_TAC (srw_ss()) [b2w_def] \\ DECIDE_TAC);
 
-val x64_add_loop2_thm = prove(
+val mc_add_loop2_thm = prove(
   ``!(xs:'a word list) zs xs1 zs1 xs2 zs2 r8 c l.
       (LENGTH zs1 = LENGTH xs1) /\ (LENGTH zs = LENGTH xs) /\
       LENGTH (xs1 ++ xs) + 1 < dimword(:'a) /\
       LENGTH xs <= l ==>
       ?r8' r9' l2.
-        x64_add_loop2_pre (l,n2w (LENGTH xs + 1),b2w c,r8,0w,n2w (LENGTH xs1),
+        mc_add_loop2_pre (l,n2w (LENGTH xs + 1),b2w c,r8,0w,n2w (LENGTH xs1),
           xs1 ++ xs ++ xs2,zs1 ++ zs ++ zs2) /\
-        (x64_add_loop2 (l,n2w (LENGTH xs + 1),b2w c,r8,0w,n2w (LENGTH xs1),
+        (mc_add_loop2 (l,n2w (LENGTH xs + 1),b2w c,r8,0w,n2w (LENGTH xs1),
           xs1 ++ xs ++ xs2,zs1 ++ zs ++ zs2) =
           (l2,0w,b2w ((SND (mw_add xs (MAP (\x.0w) xs) c))),
            r8',r9',n2w (LENGTH (xs1++xs)),xs1 ++ xs ++ xs2,
@@ -473,10 +473,10 @@ val x64_add_loop2_thm = prove(
         l <= l2 + LENGTH xs``,
   Induct THEN1
    (FULL_SIMP_TAC (srw_ss()) [LENGTH,LENGTH_NIL,mw_add_def]
-    \\ ONCE_REWRITE_TAC [x64_add_loop_def]
+    \\ ONCE_REWRITE_TAC [mc_add_loop_def]
     \\ FULL_SIMP_TAC (srw_ss()) [LENGTH,LENGTH_NIL,mw_add_def,LET_DEF])
   \\ FULL_SIMP_TAC std_ss [LENGTH,ADD1]
-  \\ ONCE_REWRITE_TAC [x64_add_loop_def]
+  \\ ONCE_REWRITE_TAC [mc_add_loop_def]
   \\ FULL_SIMP_TAC (srw_ss()) [LET_DEF,single_add_word_thm]
   \\ REPEAT STRIP_TAC
   \\ `LENGTH xs < dimword(:'a) /\
@@ -495,7 +495,7 @@ val x64_add_loop2_thm = prove(
   \\ `LENGTH xs1 + 1 = LENGTH (SNOC h xs1)` by
     FULL_SIMP_TAC std_ss [LENGTH_SNOC,ADD1] \\ ASM_SIMP_TAC std_ss []
   \\ ASM_SIMP_TAC std_ss [LUPDATE_SNOC]
-  \\ SEP_I_TAC "x64_add_loop2" \\ POP_ASSUM MP_TAC
+  \\ SEP_I_TAC "mc_add_loop2" \\ POP_ASSUM MP_TAC
   \\ MATCH_MP_TAC IMP_IMP \\ STRIP_TAC
   THEN1 (FULL_SIMP_TAC (srw_ss()) [] \\ DECIDE_TAC)
   \\ STRIP_TAC \\ ASM_SIMP_TAC std_ss []
@@ -505,26 +505,26 @@ val x64_add_loop2_thm = prove(
   \\ FULL_SIMP_TAC (srw_ss()) [b2w_def]
   \\ DECIDE_TAC)
 
-val x64_add_thm = prove(
+val mc_add_thm = prove(
   ``!(xs:'a word list) ys zs zs2 l.
       LENGTH ys <= LENGTH xs /\ (LENGTH zs = LENGTH (mw_addv xs ys F)) /\
       LENGTH xs + 1 < dimword(:'a) /\ LENGTH xs + 2 <= l ==>
       ?r1' r2' r8' r9' r10' l2.
-        x64_add_pre (l,n2w (LENGTH ys),n2w (LENGTH xs),0w,0w,0w,xs,ys,zs++zs2) /\
-        (x64_add (l,n2w (LENGTH ys),n2w (LENGTH xs),0w,0w,0w,xs,ys,zs++zs2) =
+        mc_add_pre (l,n2w (LENGTH ys),n2w (LENGTH xs),0w,0w,0w,xs,ys,zs++zs2) /\
+        (mc_add (l,n2w (LENGTH ys),n2w (LENGTH xs),0w,0w,0w,xs,ys,zs++zs2) =
           (l2,r1',r2',r8',r9',n2w (LENGTH (mw_addv xs ys F)),xs,ys,
             mw_addv xs ys F ++ zs2)) /\
         l <= l2 + LENGTH xs + 2``,
   REPEAT STRIP_TAC \\ IMP_RES_TAC LESS_EQ_LENGTH
-  \\ FULL_SIMP_TAC std_ss [LENGTH_APPEND,x64_add_def,x64_add_pre_def,LET_DEF]
+  \\ FULL_SIMP_TAC std_ss [LENGTH_APPEND,mc_add_def,mc_add_pre_def,LET_DEF]
   \\ ONCE_REWRITE_TAC [ADD_COMM]
   \\ SIMP_TAC std_ss [GSYM word_add_n2w,WORD_ADD_SUB]
-  \\ ONCE_REWRITE_TAC [x64_add_loop_def]
+  \\ ONCE_REWRITE_TAC [mc_add_loop_def]
   \\ SIMP_TAC (srw_ss()) [LET_DEF,w2n_n2w,word_add_n2w]
   \\ `~((dimword(:'a) <= (LENGTH ys + 1) MOD dimword(:'a)))` by ALL_TAC
   THEN1 (fs[])
   \\ FULL_SIMP_TAC std_ss []
-  \\ (x64_add_loop1_thm |> Q.SPECL [`xs1`,`ys`,`zs`,`[]`,`[]`,`[]`,
+  \\ (mc_add_loop1_thm |> Q.SPECL [`xs1`,`ys`,`zs`,`[]`,`[]`,`[]`,
          `xs2`,`[]`,`zs2`,`r8`,`r9`,`F`] |> SIMP_RULE std_ss [EVAL ``b2w F``]
       |> GEN_ALL |> MP_TAC)
   \\ FULL_SIMP_TAC std_ss [LENGTH,APPEND,APPEND_NIL] \\ STRIP_TAC
@@ -550,13 +550,13 @@ val x64_add_thm = prove(
     \\ FULL_SIMP_TAC std_ss [APPEND_ASSOC,LENGTH_APPEND]
     \\ DECIDE_TAC)
   \\ FULL_SIMP_TAC std_ss [GSYM APPEND_ASSOC]
-  \\ SEP_I_TAC "x64_add_loop1" \\ POP_ASSUM MP_TAC
+  \\ SEP_I_TAC "mc_add_loop1" \\ POP_ASSUM MP_TAC
   \\ MATCH_MP_TAC IMP_IMP \\ STRIP_TAC
   THEN1 (FULL_SIMP_TAC (srw_ss()) [] \\ DECIDE_TAC)
   \\ STRIP_TAC \\ ASM_SIMP_TAC std_ss []
-  \\ (x64_add_loop2_thm |> Q.SPECL [`xs`,`ys`,`xs1`,`zs1`,`[]`] |> GEN_ALL
+  \\ (mc_add_loop2_thm |> Q.SPECL [`xs`,`ys`,`xs1`,`zs1`,`[]`] |> GEN_ALL
        |> SIMP_RULE std_ss [GSYM APPEND_ASSOC,APPEND_NIL] |> ASSUME_TAC)
-  \\ SEP_I_TAC "x64_add_loop2" \\ POP_ASSUM MP_TAC
+  \\ SEP_I_TAC "mc_add_loop2" \\ POP_ASSUM MP_TAC
   \\ MATCH_MP_TAC IMP_IMP \\ STRIP_TAC
   THEN1 (IMP_RES_TAC LENGTH_mw_add \\ FULL_SIMP_TAC (srw_ss()) [] \\ DECIDE_TAC)
   \\ STRIP_TAC \\ ASM_SIMP_TAC std_ss [b2w_eq]
@@ -587,9 +587,9 @@ val single_sub_word_thm =
   |> SIMP_RULE std_ss [LET_DEF]
   |> CONV_RULE (DEPTH_CONV PairRules.PBETA_CONV);
 
-val (x64_sub_loop2_def, _,
-     x64_sub_loop2_pre_def, _) =
-  tailrec_define "x64_sub_loop2" ``
+val (mc_sub_loop2_def, _,
+     mc_sub_loop2_pre_def, _) =
+  tailrec_define "mc_sub_loop2" ``
     (\(l,r1:'a word,r3:'a word,r8:'a word,r9:'a word,r10:'a word,xs,zs).
       if r1 = 0x1w then
         (let r1 = 0x0w:'a word
@@ -607,9 +607,9 @@ val (x64_sub_loop2_def, _,
          in
            (INL (l-1,r1,r3,r8,r9,r10,xs,zs),cond /\ l <> 0n)))``;
 
-val (x64_sub_loop1_def, _,
-     x64_sub_loop1_pre_def, _) =
-  tailrec_define "x64_sub_loop1" ``
+val (mc_sub_loop1_def, _,
+     mc_sub_loop1_pre_def, _) =
+  tailrec_define "mc_sub_loop1" ``
     (\(l,r1:'a word,r3:'a word,r8:'a word,r9:'a word,r10:'a word,xs,ys,zs).
       if r1 = 0x1w then
         (let r1 = 0x0w:'a word
@@ -629,20 +629,20 @@ val (x64_sub_loop1_def, _,
          in
            (INL (l-1,r1,r3,r8,r9,r10,xs,ys,zs),cond /\ l <> 0n)))``;
 
-val (x64_sub_loop_def, _,
-     x64_sub_loop_pre_def, _) =
-  tailrec_define "x64_sub_loop" ``
+val (mc_sub_loop_def, _,
+     mc_sub_loop_pre_def, _) =
+  tailrec_define "mc_sub_loop" ``
     (\(l,r1,r2,r8,r9,r10,xs,ys,zs).
       (let r1 = r1 + 0x1w in
        let r2 = r2 + 0x1w in
        let r3 = 1w in
        let r8 = r8 - 0x0w in
-       let cond = x64_sub_loop1_pre (l-1,r1,r3,r8,r9,r10,xs,ys,zs) /\ l <> 0n in
-       let (l,r1,r3,r8,r9,r10,xs,ys,zs) = x64_sub_loop1 (l-1,r1,r3,r8,r9,r10,xs,ys,zs) in
+       let cond = mc_sub_loop1_pre (l-1,r1,r3,r8,r9,r10,xs,ys,zs) /\ l <> 0n in
+       let (l,r1,r3,r8,r9,r10,xs,ys,zs) = mc_sub_loop1 (l-1,r1,r3,r8,r9,r10,xs,ys,zs) in
        let r1 = r2 in
        let r9 = 0x0w in
-       let cond = cond /\ x64_sub_loop2_pre (l-1,r1,r3,r8,r9,r10,xs,zs) /\ l <> 0n in
-       let (l,r1,r3,r8,r9,r10,xs,zs) = x64_sub_loop2 (l-1,r1,r3,r8,r9,r10,xs,zs)
+       let cond = cond /\ mc_sub_loop2_pre (l-1,r1,r3,r8,r9,r10,xs,zs) /\ l <> 0n in
+       let (l,r1,r3,r8,r9,r10,xs,zs) = mc_sub_loop2 (l-1,r1,r3,r8,r9,r10,xs,zs)
        in
          (INR (l,r1,r2,r8,r9,r10,xs,ys,zs),cond)))
   :num # 'a word # 'a word # 'a word # 'a word # 'a word # 'a word
@@ -651,14 +651,14 @@ val (x64_sub_loop_def, _,
    list + num # 'a word # 'a word # 'a word # 'a word # 'a word # 'a
    word list # 'a word list # 'a word list) # bool``
 
-val x64_sub_loop_def =
-  LIST_CONJ [x64_sub_loop_def,x64_sub_loop_pre_def,
-             x64_sub_loop1_def,x64_sub_loop1_pre_def,
-             x64_sub_loop2_def,x64_sub_loop2_pre_def]
+val mc_sub_loop_def =
+  LIST_CONJ [mc_sub_loop_def,mc_sub_loop_pre_def,
+             mc_sub_loop1_def,mc_sub_loop1_pre_def,
+             mc_sub_loop2_def,mc_sub_loop2_pre_def]
 
-val (x64_fix_def, _,
-     x64_fix_pre_def, _) =
-  tailrec_define "x64_fix" ``
+val (mc_fix_def, _,
+     mc_fix_pre_def, _) =
+  tailrec_define "mc_fix" ``
     (\(l:num,r8:'a word,r10:'a word,zs:'a word list).
       if r10 = 0x0w then (INR (l,r8,r10,zs),T)
       else
@@ -669,18 +669,18 @@ val (x64_fix_def, _,
            if r8 = 0x0w then (INL (l-1,r8,r10,zs),cond /\ l <> 0)
            else (let r10 = r10 + 0x1w in (INR (l,r8,r10,zs),cond))))``;
 
-val x64_fix_def =
-  LIST_CONJ [x64_fix_def,x64_fix_pre_def]
+val mc_fix_def =
+  LIST_CONJ [mc_fix_def,mc_fix_pre_def]
 
-val (x64_sub_def, _,
-     x64_sub_pre_def, _) =
-  tailrec_define "x64_sub" ``
+val (mc_sub_def, _,
+     mc_sub_pre_def, _) =
+  tailrec_define "mc_sub" ``
     (\(l,r1,r2,r8,r9,r10,xs,ys,zs).
       (let r2 = r2 - r1 in
-       let cond = x64_sub_loop_pre (l,r1,r2,r8,r9,r10,xs,ys,zs) in
-       let (l,r1,r2,r8,r9,r10,xs,ys,zs) = x64_sub_loop (l,r1,r2,r8,r9,r10,xs,ys,zs) in
-       let cond = cond /\ x64_fix_pre (l-1,r8,r10,zs) /\ l <> 0 in
-       let (l,r8,r10,zs) = x64_fix (l-1,r8,r10,zs)
+       let cond = mc_sub_loop_pre (l,r1,r2,r8,r9,r10,xs,ys,zs) in
+       let (l,r1,r2,r8,r9,r10,xs,ys,zs) = mc_sub_loop (l,r1,r2,r8,r9,r10,xs,ys,zs) in
+       let cond = cond /\ mc_fix_pre (l-1,r8,r10,zs) /\ l <> 0 in
+       let (l,r8,r10,zs) = mc_fix (l-1,r8,r10,zs)
        in
          (INR (l,r1,r2,r8,r9,r10,xs,ys,zs),cond)))
     :num # 'a word # 'a word # 'a word # 'a word # 'a word # 'a word
@@ -689,20 +689,20 @@ val (x64_sub_def, _,
      word list + num # 'a word # 'a word # 'a word # 'a word # 'a word
      # 'a word list # 'a word list # 'a word list) # bool``;
 
-val x64_sub_def =
-  LIST_CONJ [x64_sub_def,x64_sub_pre_def]
+val mc_sub_def =
+  LIST_CONJ [mc_sub_def,mc_sub_pre_def]
 
-val x64_fix_thm = prove(
+val mc_fix_thm = prove(
   ``!(zs:'a word list) zs1 r8 l.
       LENGTH zs < dimword(:'a) /\ LENGTH zs <= l ==>
       ?r8' l2.
-        x64_fix_pre (l,r8,n2w (LENGTH zs),zs++zs1) /\
-        (x64_fix (l,r8,n2w (LENGTH zs),zs++zs1) =
+        mc_fix_pre (l,r8,n2w (LENGTH zs),zs++zs1) /\
+        (mc_fix (l,r8,n2w (LENGTH zs),zs++zs1) =
          (l2,r8',n2w (LENGTH (mw_fix zs)),
           mw_fix zs ++ REPLICATE (LENGTH zs - LENGTH (mw_fix zs)) 0w ++ zs1)) /\
         l <= l2 + LENGTH zs``,
   HO_MATCH_MP_TAC SNOC_INDUCT \\ FULL_SIMP_TAC std_ss [LENGTH,LENGTH_NIL]
-  \\ REPEAT STRIP_TAC \\ ONCE_REWRITE_TAC [x64_fix_def,mw_fix_def]
+  \\ REPEAT STRIP_TAC \\ ONCE_REWRITE_TAC [mc_fix_def,mw_fix_def]
   \\ FULL_SIMP_TAC (srw_ss()) [rich_listTheory.REPLICATE,LET_DEF]
   \\ FULL_SIMP_TAC std_ss [GSYM word_add_n2w,ADD1,GSYM word_sub_def,WORD_ADD_SUB]
   \\ IMP_RES_TAC (DECIDE ``n + 1 < k ==> n < k:num``)
@@ -712,7 +712,7 @@ val x64_fix_thm = prove(
   \\ REV (Cases_on `x = 0w`) \\ FULL_SIMP_TAC std_ss [] THEN1
    (FULL_SIMP_TAC std_ss [LENGTH_APPEND,LENGTH,REPLICATE,APPEND,
       GSYM APPEND_ASSOC,word_add_n2w] \\ DECIDE_TAC)
-  \\ SEP_I_TAC "x64_fix" \\ FULL_SIMP_TAC std_ss [] \\ rfs []
+  \\ SEP_I_TAC "mc_fix" \\ FULL_SIMP_TAC std_ss [] \\ rfs []
   \\ `LENGTH (mw_fix zs) <= LENGTH zs` by
       FULL_SIMP_TAC std_ss [LENGTH_mw_fix]
   \\ `LENGTH zs + 1 - LENGTH (mw_fix zs) =
@@ -728,16 +728,16 @@ val sub_borrow_lemma = prove(
   \\ `(dimword(:'a) - 1 - n) < dimword(:'a)` by DECIDE_TAC
   \\ FULL_SIMP_TAC (srw_ss()) [b2n_def,word_1comp_n2w] \\ DECIDE_TAC);
 
-val x64_sub_loop1_thm = prove(
+val mc_sub_loop1_thm = prove(
   ``!(xs:'a word list) ys zs xs1 ys1 zs1 xs2 ys2 zs2 c r8 r9 l.
       (LENGTH ys1 = LENGTH xs1) /\ (LENGTH zs1 = LENGTH xs1) /\
       (LENGTH ys = LENGTH xs) /\ (LENGTH zs = LENGTH xs) /\
       LENGTH (xs1 ++ xs) + 1 < dimword(:'a) /\
       LENGTH xs <= l ==>
       ?r8' r9' l2.
-        x64_sub_loop1_pre (l,n2w (LENGTH xs + 1),b2w c,r8,r9,n2w (LENGTH xs1),
+        mc_sub_loop1_pre (l,n2w (LENGTH xs + 1),b2w c,r8,r9,n2w (LENGTH xs1),
           xs1 ++ xs ++ xs2, ys1 ++ ys ++ ys2,zs1 ++ zs ++ zs2) /\
-        (x64_sub_loop1 (l,n2w (LENGTH xs + 1),b2w c,r8,r9,n2w (LENGTH xs1),
+        (mc_sub_loop1 (l,n2w (LENGTH xs + 1),b2w c,r8,r9,n2w (LENGTH xs1),
           xs1 ++ xs ++ xs2, ys1 ++ ys ++ ys2,zs1 ++ zs ++ zs2) =
           (l2,0w,b2w (SND (mw_sub xs ys c)),r8',r9',n2w (LENGTH (xs1++xs)),
            xs1 ++ xs ++ xs2,ys1 ++ ys ++ ys2,
@@ -745,10 +745,10 @@ val x64_sub_loop1_thm = prove(
         l <= l2 + LENGTH xs``,
   Induct THEN1
    (FULL_SIMP_TAC (srw_ss()) [LENGTH,LENGTH_NIL,mw_sub_def]
-    \\ ONCE_REWRITE_TAC [x64_sub_loop_def]
+    \\ ONCE_REWRITE_TAC [mc_sub_loop_def]
     \\ FULL_SIMP_TAC (srw_ss()) [LENGTH,LENGTH_NIL,mw_sub_def,LET_DEF])
   \\ Cases_on `ys` \\ FULL_SIMP_TAC std_ss [LENGTH,ADD1]
-  \\ ONCE_REWRITE_TAC [x64_sub_loop_def]
+  \\ ONCE_REWRITE_TAC [mc_sub_loop_def]
   \\ FULL_SIMP_TAC (srw_ss()) [LET_DEF,single_sub_word_thm]
   \\ REPEAT STRIP_TAC
   \\ `LENGTH xs < dimword(:'a) /\
@@ -770,7 +770,7 @@ val x64_sub_loop1_thm = prove(
   \\ `LENGTH xs1 + 1 = LENGTH (SNOC h' xs1)` by
     FULL_SIMP_TAC std_ss [LENGTH_SNOC,ADD1] \\ ASM_SIMP_TAC std_ss []
   \\ ASM_SIMP_TAC std_ss [LUPDATE_SNOC]
-  \\ SEP_I_TAC "x64_sub_loop1" \\ POP_ASSUM MP_TAC
+  \\ SEP_I_TAC "mc_sub_loop1" \\ POP_ASSUM MP_TAC
   \\ MATCH_MP_TAC IMP_IMP \\ STRIP_TAC
   THEN1 (FULL_SIMP_TAC (srw_ss()) [] \\ DECIDE_TAC)
   \\ STRIP_TAC \\ ASM_SIMP_TAC std_ss []
@@ -780,24 +780,24 @@ val x64_sub_loop1_thm = prove(
   \\ FULL_SIMP_TAC (srw_ss()) [b2w_def]
   \\ DECIDE_TAC);
 
-val x64_sub_loop2_thm = prove(
+val mc_sub_loop2_thm = prove(
   ``!(xs:'a word list) zs xs1 zs1 xs2 zs2 c r8 l.
       (LENGTH zs1 = LENGTH xs1) /\ (LENGTH zs = LENGTH xs) /\
       LENGTH (xs1 ++ xs) + 1 < dimword(:'a) /\ LENGTH xs <= l ==>
       ?r8' r9' l2.
-        x64_sub_loop2_pre (l,n2w (LENGTH xs + 1),b2w c,r8,0w,n2w (LENGTH xs1),
+        mc_sub_loop2_pre (l,n2w (LENGTH xs + 1),b2w c,r8,0w,n2w (LENGTH xs1),
           xs1 ++ xs ++ xs2,zs1 ++ zs ++ zs2) /\
-        (x64_sub_loop2 (l,n2w (LENGTH xs + 1),b2w c,r8,0w,n2w (LENGTH xs1),
+        (mc_sub_loop2 (l,n2w (LENGTH xs + 1),b2w c,r8,0w,n2w (LENGTH xs1),
           xs1 ++ xs ++ xs2,zs1 ++ zs ++ zs2) =
           (l2,0w,b2w (SND (mw_sub xs [] c)),r8',r9',n2w (LENGTH (xs1++xs)),
            xs1 ++ xs ++ xs2,zs1 ++ FST (mw_sub xs [] c) ++ zs2)) /\
         l <= l2 + LENGTH xs``,
   Induct THEN1
    (FULL_SIMP_TAC (srw_ss()) [LENGTH,LENGTH_NIL,mw_sub_def]
-    \\ ONCE_REWRITE_TAC [x64_sub_loop_def]
+    \\ ONCE_REWRITE_TAC [mc_sub_loop_def]
     \\ FULL_SIMP_TAC (srw_ss()) [LENGTH,LENGTH_NIL,mw_sub_def,LET_DEF])
   \\ FULL_SIMP_TAC std_ss [LENGTH,ADD1]
-  \\ ONCE_REWRITE_TAC [x64_sub_loop_def]
+  \\ ONCE_REWRITE_TAC [mc_sub_loop_def]
   \\ FULL_SIMP_TAC (srw_ss()) [LET_DEF,single_sub_word_thm]
   \\ REPEAT STRIP_TAC
   \\ `LENGTH xs < dimword(:'a) /\
@@ -816,7 +816,7 @@ val x64_sub_loop2_thm = prove(
   \\ `LENGTH xs1 + 1 = LENGTH (SNOC h xs1)` by
     FULL_SIMP_TAC std_ss [LENGTH_SNOC,ADD1] \\ ASM_SIMP_TAC std_ss []
   \\ ASM_SIMP_TAC std_ss [LUPDATE_SNOC]
-  \\ SEP_I_TAC "x64_sub_loop2" \\ POP_ASSUM MP_TAC
+  \\ SEP_I_TAC "mc_sub_loop2" \\ POP_ASSUM MP_TAC
   \\ MATCH_MP_TAC IMP_IMP \\ STRIP_TAC
   THEN1 (FULL_SIMP_TAC (srw_ss()) [] \\ DECIDE_TAC)
   \\ STRIP_TAC \\ ASM_SIMP_TAC std_ss []
@@ -825,24 +825,24 @@ val x64_sub_loop2_thm = prove(
   \\ CONV_TAC (DEPTH_CONV PairRules.PBETA_CONV)
   \\ FULL_SIMP_TAC (srw_ss()) [b2w_def] \\ DECIDE_TAC);
 
-val x64_sub_thm = prove(
+val mc_sub_thm = prove(
   ``!(xs:'a word list) ys zs zs2 l.
       LENGTH ys <= LENGTH xs /\ (LENGTH zs = LENGTH xs) /\
       LENGTH xs + 1 < dimword(:'a) /\ LENGTH xs + LENGTH xs + 3 <= l ==>
       ?r1' r2' r8' r9' r10' l2.
-        x64_sub_pre (l,n2w (LENGTH ys),n2w (LENGTH xs),0w,0w,0w,xs,ys,zs++zs2) /\
-        (x64_sub (l,n2w (LENGTH ys),n2w (LENGTH xs),0w,0w,0w,xs,ys,zs++zs2) =
+        mc_sub_pre (l,n2w (LENGTH ys),n2w (LENGTH xs),0w,0w,0w,xs,ys,zs++zs2) /\
+        (mc_sub (l,n2w (LENGTH ys),n2w (LENGTH xs),0w,0w,0w,xs,ys,zs++zs2) =
           (l2,r1',r2',r8',r9',n2w (LENGTH (mw_subv xs ys)),xs,ys,
            mw_subv xs ys ++ REPLICATE (LENGTH xs - LENGTH (mw_subv xs ys)) 0w ++ zs2)) /\
         l <= l2 + LENGTH xs + LENGTH xs + 3``,
   REPEAT STRIP_TAC \\ IMP_RES_TAC LESS_EQ_LENGTH
-  \\ FULL_SIMP_TAC std_ss [LENGTH_APPEND,x64_sub_def,LET_DEF]
+  \\ FULL_SIMP_TAC std_ss [LENGTH_APPEND,mc_sub_def,LET_DEF]
   \\ ONCE_REWRITE_TAC [ADD_COMM]
   \\ SIMP_TAC std_ss [GSYM word_add_n2w,WORD_ADD_SUB]
-  \\ ONCE_REWRITE_TAC [x64_sub_loop_def]
+  \\ ONCE_REWRITE_TAC [mc_sub_loop_def]
   \\ SIMP_TAC std_ss [LET_DEF,w2n_n2w,word_add_n2w,WORD_LO]
   \\ FULL_SIMP_TAC (srw_ss()) []
-  \\ (x64_sub_loop1_thm |> Q.SPECL [`xs1`,`ys`,`zs`,`[]`,`[]`,`[]`,
+  \\ (mc_sub_loop1_thm |> Q.SPECL [`xs1`,`ys`,`zs`,`[]`,`[]`,`[]`,
            `xs2`,`[]`,`zs2`,`T`]
       |> SIMP_RULE std_ss [EVAL ``b2w T``]
       |> GEN_ALL |> MP_TAC)
@@ -863,13 +863,13 @@ val x64_sub_thm = prove(
       \\ `LENGTH (xs1' ++ xs2') = LENGTH (qs1 ++ qs2)` by ALL_TAC
       \\ FULL_SIMP_TAC std_ss [LENGTH_APPEND] \\ DECIDE_TAC)
   \\ FULL_SIMP_TAC std_ss [GSYM APPEND_ASSOC]
-  \\ SEP_I_TAC "x64_sub_loop1" \\ POP_ASSUM MP_TAC
+  \\ SEP_I_TAC "mc_sub_loop1" \\ POP_ASSUM MP_TAC
   \\ MATCH_MP_TAC IMP_IMP \\ STRIP_TAC
   THEN1 (FULL_SIMP_TAC (srw_ss()) [] \\ fs [] \\ DECIDE_TAC)
   \\ STRIP_TAC \\ ASM_SIMP_TAC std_ss []
-  \\ (x64_sub_loop2_thm |> Q.SPECL [`xs`,`ys`,`xs1`,`zs1`,`[]`] |> GEN_ALL
+  \\ (mc_sub_loop2_thm |> Q.SPECL [`xs`,`ys`,`xs1`,`zs1`,`[]`] |> GEN_ALL
        |> SIMP_RULE std_ss [GSYM APPEND_ASSOC,APPEND_NIL] |> ASSUME_TAC)
-  \\ SEP_I_TAC "x64_sub_loop2" \\ POP_ASSUM MP_TAC
+  \\ SEP_I_TAC "mc_sub_loop2" \\ POP_ASSUM MP_TAC
   \\ MATCH_MP_TAC IMP_IMP \\ STRIP_TAC
   THEN1 (IMP_RES_TAC LENGTH_mw_sub \\ fs [])
   \\ STRIP_TAC \\ ASM_SIMP_TAC std_ss []
@@ -879,15 +879,15 @@ val x64_sub_thm = prove(
   \\ `LENGTH (qs1 ++ qs2) < dimword (:'a) /\
       LENGTH (qs1 ++ qs2) <= l2' − 1` by (fs [] \\ NO_TAC)
   \\ FULL_SIMP_TAC std_ss []
-  \\ IMP_RES_TAC x64_fix_thm \\ SEP_I_TAC "x64_fix"
+  \\ IMP_RES_TAC mc_fix_thm \\ SEP_I_TAC "mc_fix"
   \\ FULL_SIMP_TAC std_ss []
   \\ FULL_SIMP_TAC std_ss [LENGTH_APPEND,AC ADD_COMM ADD_ASSOC] \\ fs []);
 
 (* integer addition *)
 
-val (x64_iadd1_def, _,
-     x64_iadd1_pre_def, _) =
-  tailrec_define "x64_iadd1" ``
+val (mc_iadd1_def, _,
+     mc_iadd1_pre_def, _) =
+  tailrec_define "mc_iadd1" ``
     (\(r1,r2,xs,ys).
       (let r0 = 0x0w
        in
@@ -906,9 +906,9 @@ val (x64_iadd1_def, _,
      word # 'a word list # 'a word list + 'a word # 'a word # 'a word
      # 'a word list # 'a word list) # bool``;
 
-val (x64_iadd2_def, _,
-     x64_iadd2_pre_def, _) =
-  tailrec_define "x64_iadd2" ``
+val (mc_iadd2_def, _,
+     mc_iadd2_pre_def, _) =
+  tailrec_define "mc_iadd2" ``
     (\(r1,r2,r10,r12,xs,ys).
       (let r0 = 0x0w
        in
@@ -929,9 +929,9 @@ val (x64_iadd2_def, _,
      'a word list + 'a word # 'a word # 'a word # 'a word # 'a word
      list # 'a word list) # bool``;
 
-val (x64_iadd3_def, _,
-     x64_iadd3_pre_def, _) =
-  tailrec_define "x64_iadd3" ``
+val (mc_iadd3_def, _,
+     mc_iadd3_pre_def, _) =
+  tailrec_define "mc_iadd3" ``
     (\(r0,xs,ys).
       if r0 = 0x0w then (INR (xs,ys),T)
       else (let (xs,ys) = (ys,xs) in (INR (xs,ys),T)))
@@ -939,9 +939,9 @@ val (x64_iadd3_def, _,
      ('a word # 'a word list # 'a word list +
       'a word list # 'a word list) # bool``;
 
-val (x64_iadd_def, _,
-     x64_iadd_pre_def, _) =
-  tailrec_define "x64_iadd" ``
+val (mc_iadd_def, _,
+     mc_iadd_pre_def, _) =
+  tailrec_define "mc_iadd" ``
     (\(l,r1,r2,xs,ys,zs).
       (let r10 = r1 in
        let r10 = r10 && 0x1w in
@@ -951,15 +951,15 @@ val (x64_iadd_def, _,
          if r10 = r11 then
            (let r1 = r1 >>> 1 in
             let r2 = r2 >>> 1 in
-            let (r1,r2,r0,xs,ys) = x64_iadd1 (r1,r2,xs,ys) in
+            let (r1,r2,r0,xs,ys) = mc_iadd1 (r1,r2,xs,ys) in
             let r8 = 0x0w in
             let r9 = r8 in
             let r10 = r8 in
-            let cond = x64_add_pre (l,r1,r2,r8,r9,r10,xs,ys,zs) in
+            let cond = mc_add_pre (l,r1,r2,r8,r9,r10,xs,ys,zs) in
             let (l,r1,r2,r8,r9,r10,xs,ys,zs) =
-                  x64_add (l,r1,r2,r8,r9,r10,xs,ys,zs)
+                  mc_add (l,r1,r2,r8,r9,r10,xs,ys,zs)
             in
-            let (xs,ys) = x64_iadd3 (r0,xs,ys) in
+            let (xs,ys) = mc_iadd3 (r0,xs,ys) in
             let r10 = r10 << 1 in
             let r10 = r10 + r11
             in
@@ -970,25 +970,25 @@ val (x64_iadd_def, _,
             let r10 = r10 >>> 1 in
             let r11 = r2 in
             let r11 = r11 >>> 1 in
-            let cond = x64_compare_pre (l,r10,r11,xs,ys) in
-            let (l,r10,xs,ys) = x64_compare (l,r10,r11,xs,ys)
+            let cond = mc_compare_pre (l,r10,r11,xs,ys) in
+            let (l,r10,xs,ys) = mc_compare (l,r10,r11,xs,ys)
             in
               if r10 = 0x0w then (INR (l,r10,xs,ys,zs),cond)
               else
                 (let (r1,r2,r0,r12,xs,ys) =
-                       x64_iadd2 (r1,r2,r10,r12,xs,ys)
+                       mc_iadd2 (r1,r2,r10,r12,xs,ys)
                  in
                  let r8 = 0x0w in
                  let r9 = r8 in
                  let r10 = r8 in
                  let r1 = r1 >>> 1 in
                  let r2 = r2 >>> 1 in
-                 let cond = cond /\ x64_sub_pre (l,r1,r2,r8,r9,r10,xs,ys,zs)
+                 let cond = cond /\ mc_sub_pre (l,r1,r2,r8,r9,r10,xs,ys,zs)
                  in
                  let (l,r1,r2,r8,r9,r10,xs,ys,zs) =
-                       x64_sub (l,r1,r2,r8,r9,r10,xs,ys,zs)
+                       mc_sub (l,r1,r2,r8,r9,r10,xs,ys,zs)
                  in
-                 let (xs,ys) = x64_iadd3 (r0,xs,ys) in
+                 let (xs,ys) = mc_iadd3 (r0,xs,ys) in
                  let r10 = r10 << 1 in
                  let r10 = r10 + r12
                  in
@@ -998,98 +998,98 @@ val (x64_iadd_def, _,
      'a word list + num # 'a word # 'a word list # 'a word list # 'a
      word list) # bool``;
 
-val x64_header_EQ = prove(
-  ``(x64_header (s,xs) && 0x1w = x64_header (t,ys) && 0x1w) = (s = t)``,
-  FULL_SIMP_TAC std_ss [x64_header_AND_1]
+val mc_header_EQ = prove(
+  ``(mc_header (s,xs) && 0x1w = mc_header (t,ys) && 0x1w) = (s = t)``,
+  FULL_SIMP_TAC std_ss [mc_header_AND_1]
   \\ Cases_on `s` \\ Cases_on `t` \\ EVAL_TAC \\ simp[]);
 
 val b2w_NOT = prove(
   ``!s. b2w s ?? 0x1w = b2w (~s):'a word``,
   Cases \\ rw[b2w_def,b2n_def]);
 
-val x64_iadd_thm = prove(
+val mc_iadd_thm = prove(
   ``LENGTH (xs:'a word list) < dimword (:'a) DIV 2 /\
     LENGTH ys < dimword (:'a) DIV 2 /\
     LENGTH xs + LENGTH ys <= LENGTH zs /\ mw_ok xs /\ mw_ok ys /\
     4 * LENGTH xs + 4 * LENGTH ys + 4 <= l ==>
     ?zs1 l2.
-      x64_iadd_pre (l,x64_header (s,xs),x64_header (t,ys),xs,ys,zs) /\
-      (x64_iadd (l,x64_header (s,xs),x64_header (t,ys),xs,ys,zs) =
-        (l2,x64_header (mwi_add (s,xs) (t,ys)),xs,ys,
+      mc_iadd_pre (l,mc_header (s,xs),mc_header (t,ys),xs,ys,zs) /\
+      (mc_iadd (l,mc_header (s,xs),mc_header (t,ys),xs,ys,zs) =
+        (l2,mc_header (mwi_add (s,xs) (t,ys)),xs,ys,
          SND (mwi_add (s,xs) (t,ys))++zs1)) /\
       (LENGTH (SND (mwi_add (s,xs) (t,ys))++zs1) = LENGTH zs) /\
       l <= l2 + 4 * LENGTH xs + 4 * LENGTH ys + 4``,
-  FULL_SIMP_TAC std_ss [x64_iadd_def,x64_iadd_pre_def,LET_DEF]
-  \\ FULL_SIMP_TAC std_ss [x64_header_EQ,mwi_add_def,x64_length]
+  FULL_SIMP_TAC std_ss [mc_iadd_def,mc_iadd_pre_def,LET_DEF]
+  \\ FULL_SIMP_TAC std_ss [mc_header_EQ,mwi_add_def,mc_length]
   \\ Cases_on `s <=> t` \\ FULL_SIMP_TAC std_ss []
   \\ REPEAT STRIP_TAC \\ IMP_RES_TAC dim63_IMP_dim64 THEN1
    (Cases_on `LENGTH ys <= LENGTH xs` \\ FULL_SIMP_TAC std_ss []
-    \\ FULL_SIMP_TAC (srw_ss()) [x64_iadd1_def,WORD_LO,GSYM NOT_LESS,LET_DEF]
+    \\ FULL_SIMP_TAC (srw_ss()) [mc_iadd1_def,WORD_LO,GSYM NOT_LESS,LET_DEF]
     THEN1
-     (ASSUME_TAC x64_add_thm
+     (ASSUME_TAC mc_add_thm
       \\ `LENGTH (mw_addv xs ys F) <= LENGTH xs + LENGTH ys` by
             FULL_SIMP_TAC std_ss [LENGTH_mw_addv,NOT_LESS]
       \\ `LENGTH (mw_addv xs ys F) <= LENGTH zs` by DECIDE_TAC
       \\ IMP_RES_TAC LESS_EQ_LENGTH
       \\ FULL_SIMP_TAC std_ss []
-      \\ SEP_I_TAC "x64_add" \\ POP_ASSUM MP_TAC
+      \\ SEP_I_TAC "mc_add" \\ POP_ASSUM MP_TAC
       \\ MATCH_MP_TAC IMP_IMP \\ STRIP_TAC
       THEN1 (FULL_SIMP_TAC std_ss [X_LT_DIV] \\ DECIDE_TAC)
       \\ REPEAT STRIP_TAC \\ FULL_SIMP_TAC std_ss [LENGTH_APPEND]
-      \\ FULL_SIMP_TAC (srw_ss()) [LENGTH_APPEND,x64_iadd3_def,x64_iadd3_pre_def,LET_DEF]
+      \\ FULL_SIMP_TAC (srw_ss()) [LENGTH_APPEND,mc_iadd3_def,mc_iadd3_pre_def,LET_DEF]
       \\ FULL_SIMP_TAC std_ss [WORD_MUL_LSL,word_mul_n2w]
       \\ ONCE_REWRITE_TAC [WORD_AND_COMM]
-      \\ FULL_SIMP_TAC std_ss [x64_header_AND_1]
-      \\ FULL_SIMP_TAC std_ss [x64_header_def,AC MULT_COMM MULT_ASSOC]
+      \\ FULL_SIMP_TAC std_ss [mc_header_AND_1]
+      \\ FULL_SIMP_TAC std_ss [mc_header_def,AC MULT_COMM MULT_ASSOC]
       \\ Cases_on `t` \\ FULL_SIMP_TAC (srw_ss()) [b2w_def,b2n_def,
            AC ADD_COMM ADD_ASSOC,word_add_n2w] \\ fs [])
     THEN1
-     (ASSUME_TAC x64_add_thm
+     (ASSUME_TAC mc_add_thm
       \\ `LENGTH (mw_addv ys xs F) <= LENGTH ys + LENGTH xs` by
          (`LENGTH xs <= LENGTH ys` by DECIDE_TAC
           \\ FULL_SIMP_TAC std_ss [LENGTH_mw_addv])
       \\ `LENGTH (mw_addv ys xs F) <= LENGTH zs` by DECIDE_TAC
       \\ IMP_RES_TAC LESS_EQ_LENGTH
       \\ FULL_SIMP_TAC std_ss []
-      \\ SEP_I_TAC "x64_add" \\ POP_ASSUM MP_TAC
+      \\ SEP_I_TAC "mc_add" \\ POP_ASSUM MP_TAC
       \\ MATCH_MP_TAC IMP_IMP \\ STRIP_TAC
       THEN1 (FULL_SIMP_TAC std_ss [X_LT_DIV] \\ DECIDE_TAC)
       \\ REPEAT STRIP_TAC \\ FULL_SIMP_TAC std_ss [LENGTH_APPEND]
-      \\ FULL_SIMP_TAC (srw_ss()) [LENGTH_APPEND,x64_iadd3_def,x64_iadd3_pre_def,LET_DEF]
+      \\ FULL_SIMP_TAC (srw_ss()) [LENGTH_APPEND,mc_iadd3_def,mc_iadd3_pre_def,LET_DEF]
       \\ FULL_SIMP_TAC std_ss [WORD_MUL_LSL,word_mul_n2w]
       \\ ONCE_REWRITE_TAC [WORD_AND_COMM]
-      \\ FULL_SIMP_TAC std_ss [x64_header_AND_1]
-      \\ FULL_SIMP_TAC std_ss [x64_header_def,AC MULT_COMM MULT_ASSOC]
+      \\ FULL_SIMP_TAC std_ss [mc_header_AND_1]
+      \\ FULL_SIMP_TAC std_ss [mc_header_def,AC MULT_COMM MULT_ASSOC]
       \\ Cases_on `t` \\ FULL_SIMP_TAC (srw_ss()) [b2w_def,b2n_def,
            AC ADD_COMM ADD_ASSOC,word_add_n2w] \\ fs []))
-  \\ mp_tac x64_compare_thm
+  \\ mp_tac mc_compare_thm
   \\ match_mp_tac IMP_IMP \\ conj_tac THEN1 fs []
   \\ strip_tac
   \\ FULL_SIMP_TAC std_ss [mw_compare_thm]
   \\ Cases_on `mw2n ys = mw2n xs` \\ FULL_SIMP_TAC std_ss [cmp2w_def]
-  THEN1 (FULL_SIMP_TAC (srw_ss()) [x64_header_def,APPEND,LENGTH] \\ fs [])
+  THEN1 (FULL_SIMP_TAC (srw_ss()) [mc_header_def,APPEND,LENGTH] \\ fs [])
   \\ Cases_on `mw2n xs < mw2n ys` \\ FULL_SIMP_TAC std_ss [GSYM NOT_LESS]
-  \\ FULL_SIMP_TAC (srw_ss()) [cmp2w_def,x64_iadd2_def,LET_DEF]
+  \\ FULL_SIMP_TAC (srw_ss()) [cmp2w_def,mc_iadd2_def,LET_DEF]
   THEN1
    (`LENGTH ys <= LENGTH zs` by DECIDE_TAC
     \\ IMP_RES_TAC LESS_EQ_LENGTH
     \\ FULL_SIMP_TAC std_ss []
-    \\ ASSUME_TAC x64_sub_thm
-    \\ FULL_SIMP_TAC (srw_ss()) [x64_length]
-    \\ SEP_I_TAC "x64_sub" \\ POP_ASSUM MP_TAC
+    \\ ASSUME_TAC mc_sub_thm
+    \\ FULL_SIMP_TAC (srw_ss()) [mc_length]
+    \\ SEP_I_TAC "mc_sub" \\ POP_ASSUM MP_TAC
     \\ MATCH_MP_TAC IMP_IMP \\ STRIP_TAC
     \\ `mw2n xs <= mw2n ys` by DECIDE_TAC
     \\ IMP_RES_TAC mw2n_LESS
     THEN1 (FULL_SIMP_TAC std_ss [X_LT_DIV] \\ DECIDE_TAC)
     \\ REPEAT STRIP_TAC
-    \\ FULL_SIMP_TAC std_ss [LENGTH_APPEND,x64_iadd3_def,
-         x64_iadd3_pre_def,LET_DEF,one_neq_zero_word]
+    \\ FULL_SIMP_TAC std_ss [LENGTH_APPEND,mc_iadd3_def,
+         mc_iadd3_pre_def,LET_DEF,one_neq_zero_word]
     \\ SIMP_TAC (srw_ss()) [GSYM APPEND_ASSOC,LENGTH_REPLICATE]
     \\ STRIP_TAC THEN1
      (FULL_SIMP_TAC std_ss [WORD_MUL_LSL,word_mul_n2w]
       \\ ONCE_REWRITE_TAC [WORD_AND_COMM]
-      \\ FULL_SIMP_TAC std_ss [x64_header_AND_1]
-      \\ FULL_SIMP_TAC std_ss [x64_header_def,AC MULT_COMM MULT_ASSOC]
+      \\ FULL_SIMP_TAC std_ss [mc_header_AND_1]
+      \\ FULL_SIMP_TAC std_ss [mc_header_def,AC MULT_COMM MULT_ASSOC]
       \\ FULL_SIMP_TAC std_ss [b2w_NOT]
       \\ Cases_on `s` \\ FULL_SIMP_TAC (srw_ss()) [b2w_def,b2n_def,
            AC ADD_COMM ADD_ASSOC,word_add_n2w])
@@ -1111,21 +1111,21 @@ val x64_iadd_thm = prove(
    (`LENGTH xs <= LENGTH zs` by DECIDE_TAC
     \\ IMP_RES_TAC LESS_EQ_LENGTH
     \\ FULL_SIMP_TAC std_ss []
-    \\ ASSUME_TAC x64_sub_thm
-    \\ FULL_SIMP_TAC (srw_ss()) [x64_length]
-    \\ SEP_I_TAC "x64_sub" \\ POP_ASSUM MP_TAC
+    \\ ASSUME_TAC mc_sub_thm
+    \\ FULL_SIMP_TAC (srw_ss()) [mc_length]
+    \\ SEP_I_TAC "mc_sub" \\ POP_ASSUM MP_TAC
     \\ MATCH_MP_TAC IMP_IMP \\ STRIP_TAC
     \\ `mw2n ys <= mw2n xs` by DECIDE_TAC
     \\ IMP_RES_TAC mw2n_LESS
     THEN1 (FULL_SIMP_TAC std_ss [X_LT_DIV] \\ DECIDE_TAC)
     \\ REPEAT STRIP_TAC
-    \\ FULL_SIMP_TAC std_ss [LENGTH_APPEND,x64_iadd3_def,x64_iadd3_pre_def,LET_DEF]
+    \\ FULL_SIMP_TAC std_ss [LENGTH_APPEND,mc_iadd3_def,mc_iadd3_pre_def,LET_DEF]
     \\ SIMP_TAC (srw_ss()) [GSYM APPEND_ASSOC,LENGTH_REPLICATE]
     \\ STRIP_TAC THEN1
      (FULL_SIMP_TAC std_ss [WORD_MUL_LSL,word_mul_n2w]
       \\ ONCE_REWRITE_TAC [WORD_AND_COMM]
-      \\ FULL_SIMP_TAC std_ss [x64_header_AND_1]
-      \\ FULL_SIMP_TAC std_ss [x64_header_def,AC MULT_COMM MULT_ASSOC]
+      \\ FULL_SIMP_TAC std_ss [mc_header_AND_1]
+      \\ FULL_SIMP_TAC std_ss [mc_header_def,AC MULT_COMM MULT_ASSOC]
       \\ FULL_SIMP_TAC std_ss [b2w_NOT]
       \\ Cases_on `s` \\ FULL_SIMP_TAC (srw_ss()) [b2w_def,b2n_def,
            AC ADD_COMM ADD_ASSOC,word_add_n2w])
@@ -1134,9 +1134,9 @@ val x64_iadd_thm = prove(
 
 (* multiplication *)
 
-val (x64_single_mul_add_def, _,
-     x64_single_mul_add_pre_def, _) =
-  tailrec_define "x64_single_mul_add" ``
+val (mc_single_mul_add_def, _,
+     mc_single_mul_add_pre_def, _) =
+  tailrec_define "mc_single_mul_add" ``
     (\(r0,r1,r2,r3).
       (let cond = T in
        let (r0,r2) = single_mul r0 r2 0w in
@@ -1148,14 +1148,14 @@ val (x64_single_mul_add_def, _,
     :'a word # 'a word # 'a word # 'a word -> ('a word # 'a word # 'a
      word # 'a word + 'a word # 'a word # 'a word # 'a word) # bool``;
 
-val x64_single_mul_add_def =
-  LIST_CONJ [x64_single_mul_add_def,x64_single_mul_add_pre_def]
+val mc_single_mul_add_def =
+  LIST_CONJ [mc_single_mul_add_def,mc_single_mul_add_pre_def]
 
-val x64_single_mul_add_thm = prove(
-  ``x64_single_mul_add_pre (p,k,q,s) /\
-    (x64_single_mul_add (p,k,q,s) =
+val mc_single_mul_add_thm = prove(
+  ``mc_single_mul_add_pre (p,k,q,s) /\
+    (mc_single_mul_add (p,k,q,s) =
       let (x1,x2) = single_mul_add p q k s in (x1,k,x2,s))``,
-  FULL_SIMP_TAC (srw_ss()) [x64_single_mul_add_def,LET_DEF]
+  FULL_SIMP_TAC (srw_ss()) [mc_single_mul_add_def,LET_DEF]
   \\ Cases_on `k` \\ Cases_on `s` \\ Cases_on `p` \\ Cases_on `q`
   \\ FULL_SIMP_TAC (srw_ss()) [single_mul_add_def,LET_DEF,single_mul_def,b2n_thm,
        mw_add_def,single_add_def,b2n_def(*,b2w_def*),word_add_n2w,word_mul_n2w,
@@ -1183,9 +1183,9 @@ val x64_single_mul_add_thm = prove(
   \\ `l MOD k < k` by FULL_SIMP_TAC std_ss []
   \\ ASM_SIMP_TAC std_ss [DIV_EQ_X] \\ DECIDE_TAC);
 
-val (x64_mul_pass_def, _,
-     x64_mul_pass_pre_def, _) =
-  tailrec_define "x64_mul_pass" ``
+val (mc_mul_pass_def, _,
+     mc_mul_pass_pre_def, _) =
+  tailrec_define "mc_mul_pass" ``
     (\(l,r1,r8,r9,r10,r11,ys,zs).
       if r9 = r11 then
         (let cond = w2n r10 < LENGTH zs in
@@ -1199,8 +1199,8 @@ val (x64_mul_pass_def, _,
          let cond = cond /\ w2n r11 < LENGTH ys in
          let r2 = EL (w2n r11) ys in
          let r0 = r8 in
-         let cond = cond /\ x64_single_mul_add_pre (r0,r1,r2,r3) in
-         let (r0,r1,r2,r3) = x64_single_mul_add (r0,r1,r2,r3) in
+         let cond = cond /\ mc_single_mul_add_pre (r0,r1,r2,r3) in
+         let (r0,r1,r2,r3) = mc_single_mul_add (r0,r1,r2,r3) in
          let zs = LUPDATE r0 (w2n r10) zs in
          let r1 = r2 in
          let r10 = r10 + 0x1w in
@@ -1212,9 +1212,9 @@ val (x64_mul_pass_def, _,
      word # 'a word # 'a word list # 'a word list + num # 'a word # 'a
      word # 'a word # 'a word list # 'a word list) # bool``;
 
-val (x64_mul_def, _,
-     x64_mul_pre_def, _) =
-  tailrec_define "x64_mul" ``
+val (mc_mul_def, _,
+     mc_mul_pre_def, _) =
+  tailrec_define "mc_mul" ``
     (\(l,r7,r9,r10,r12,xs,ys,zs).
       if r7 = 0x0w then (let r10 = r10 + r9 in (INR (l,r10,xs,ys,zs),T))
       else
@@ -1224,8 +1224,8 @@ val (x64_mul_def, _,
          let r12 = r12 + 0x1w in
          let r11 = 0x0w in
          let r1 = r11 in
-         let cond = cond /\ x64_mul_pass_pre (l-1,r1,r8,r9,r10,r11,ys,zs) /\ l <> 0 in
-         let (l,r1,r9,r10,ys,zs) = x64_mul_pass (l-1,r1,r8,r9,r10,r11,ys,zs) in
+         let cond = cond /\ mc_mul_pass_pre (l-1,r1,r8,r9,r10,r11,ys,zs) /\ l <> 0 in
+         let (l,r1,r9,r10,ys,zs) = mc_mul_pass (l-1,r1,r8,r9,r10,r11,ys,zs) in
          let r10 = r10 - r9
          in
            (INL (l-1,r7,r9,r10,r12,xs,ys,zs),cond /\ l <> 0)))
@@ -1234,9 +1234,9 @@ val (x64_mul_def, _,
      'a word # 'a word list # 'a word list # 'a word list + num # 'a
      word # 'a word list # 'a word list # 'a word list) # bool``;
 
-val (x64_mul_zero_def, _,
-     x64_mul_zero_pre_def, _) =
-  tailrec_define "x64_mul_zero" ``
+val (mc_mul_zero_def, _,
+     mc_mul_zero_pre_def, _) =
+  tailrec_define "mc_mul_zero" ``
     (\(l:num,r0:'a word,r10:'a word,zs:'a word list).
       if r10 = 0x0w then (INR (l,r10,zs),T)
       else
@@ -1246,18 +1246,18 @@ val (x64_mul_zero_def, _,
          in
            (INL (l-1,r0,r10,zs),cond /\ l <> 0)))``;
 
-val (x64_imul1_def, _,
-     x64_imul1_pre_def, _) =
-  tailrec_define "x64_imul1" ``
+val (mc_imul1_def, _,
+     mc_imul1_pre_def, _) =
+  tailrec_define "mc_imul1" ``
     (\(r10:'a word,r11:'a word).
       if r10 = r11
       then let r13 = (0w:'a word) in (INR (r10,r11,r13),T)
       else let r13 = (1w:'a word) in (INR (r10,r11,r13),T))
     :α word # α word -> (α word # α word + α word # α word # α word) # bool``;
 
-val (x64_imul_def, _,
-     x64_imul_pre_def, _) =
-  tailrec_define "x64_imul" ``
+val (mc_imul_def, _,
+     mc_imul_pre_def, _) =
+  tailrec_define "mc_imul" ``
     ( \ (l,r1,r2,xs,ys,zs).
       (let r10 = 0x0w
        in
@@ -1267,24 +1267,24 @@ val (x64_imul_def, _,
            (let r0 = 0x0w in
             let r10 = r2 in
             let r10 = r10 >>> 1 in
-            let cond = x64_mul_zero_pre (l-1,r0,r10,zs) /\ l <> 0 in
-            let (l,r10,zs) = x64_mul_zero (l-1,r0,r10,zs) in
+            let cond = mc_mul_zero_pre (l-1,r0,r10,zs) /\ l <> 0 in
+            let (l,r10,zs) = mc_mul_zero (l-1,r0,r10,zs) in
             let r10 = r1 in
             let r10 = r10 && 0x1w in
             let r11 = r2 in
             let r11 = r11 && 0x1w in
-            let (r10,r11,r13) = x64_imul1 (r10,r11) in
+            let (r10,r11,r13) = mc_imul1 (r10,r11) in
             let r7 = r1 in
             let r7 = r7 >>> 1 in
             let r9 = r2 in
             let r9 = r9 >>> 1 in
             let r10 = 0x0w in
             let r5 = r10 in
-            let cond = cond /\ x64_mul_pre (l-1,r7,r9,r10,r5,xs,ys,zs) /\ l <> 0 in
-            let (l,r10,xs,ys,zs) = x64_mul (l-1,r7,r9,r10,r5,xs,ys,zs) in
+            let cond = cond /\ mc_mul_pre (l-1,r7,r9,r10,r5,xs,ys,zs) /\ l <> 0 in
+            let (l,r10,xs,ys,zs) = mc_mul (l-1,r7,r9,r10,r5,xs,ys,zs) in
             let r8 = 0x0w in
-            let cond = cond /\ x64_fix_pre (l-1,r8,r10,zs) /\ l <> 0 in
-            let (l,r8,r10,zs) = x64_fix (l-1,r8,r10,zs) in
+            let cond = cond /\ mc_fix_pre (l-1,r8,r10,zs) /\ l <> 0 in
+            let (l,r8,r10,zs) = mc_fix (l-1,r8,r10,zs) in
             let r10 = r10 << 1 in
             let r10 = r10 + r13
             in
@@ -1294,27 +1294,27 @@ val (x64_imul_def, _,
      'a word list + num # 'a word # 'a word list # 'a word list # 'a
      word list) # bool``;
 
-val x64_mul_pass_thm = prove(
+val mc_mul_pass_thm = prove(
   ``!(ys:'a word list) ys1 x zs k zs1 zs2 z2 l.
       LENGTH (ys1++ys) < dimword (:'a) /\ (LENGTH zs = LENGTH ys) /\
       LENGTH (zs1++zs) < dimword (:'a) /\ LENGTH ys <= l ==>
       ?r1 l2.
-        x64_mul_pass_pre (l,k,x,n2w (LENGTH (ys1++ys)),n2w (LENGTH zs1),
+        mc_mul_pass_pre (l,k,x,n2w (LENGTH (ys1++ys)),n2w (LENGTH zs1),
                           n2w (LENGTH ys1),ys1++ys,zs1++zs++z2::zs2) /\
-        (x64_mul_pass (l,k,x,n2w (LENGTH (ys1++ys)),n2w (LENGTH zs1),
+        (mc_mul_pass (l,k,x,n2w (LENGTH (ys1++ys)),n2w (LENGTH zs1),
                        n2w (LENGTH ys1),ys1++ys,zs1++zs++z2::zs2) =
            (l2,r1,n2w (LENGTH (ys1++ys)),n2w (LENGTH (zs1++zs)+1),ys1++ys,
             zs1++(mw_mul_pass x ys zs k)++zs2)) /\
         l <= l2 + LENGTH ys``,
   Induct \\ Cases_on `zs`
   \\ FULL_SIMP_TAC std_ss [LENGTH,APPEND_NIL,mw_mul_pass_def,ADD1]
-  \\ ONCE_REWRITE_TAC [x64_mul_pass_def,x64_mul_pass_pre_def]
+  \\ ONCE_REWRITE_TAC [mc_mul_pass_def,mc_mul_pass_pre_def]
   \\ FULL_SIMP_TAC std_ss [LET_DEF,n2w_11,w2n_n2w,LUPDATE_LENGTH]
   \\ FULL_SIMP_TAC std_ss [GSYM APPEND_ASSOC,APPEND,word_add_n2w,LENGTH_APPEND]
   \\ FULL_SIMP_TAC std_ss [LENGTH]
   \\ REPEAT STRIP_TAC
   \\ IMP_RES_TAC (DECIDE ``m+n<k ==> m < k /\ n<k:num``)
-  \\ FULL_SIMP_TAC std_ss [ADD1,x64_single_mul_add_thm]
+  \\ FULL_SIMP_TAC std_ss [ADD1,mc_single_mul_add_thm]
   \\ FULL_SIMP_TAC std_ss [rich_listTheory.EL_LENGTH_APPEND,LUPDATE_LENGTH,NULL,HD]
   \\ Cases_on `single_mul_add x h' k h` \\ FULL_SIMP_TAC std_ss [LET_DEF,TL]
   \\ ONCE_REWRITE_TAC [SNOC_INTRO |> Q.INST [`xs2`|->`[]`] |> REWRITE_RULE [APPEND_NIL]]
@@ -1323,7 +1323,7 @@ val x64_mul_pass_thm = prove(
       ((LENGTH zs1 + 1) = LENGTH (SNOC q zs1))` by ALL_TAC
   THEN1 (FULL_SIMP_TAC std_ss [LENGTH_SNOC] \\ DECIDE_TAC)
   \\ FULL_SIMP_TAC std_ss []
-  \\ SEP_I_TAC "x64_mul_pass" \\ POP_ASSUM MP_TAC
+  \\ SEP_I_TAC "mc_mul_pass" \\ POP_ASSUM MP_TAC
   \\ MATCH_MP_TAC IMP_IMP \\ STRIP_TAC
   THEN1 (FULL_SIMP_TAC (srw_ss()) [] \\ DECIDE_TAC)
   \\ REPEAT STRIP_TAC \\ FULL_SIMP_TAC std_ss []
@@ -1335,21 +1335,21 @@ val WORD_SUB_LEMMA = prove(
   ``v + -1w * w = v - w``,
   FULL_SIMP_TAC (srw_ss()) []);
 
-val x64_mul_thm = prove(
+val mc_mul_thm = prove(
   ``!(xs:'a word list) ys zs xs1 zs1 zs2 l.
       LENGTH (xs1 ++ xs) < dimword (:'a) /\ LENGTH ys < dimword (:'a) /\
       (LENGTH zs = LENGTH ys) /\ LENGTH (zs1++zs++zs2) < dimword (:'a) /\
       LENGTH xs <= LENGTH zs2 /\ ys <> [] /\
       2 * LENGTH xs + LENGTH xs * LENGTH ys <= l ==>
       ?zs3 l2.
-        x64_mul_pre (l,n2w (LENGTH xs),n2w (LENGTH ys),n2w (LENGTH zs1),n2w (LENGTH xs1),
+        mc_mul_pre (l,n2w (LENGTH xs),n2w (LENGTH ys),n2w (LENGTH zs1),n2w (LENGTH xs1),
                  xs1 ++ xs,ys,zs1 ++ zs ++ zs2) /\
-       (x64_mul (l,n2w (LENGTH xs),n2w (LENGTH ys),n2w (LENGTH zs1),n2w (LENGTH xs1),
+       (mc_mul (l,n2w (LENGTH xs),n2w (LENGTH ys),n2w (LENGTH zs1),n2w (LENGTH xs1),
                  xs1 ++ xs,ys,zs1 ++ zs ++ zs2) =
           (l2,n2w (LENGTH (zs1 ++ mw_mul xs ys zs)),xs1++xs,ys,zs1 ++ mw_mul xs ys zs ++ zs3)) /\
        (LENGTH (zs1 ++ zs ++ zs2) = LENGTH (zs1 ++ mw_mul xs ys zs ++ zs3)) /\
        l <= l2 + 2 * LENGTH xs + LENGTH xs * LENGTH ys``,
-  Induct \\ ONCE_REWRITE_TAC [x64_mul_def,x64_mul_pre_def]
+  Induct \\ ONCE_REWRITE_TAC [mc_mul_def,mc_mul_pre_def]
   \\ FULL_SIMP_TAC std_ss [LENGTH,mw_mul_def,APPEND_NIL,LET_DEF]
   \\ FULL_SIMP_TAC std_ss [LENGTH_APPEND,word_add_n2w]
   THEN1 (METIS_TAC [])
@@ -1360,8 +1360,8 @@ val x64_mul_thm = prove(
   \\ FULL_SIMP_TAC std_ss [rich_listTheory.EL_LENGTH_APPEND,LUPDATE_LENGTH,NULL,HD]
   \\ FULL_SIMP_TAC std_ss [GSYM word_sub_def,ADD1,GSYM word_add_n2w,WORD_ADD_SUB]
   \\ Cases_on `zs2` \\ FULL_SIMP_TAC std_ss [LENGTH]
-  \\ ASSUME_TAC x64_mul_pass_thm
-  \\ SEP_I_TAC "x64_mul_pass" \\ POP_ASSUM MP_TAC
+  \\ ASSUME_TAC mc_mul_pass_thm
+  \\ SEP_I_TAC "mc_mul_pass" \\ POP_ASSUM MP_TAC
   \\ MATCH_MP_TAC IMP_IMP \\ STRIP_TAC
   THEN1 (FULL_SIMP_TAC (srw_ss()) [RIGHT_ADD_DISTRIB] \\ fs [])
   \\ STRIP_TAC \\ FULL_SIMP_TAC std_ss []
@@ -1381,7 +1381,7 @@ val x64_mul_thm = prove(
   \\ FULL_SIMP_TAC std_ss []
   \\ FULL_SIMP_TAC std_ss [GSYM APPEND_ASSOC,APPEND]
   \\ ONCE_REWRITE_TAC [SNOC_INTRO |> Q.INST [`xs2`|->`[]`] |> REWRITE_RULE [APPEND_NIL]]
-  \\ SEP_I_TAC "x64_mul" \\ POP_ASSUM MP_TAC
+  \\ SEP_I_TAC "mc_mul" \\ POP_ASSUM MP_TAC
   \\ MATCH_MP_TAC IMP_IMP \\ STRIP_TAC
   THEN1 (fs [LEFT_ADD_DISTRIB])
   \\ STRIP_TAC \\ FULL_SIMP_TAC std_ss []
@@ -1394,15 +1394,15 @@ val x64_mul_thm = prove(
   |> Q.SPECL [`xs`,`ys`,`zs`,`[]`,`[]`,`zs2`]
   |> SIMP_RULE std_ss [LENGTH,APPEND] |> GEN_ALL;
 
-val x64_mul_zero_thm = prove(
+val mc_mul_zero_thm = prove(
   ``!zs zs1 l.
       LENGTH zs < dimword(:'a) /\ LENGTH zs <= l ==>
-        x64_mul_zero_pre (l,0w:'a word,n2w (LENGTH zs),zs++zs1) /\
-        (x64_mul_zero (l,0w,n2w (LENGTH zs),zs++zs1) =
+        mc_mul_zero_pre (l,0w:'a word,n2w (LENGTH zs),zs++zs1) /\
+        (mc_mul_zero (l,0w,n2w (LENGTH zs),zs++zs1) =
           (l - LENGTH zs,0w,MAP (\x.0w) zs ++ zs1))``,
   HO_MATCH_MP_TAC SNOC_INDUCT \\ FULL_SIMP_TAC std_ss [LENGTH,LENGTH_NIL]
   \\ NTAC 4 STRIP_TAC
-  \\ ONCE_REWRITE_TAC [x64_mul_zero_def,x64_mul_zero_pre_def]
+  \\ ONCE_REWRITE_TAC [mc_mul_zero_def,mc_mul_zero_pre_def]
   \\ FULL_SIMP_TAC (srw_ss()) [rich_listTheory.REPLICATE,LET_DEF]
   \\ NTAC 3 STRIP_TAC
   \\ FULL_SIMP_TAC std_ss [GSYM word_add_n2w,ADD1,GSYM word_sub_def,WORD_ADD_SUB]
@@ -1416,26 +1416,26 @@ val MAP_EQ_MAP_EQ = prove(
   ``!xs ys. (MAP (\x.0w) xs = MAP (\x.0w) ys) = (LENGTH xs = LENGTH ys)``,
   Induct \\ Cases_on `ys` \\ FULL_SIMP_TAC (srw_ss()) []);
 
-val x64_imul1_thm = prove(
-  ``x64_imul1_pre (r10,r11) /\
-    (x64_imul1 (r10,r11) = (r10,r11,if r10 = r11 then 0w else 1w))``,
-  fs [x64_imul1_def,x64_imul1_pre_def] \\ rw []);
+val mc_imul1_thm = prove(
+  ``mc_imul1_pre (r10,r11) /\
+    (mc_imul1 (r10,r11) = (r10,r11,if r10 = r11 then 0w else 1w))``,
+  fs [mc_imul1_def,mc_imul1_pre_def] \\ rw []);
 
-val x64_imul_thm = prove(
-  ``((x64_header (s,xs) = (0w:'a word)) = (xs = [])) /\
-    ((x64_header (t,ys) = 0w) = (ys = [])) /\
+val mc_imul_thm = prove(
+  ``((mc_header (s,xs) = (0w:'a word)) = (xs = [])) /\
+    ((mc_header (t,ys) = 0w) = (ys = [])) /\
     LENGTH xs < dimword (:'a) DIV 2 /\ LENGTH ys < dimword (:'a) DIV 2 /\
     LENGTH xs + LENGTH ys <= LENGTH zs /\ LENGTH zs < dimword (:'a) DIV 2 /\
     3 * LENGTH xs + 3 * LENGTH ys + LENGTH xs * LENGTH ys + 3 <= l ==>
     ?zs1 l2.
-      x64_imul_pre (l,x64_header (s,xs),x64_header (t,ys),xs,ys,zs) /\
-      (x64_imul (l,x64_header (s,xs),x64_header (t,ys),xs,ys,zs) =
-        (l2,x64_header (mwi_mul (s,xs) (t,ys)),xs,ys,
+      mc_imul_pre (l,mc_header (s,xs),mc_header (t,ys),xs,ys,zs) /\
+      (mc_imul (l,mc_header (s,xs),mc_header (t,ys),xs,ys,zs) =
+        (l2,mc_header (mwi_mul (s,xs) (t,ys)),xs,ys,
          SND (mwi_mul (s,xs) (t,ys))++zs1)) /\
       (LENGTH (SND (mwi_mul (s,xs) (t,ys))++zs1) = LENGTH zs) /\
       l <= l2 + 3 * LENGTH xs + 3 * LENGTH ys + LENGTH xs * LENGTH ys + 3``,
-  FULL_SIMP_TAC std_ss [x64_imul_def,x64_imul_pre_def,LET_DEF,x64_imul1_thm]
-  \\ FULL_SIMP_TAC std_ss [x64_header_EQ,mwi_mul_def,x64_length]
+  FULL_SIMP_TAC std_ss [mc_imul_def,mc_imul_pre_def,LET_DEF,mc_imul1_thm]
+  \\ FULL_SIMP_TAC std_ss [mc_header_EQ,mwi_mul_def,mc_length]
   \\ Cases_on `xs = []` \\ FULL_SIMP_TAC std_ss [APPEND]
   THEN1 (REPEAT STRIP_TAC \\ EVAL_TAC \\ simp[])
   \\ Cases_on `ys = []` \\ FULL_SIMP_TAC std_ss [APPEND]
@@ -1446,25 +1446,25 @@ val x64_imul_thm = prove(
        METIS_TAC [LESS_EQ_LENGTH]
   \\ `LENGTH qs1 < dimword (:'a)` by (fs [X_LT_DIV] \\ DECIDE_TAC)
   \\ `LENGTH ys <= l-1` by fs []
-  \\ REV_FULL_SIMP_TAC std_ss [x64_mul_zero_thm]
-  \\ ASSUME_TAC x64_mul_thm
+  \\ REV_FULL_SIMP_TAC std_ss [mc_mul_zero_thm]
+  \\ ASSUME_TAC mc_mul_thm
   \\ Q.PAT_X_ASSUM `LENGTH ys = LENGTH qs1` (ASSUME_TAC o GSYM)
   \\ `MAP (\x. 0x0w:'a word) qs1 = MAP (\x. 0x0w) ys` by
        (ASM_SIMP_TAC std_ss [MAP_EQ_MAP_EQ] \\ NO_TAC)
   \\ FULL_SIMP_TAC std_ss []
-  \\ SEP_I_TAC "x64_mul" \\ POP_ASSUM MP_TAC
+  \\ SEP_I_TAC "mc_mul" \\ POP_ASSUM MP_TAC
   \\ MATCH_MP_TAC IMP_IMP \\ STRIP_TAC
   THEN1 (fs [LENGTH_APPEND,X_LT_DIV])
   \\ STRIP_TAC \\ FULL_SIMP_TAC std_ss []
   \\ `LENGTH qs1 < dimword (:'a)` by (FULL_SIMP_TAC (srw_ss()) [] \\ DECIDE_TAC)
   \\ `LENGTH (mw_mul xs ys (MAP (\x. 0x0w) ys)) < dimword (:'a)` by ALL_TAC
   THEN1 (FULL_SIMP_TAC (srw_ss()) [LENGTH_mw_mul,LENGTH_MAP,X_LT_DIV] \\ DECIDE_TAC)
-  \\ ASSUME_TAC x64_fix_thm \\ SEP_I_TAC "x64_fix" \\ POP_ASSUM MP_TAC
+  \\ ASSUME_TAC mc_fix_thm \\ SEP_I_TAC "mc_fix" \\ POP_ASSUM MP_TAC
   \\ MATCH_MP_TAC IMP_IMP \\ STRIP_TAC
   THEN1 (fs [LENGTH_mw_mul])
   \\ STRIP_TAC \\ FULL_SIMP_TAC std_ss []
   \\ Cases_on `s = t` \\ FULL_SIMP_TAC std_ss []
-  \\ FULL_SIMP_TAC std_ss [x64_header_def,GSYM APPEND_ASSOC]
+  \\ FULL_SIMP_TAC std_ss [mc_header_def,GSYM APPEND_ASSOC]
   \\ FULL_SIMP_TAC (srw_ss()) [LENGTH_REPLICATE,WORD_MUL_LSL,word_mul_n2w]
   \\ FULL_SIMP_TAC std_ss [AC MULT_COMM MULT_ASSOC]
   \\ Q.ABBREV_TAC `ts = mw_mul xs ys (MAP (\x. 0x0w) ys)`
@@ -1479,9 +1479,9 @@ val single_div_pre_def = Define `
     r9 <> (0x0w:'a word) /\
     (w2n r2 * dimword(:'a) + w2n r0) DIV w2n r9 < dimword(:'a)`;
 
-val (x64_single_div_def, _,
-     x64_single_div_pre_def, _) =
-  tailrec_define "x64_single_div" ``
+val (mc_single_div_def, _,
+     mc_single_div_pre_def, _) =
+  tailrec_define "mc_single_div" ``
     (\(r0,r2,r9).
       (let cond = single_div_pre r2 r0 r9 in
        let (r0,r2) = single_div r2 r0 r9
@@ -1490,7 +1490,7 @@ val (x64_single_div_def, _,
     :'a word # 'a word # 'a word -> ('a word # 'a word # 'a word + 'a
     word # 'a word # 'a word) # bool``;
 
-val x64_single_div_def = LIST_CONJ [x64_single_div_def,x64_single_div_pre_def]
+val mc_single_div_def = LIST_CONJ [mc_single_div_def,mc_single_div_pre_def]
 
 val MULT_LEMMA_LEMMA = prove(
   ``!m n. l < k /\ l + k * m < k + k * n ==> m <= n:num``,
@@ -1507,10 +1507,10 @@ val MULT_LEMMA = prove(
   \\ CCONTR_TAC \\ FULL_SIMP_TAC std_ss [GSYM NOT_LESS]
   \\ IMP_RES_TAC MULT_LEMMA_LEMMA \\ DECIDE_TAC);
 
-val x64_single_div_thm = prove(
-  ``(x64_single_div_pre (x2,x1,y) = x1 <+ y) /\
-    (x64_single_div (x2,x1,y) = let (q,r) = single_div x1 x2 y in (q,r,y))``,
-  FULL_SIMP_TAC (srw_ss()) [x64_single_div_def,single_div_def,LET_DEF,
+val mc_single_div_thm = prove(
+  ``(mc_single_div_pre (x2,x1,y) = x1 <+ y) /\
+    (mc_single_div (x2,x1,y) = let (q,r) = single_div x1 x2 y in (q,r,y))``,
+  FULL_SIMP_TAC (srw_ss()) [mc_single_div_def,single_div_def,LET_DEF,
        single_div_pre_def]
   \\ Cases_on `y` \\ Cases_on `n` \\ FULL_SIMP_TAC (srw_ss()) [WORD_LO,DIV_LT_X]
   \\ FULL_SIMP_TAC std_ss [MULT_CLAUSES]
@@ -1521,17 +1521,17 @@ val x64_single_div_thm = prove(
   \\ FULL_SIMP_TAC std_ss [MULT_LEMMA]
   \\ DECIDE_TAC);
 
-val (x64_simple_div_def, _,
-     x64_simple_div_pre_def, _) =
-  tailrec_define "x64_simple_div" ``
+val (mc_simple_div_def, _,
+     mc_simple_div_pre_def, _) =
+  tailrec_define "mc_simple_div" ``
     (\(l,r2,r9,r10,xs,zs).
       if r10 = 0x0w then (INR (l,r2,r9,r10,xs,zs),T)
       else
         (let r10 = r10 - 0x1w in
          let cond = w2n r10 < LENGTH xs in
          let r0 = EL (w2n r10) xs in
-         let cond = cond /\ x64_single_div_pre (r0,r2,r9) in
-         let (r0,r2,r9) = x64_single_div (r0,r2,r9) in
+         let cond = cond /\ mc_single_div_pre (r0,r2,r9) in
+         let (r0,r2,r9) = mc_single_div (r0,r2,r9) in
          let cond = cond /\ w2n r10 < LENGTH zs in
          let zs = LUPDATE r0 (w2n r10) zs
          in
@@ -1540,17 +1540,17 @@ val (x64_simple_div_def, _,
      (num # 'a word # 'a word # 'a word # 'a word list # 'a word list +
       num # 'a word # 'a word # 'a word # 'a word list # 'a word list) # bool``;
 
-val (x64_simple_div1_def, _,
-     x64_simple_div1_pre_def, _) =
-  tailrec_define "x64_simple_div1" ``
+val (mc_simple_div1_def, _,
+     mc_simple_div1_pre_def, _) =
+  tailrec_define "mc_simple_div1" ``
     (\(l,r2,r9,r10,zs).
       if r10 = 0x0w then (INR (l,r2,r9,r10,zs),T)
       else
         (let r10 = r10 - 0x1w in
          let cond = w2n r10 < LENGTH zs in
          let r0 = EL (w2n r10) zs in
-         let cond = cond /\ x64_single_div_pre (r0,r2,r9) in
-         let (r0,r2,r9) = x64_single_div (r0,r2,r9) in
+         let cond = cond /\ mc_single_div_pre (r0,r2,r9) in
+         let (r0,r2,r9) = mc_single_div (r0,r2,r9) in
          let zs = LUPDATE r0 (w2n r10) zs
          in
            (INL (l-1,r2,r9,r10,zs),cond /\ l <> 0)))
@@ -1558,18 +1558,18 @@ val (x64_simple_div1_def, _,
     word # 'a word # 'a word # 'a word list + num # 'a word # 'a word
     # 'a word # 'a word list) # bool``;
 
-val x64_simple_div_thm = prove(
+val mc_simple_div_thm = prove(
   ``!(xs:'a word list) xs1 zs zs1 r2 r9 qs r l.
       LENGTH xs < dimword(:'a) /\ (LENGTH zs = LENGTH xs) /\
       LENGTH xs <= l /\
       (mw_simple_div r2 (REVERSE xs) r9 = (qs,r,T)) ==>
-      x64_simple_div_pre (l,r2,r9,n2w (LENGTH xs),xs++xs1,zs++zs1) /\
-      (x64_simple_div (l,r2,r9,n2w (LENGTH xs),xs++xs1,zs++zs1) =
+      mc_simple_div_pre (l,r2,r9,n2w (LENGTH xs),xs++xs1,zs++zs1) /\
+      (mc_simple_div (l,r2,r9,n2w (LENGTH xs),xs++xs1,zs++zs1) =
          (l - LENGTH xs,r,r9,0w,xs++xs1,REVERSE qs++zs1))``,
   HO_MATCH_MP_TAC SNOC_INDUCT \\ STRIP_TAC THEN1
    (REPEAT STRIP_TAC \\ POP_ASSUM MP_TAC
-    \\ FULL_SIMP_TAC std_ss [LENGTH,Once x64_simple_div_pre_def,
-         Once x64_simple_div_def,REVERSE,mw_simple_div_def]
+    \\ FULL_SIMP_TAC std_ss [LENGTH,Once mc_simple_div_pre_def,
+         Once mc_simple_div_def,REVERSE,mw_simple_div_def]
     \\ Q.SPEC_TAC (`qs`,`qs`)
     \\ Cases_on `zs` \\ FULL_SIMP_TAC (srw_ss()) [LENGTH,ADD1])
   \\ NTAC 12 STRIP_TAC
@@ -1577,8 +1577,8 @@ val x64_simple_div_thm = prove(
   \\ `(zs = []) \/ ?z zs2. zs = SNOC z zs2` by METIS_TAC [SNOC_CASES]
   THEN1 (FULL_SIMP_TAC (srw_ss()) [LENGTH])
   \\ FULL_SIMP_TAC std_ss [LENGTH_SNOC]
-  \\ SIMP_TAC std_ss [LENGTH,Once x64_simple_div_pre_def,
-         Once x64_simple_div_def,REVERSE,mw_simple_div_def]
+  \\ SIMP_TAC std_ss [LENGTH,Once mc_simple_div_pre_def,
+         Once mc_simple_div_def,REVERSE,mw_simple_div_def]
   \\ FULL_SIMP_TAC (srw_ss()) [n2w_11,LET_DEF]
   \\ FULL_SIMP_TAC std_ss [ADD1,GSYM word_add_n2w,GSYM word_sub_def,WORD_ADD_SUB]
   \\ IMP_RES_TAC (DECIDE ``n+1<k ==> n<k:num``)
@@ -1587,7 +1587,7 @@ val x64_simple_div_thm = prove(
   \\ FULL_SIMP_TAC std_ss [rich_listTheory.EL_LENGTH_APPEND,NULL,HD]
   \\ Q.PAT_X_ASSUM `LENGTH zs2 = LENGTH xs` (ASSUME_TAC o GSYM)
   \\ `LENGTH zs2 ≤ l - 1` by fs []
-  \\ FULL_SIMP_TAC std_ss [LUPDATE_LENGTH,x64_single_div_thm]
+  \\ FULL_SIMP_TAC std_ss [LUPDATE_LENGTH,mc_single_div_thm]
   \\ `?q1 r1. single_div r2 x r9 = (q1,r1)` by METIS_TAC [PAIR]
   \\ `?qs2 r2 c2. mw_simple_div r1 (REVERSE xs) r9 = (qs2,r2,c2)` by METIS_TAC [PAIR]
   \\ FULL_SIMP_TAC std_ss [LET_DEF] \\ rfs []
@@ -1596,30 +1596,30 @@ val x64_simple_div_thm = prove(
   \\ Q.PAT_X_ASSUM `q1::qs2 = qs` (ASSUME_TAC o GSYM)
   \\ FULL_SIMP_TAC std_ss [REVERSE,SNOC_APPEND,GSYM APPEND_ASSOC,APPEND]);
 
-val x64_simple_div1_thm = prove(
+val mc_simple_div1_thm = prove(
   ``!(zs:'a word list) zs1 r2 r9 qs r l.
       LENGTH zs < dimword(:'a) /\ LENGTH zs <= l /\
       (mw_simple_div r2 (REVERSE zs) r9 = (qs,r,T)) ==>
-      x64_simple_div1_pre (l,r2,r9,n2w (LENGTH zs),zs++zs1) /\
-      (x64_simple_div1 (l,r2,r9,n2w (LENGTH zs),zs++zs1) =
+      mc_simple_div1_pre (l,r2,r9,n2w (LENGTH zs),zs++zs1) /\
+      (mc_simple_div1 (l,r2,r9,n2w (LENGTH zs),zs++zs1) =
          (l - LENGTH zs,r,r9,0w,REVERSE qs++zs1))``,
   HO_MATCH_MP_TAC SNOC_INDUCT \\ STRIP_TAC THEN1
    (REPEAT STRIP_TAC \\ POP_ASSUM MP_TAC
-    \\ FULL_SIMP_TAC std_ss [LENGTH,Once x64_simple_div1_pre_def,
-         Once x64_simple_div1_def,REVERSE,mw_simple_div_def]
+    \\ FULL_SIMP_TAC std_ss [LENGTH,Once mc_simple_div1_pre_def,
+         Once mc_simple_div1_def,REVERSE,mw_simple_div_def]
     \\ Q.SPEC_TAC (`qs`,`qs`) \\ FULL_SIMP_TAC (srw_ss()) [LENGTH,ADD1])
   \\ NTAC 10 STRIP_TAC
   \\ FULL_SIMP_TAC std_ss [REVERSE_SNOC,mw_simple_div_def,LET_DEF]
   \\ FULL_SIMP_TAC std_ss [LENGTH_SNOC]
-  \\ SIMP_TAC std_ss [LENGTH,Once x64_simple_div1_pre_def,
-         Once x64_simple_div1_def,REVERSE,mw_simple_div_def]
+  \\ SIMP_TAC std_ss [LENGTH,Once mc_simple_div1_pre_def,
+         Once mc_simple_div1_def,REVERSE,mw_simple_div_def]
   \\ FULL_SIMP_TAC (srw_ss()) [n2w_11,LET_DEF]
   \\ FULL_SIMP_TAC std_ss [ADD1,GSYM word_add_n2w,GSYM word_sub_def,WORD_ADD_SUB]
   \\ IMP_RES_TAC (DECIDE ``n+1<k ==> n<k:num``)
   \\ FULL_SIMP_TAC (srw_ss()) []
   \\ FULL_SIMP_TAC std_ss [SNOC_APPEND,GSYM APPEND_ASSOC,APPEND,LUPDATE_LENGTH]
   \\ FULL_SIMP_TAC std_ss [rich_listTheory.EL_LENGTH_APPEND,NULL,HD]
-  \\ FULL_SIMP_TAC std_ss [LUPDATE_LENGTH,x64_single_div_thm]
+  \\ FULL_SIMP_TAC std_ss [LUPDATE_LENGTH,mc_single_div_thm]
   \\ `?q1 r1. single_div r2 x r9 = (q1,r1)` by METIS_TAC [PAIR]
   \\ `?qs2 r2 c2. mw_simple_div r1 (REVERSE zs) r9 = (qs2,r2,c2)` by METIS_TAC [PAIR]
   \\ FULL_SIMP_TAC std_ss [LET_DEF] \\ rfs []
@@ -1630,26 +1630,26 @@ val x64_simple_div1_thm = prove(
 
 (* mw_div -- calc_d *)
 
-val (x64_calc_d_def, _,
-     x64_calc_d_pre_def, _) =
-  tailrec_define "x64_calc_d" ``
+val (mc_calc_d_def, _,
+     mc_calc_d_pre_def, _) =
+  tailrec_define "mc_calc_d" ``
     (\(l,r1,r2).
       (if r1 < 0w then (INR (l,r2),T) else
          (let r1 = r1 + r1 in let r2 = r2 + r2 in (INL (l-1,r1,r2),l <> 0))))
     :num # 'a word # 'a word -> (num # 'a word # 'a word + num # 'a word) # bool``;
 
-val x64_calc_d_thm = prove(
+val mc_calc_d_thm = prove(
   ``!(v1:'a word) d.
       (\(v1,d).
         !l n.
           (v1 <> 0w) /\ dimword (:'a) <= w2n v1 * 2 ** n /\ n <= l ==>
           ?l2.
-            x64_calc_d_pre (l,v1,d) /\
-            (x64_calc_d (l,v1,d) = (l2,calc_d (v1,d))) /\
+            mc_calc_d_pre (l,v1,d) /\
+            (mc_calc_d (l,v1,d) = (l2,calc_d (v1,d))) /\
             l <= l2 + n) (v1,d)``,
   MATCH_MP_TAC (calc_d_ind)
   \\ FULL_SIMP_TAC std_ss [] \\ rpt STRIP_TAC
-  \\ ONCE_REWRITE_TAC [x64_calc_d_pre_def,x64_calc_d_def,calc_d_def]
+  \\ ONCE_REWRITE_TAC [mc_calc_d_pre_def,mc_calc_d_def,calc_d_def]
   \\ FULL_SIMP_TAC std_ss [LET_THM,GSYM wordsTheory.word_msb_neg]
   \\ IF_CASES_TAC \\ fs []
   \\ FULL_SIMP_TAC std_ss [GSYM addressTheory.WORD_TIMES2,
@@ -1679,9 +1679,9 @@ val x64_calc_d_thm = prove(
 
 (* mw_div -- mw_div_guess *)
 
-val (x64_single_mul_def, _,
-     x64_single_mul_pre_def, _) =
-  tailrec_define "x64_single_mul" ``
+val (mc_single_mul_def, _,
+     mc_single_mul_pre_def, _) =
+  tailrec_define "mc_single_mul" ``
     (\(r0,r1,r2).
       (let cond = T in
        let (r0,r2) = single_mul r0 r2 0w in
@@ -1692,13 +1692,13 @@ val (x64_single_mul_def, _,
     :'a word # 'a word # 'a word -> ('a word # 'a word # 'a word + 'a
     word # 'a word # 'a word) # bool``;
 
-val x64_single_mul_def = LIST_CONJ [x64_single_mul_def,x64_single_mul_pre_def]
+val mc_single_mul_def = LIST_CONJ [mc_single_mul_def,mc_single_mul_pre_def]
 
 val single_mul_add_thm  = prove(
   ``single_mul_add p q k s =
-      (let (r0,r1,r2,r3) = x64_single_mul_add (p,k,q,s) in
+      (let (r0,r1,r2,r3) = mc_single_mul_add (p,k,q,s) in
          (r0,r2))``,
-  SIMP_TAC std_ss [x64_single_mul_add_thm]
+  SIMP_TAC std_ss [mc_single_mul_add_thm]
   \\ Q.SPEC_TAC (`single_mul_add p q k s`,`w`)
   \\ FULL_SIMP_TAC std_ss [FORALL_PROD,LET_DEF]);
 
@@ -1707,31 +1707,31 @@ val single_add_0_F = prove(
   fs [single_add_def,EVAL ``b2w F``,b2n_def,GSYM NOT_LESS,w2n_lt]
   \\ eq_tac \\ rw []);
 
-val x64_single_mul_thm = prove(
-  ``x64_single_mul_pre (p,k,q) /\
-    (x64_single_mul (p,k,q) =
+val mc_single_mul_thm = prove(
+  ``mc_single_mul_pre (p,k,q) /\
+    (mc_single_mul (p,k,q) =
       let (x1,x2) = single_mul_add p q k 0w in (x1,k,x2))``,
-  SIMP_TAC (srw_ss()) [single_mul_add_thm,x64_single_mul_def,LET_DEF,
-    x64_single_mul_add_def,single_add_word_def] \\ SIMP_TAC std_ss []
+  SIMP_TAC (srw_ss()) [single_mul_add_thm,mc_single_mul_def,LET_DEF,
+    mc_single_mul_add_def,single_add_word_def] \\ SIMP_TAC std_ss []
   \\ SIMP_TAC std_ss [GSYM NOT_LESS,w2n_lt,EVAL ``b2n F``,WORD_ADD_0]
   \\ rpt (pairarg_tac \\ fs [])
   \\ rw [] \\ fs [single_add_0_F] \\ rw [] \\ fs [single_add_0_F]);
 
-val (x64_mul_by_single2_def, _,
-     x64_mul_by_single2_pre_def, _) =
-  tailrec_define "x64_mul_by_single2" ``
+val (mc_mul_by_single2_def, _,
+     mc_mul_by_single2_pre_def, _) =
+  tailrec_define "mc_mul_by_single2" ``
     (\(r6,r7,r8).
       (let r0 = r6 in
        let r1 = 0x0w in
        let r2 = r7 in
-       let cond = x64_single_mul_pre (r0,r1,r2) in
-       let (r0,r1,r2) = x64_single_mul (r0,r1,r2) in
+       let cond = mc_single_mul_pre (r0,r1,r2) in
+       let (r0,r1,r2) = mc_single_mul (r0,r1,r2) in
        let r12 = r0 in
        let r0 = r6 in
        let r1 = r2 in
        let r2 = r8 in
-       let cond = cond /\ x64_single_mul_pre (r0,r1,r2) in
-       let (r0,r1,r2) = x64_single_mul (r0,r1,r2) in
+       let cond = cond /\ mc_single_mul_pre (r0,r1,r2) in
+       let (r0,r1,r2) = mc_single_mul (r0,r1,r2) in
        let r3 = r2 in
        let r2 = r0 in
        let r1 = r12
@@ -1740,24 +1740,24 @@ val (x64_mul_by_single2_def, _,
     :'a word # 'a word # 'a word -> ('a word # 'a word # 'a word + 'a
      word # 'a word # 'a word # 'a word # 'a word # 'a word) # bool``;
 
-val x64_mul_by_single2_thm = prove(
+val mc_mul_by_single2_thm = prove(
   ``!r6 r7 r8.
       ?r1 r2 r3.
-        x64_mul_by_single2_pre (r6,r7,r8) /\
-        (x64_mul_by_single2 (r6,r7,r8) = (r1,r2,r3,r6,r7,r8)) /\
+        mc_mul_by_single2_pre (r6,r7,r8) /\
+        (mc_mul_by_single2 (r6,r7,r8) = (r1,r2,r3,r6,r7,r8)) /\
         (mw_mul_by_single r6 [r7; r8] = [r1; r2; r3])``,
-  SIMP_TAC std_ss [mw_mul_by_single_def,LENGTH,mw_mul_pass_def,x64_single_mul_thm,
-    k2mw_def,HD,TL,x64_mul_by_single2_def,EVAL ``(k2mw 2 0):'a word list``,LET_DEF]
+  SIMP_TAC std_ss [mw_mul_by_single_def,LENGTH,mw_mul_pass_def,mc_single_mul_thm,
+    k2mw_def,HD,TL,mc_mul_by_single2_def,EVAL ``(k2mw 2 0):'a word list``,LET_DEF]
   \\ CONV_TAC (DEPTH_CONV (PairRules.PBETA_CONV))
   \\ assume_tac ZERO_LT_dimword
-  \\ ASM_SIMP_TAC std_ss [x64_mul_by_single2_pre_def,LET_DEF,x64_single_mul_add_def,ZERO_DIV]
+  \\ ASM_SIMP_TAC std_ss [mc_mul_by_single2_pre_def,LET_DEF,mc_single_mul_add_def,ZERO_DIV]
   \\ CONV_TAC (DEPTH_CONV (PairRules.PBETA_CONV))
-  \\ SIMP_TAC std_ss [x64_mul_by_single2_pre_def,LET_DEF,x64_single_mul_add_def]
-  \\ SIMP_TAC std_ss [x64_single_mul_thm] \\ EVAL_TAC);
+  \\ SIMP_TAC std_ss [mc_mul_by_single2_pre_def,LET_DEF,mc_single_mul_add_def]
+  \\ SIMP_TAC std_ss [mc_single_mul_thm] \\ EVAL_TAC);
 
-val (x64_cmp3_def, _,
-     x64_cmp3_pre_def, _) =
-  tailrec_define "x64_cmp3" ``
+val (mc_cmp3_def, _,
+     mc_cmp3_pre_def, _) =
+  tailrec_define "mc_cmp3" ``
     (\(r1,r2,r3,r9,r10,r11).
       (let r0 = 0x1w
        in
@@ -1776,13 +1776,13 @@ val (x64_cmp3_def, _,
      # 'a word # 'a word # 'a word # 'a word # 'a word # 'a word) #
      bool``;
 
-val x64_cmp3_thm = prove(
-  ``x64_cmp3_pre (r1,r2,r3,r9,r10,r11) /\
-    (x64_cmp3 (r1,r2,r3,r9,r10,r11) =
+val mc_cmp3_thm = prove(
+  ``mc_cmp3_pre (r1,r2,r3,r9,r10,r11) /\
+    (mc_cmp3 (r1,r2,r3,r9,r10,r11) =
       (if mw_cmp [r9;r10;r11] [r1;r2;r3] = SOME T then 1w else 0w,
        r1,r2,r3,r9,r10,r11))``,
   NTAC 5 (ONCE_REWRITE_TAC [mw_cmp_def])
-  \\ SIMP_TAC (srw_ss()) [x64_cmp3_def,x64_cmp3_pre_def,LET_DEF]
+  \\ SIMP_TAC (srw_ss()) [mc_cmp3_def,mc_cmp3_pre_def,LET_DEF]
   \\ Tactical.REVERSE (Cases_on `r3 = r11`)
   \\ FULL_SIMP_TAC std_ss [] THEN1 SRW_TAC [] []
   \\ Tactical.REVERSE (Cases_on `r2 = r10`)
@@ -1790,13 +1790,13 @@ val x64_cmp3_thm = prove(
   \\ Tactical.REVERSE (Cases_on `r1 = r9`)
   \\ FULL_SIMP_TAC std_ss [] THEN1 SRW_TAC [] []);
 
-val (x64_cmp_mul2_def, _,
-     x64_cmp_mul2_pre_def, _) =
-  tailrec_define "x64_cmp_mul2" ``
+val (mc_cmp_mul2_def, _,
+     mc_cmp_mul2_pre_def, _) =
+  tailrec_define "mc_cmp_mul2" ``
     (\(r6,r7,r8,r9,r10,r11).
-      (let cond = x64_mul_by_single2_pre (r6,r7,r8) in
-       let (r1,r2,r3,r6,r7,r8) = x64_mul_by_single2 (r6,r7,r8) in
-       let (r0,r1,r2,r3,r9,r10,r11) = x64_cmp3 (r1,r2,r3,r9,r10,r11)
+      (let cond = mc_mul_by_single2_pre (r6,r7,r8) in
+       let (r1,r2,r3,r6,r7,r8) = mc_mul_by_single2 (r6,r7,r8) in
+       let (r0,r1,r2,r3,r9,r10,r11) = mc_cmp3 (r1,r2,r3,r9,r10,r11)
        in
          (INR (r0,r6,r7,r8,r9,r10,r11),cond)))
     :'a word # 'a word # 'a word # 'a word # 'a word # 'a word -> ('a
@@ -1804,32 +1804,32 @@ val (x64_cmp_mul2_def, _,
      # 'a word # 'a word # 'a word # 'a word # 'a word # 'a word) #
      bool``;
 
-val x64_cmp_mul2_thm = prove(
-  ``x64_cmp_mul2_pre (r6,r7,r8,r9,r10,r11) /\
-    (x64_cmp_mul2 (r6,r7,r8,r9,r10,r11) =
+val mc_cmp_mul2_thm = prove(
+  ``mc_cmp_mul2_pre (r6,r7,r8,r9,r10,r11) /\
+    (mc_cmp_mul2 (r6,r7,r8,r9,r10,r11) =
       ((if mw_cmp [r9;r10;r11] (mw_mul_by_single r6 [r7; r8]) = SOME T
             then 1w else 0w),r6,r7,r8,r9,r10,r11))``,
-  SIMP_TAC std_ss [x64_cmp_mul2_pre_def,x64_cmp_mul2_def]
-  \\ STRIP_ASSUME_TAC (x64_mul_by_single2_thm |> SPEC_ALL)
-  \\ FULL_SIMP_TAC std_ss [LET_DEF,x64_cmp3_thm]);
+  SIMP_TAC std_ss [mc_cmp_mul2_pre_def,mc_cmp_mul2_def]
+  \\ STRIP_ASSUME_TAC (mc_mul_by_single2_thm |> SPEC_ALL)
+  \\ FULL_SIMP_TAC std_ss [LET_DEF,mc_cmp3_thm]);
 
-val (x64_sub1_def, _,
-     x64_sub1_pre_def, _) =
-  tailrec_define "x64_sub1" ``
+val (mc_sub1_def, _,
+     mc_sub1_pre_def, _) =
+  tailrec_define "mc_sub1" ``
     (\r6.
       if r6 = 0x0w then (INR r6,T) else (let r6 = r6 - 0x1w in (INR r6,T)))
     :'a word -> ('a word + 'a word) # bool``;
 
-val x64_sub1_thm = prove(
-  ``!r6. x64_sub1_pre r6 /\ (x64_sub1 r6 = n2w (w2n r6 - 1))``,
-  Cases \\ ASM_SIMP_TAC (srw_ss()) [x64_sub1_pre_def,x64_sub1_def]
+val mc_sub1_thm = prove(
+  ``!r6. mc_sub1_pre r6 /\ (mc_sub1 r6 = n2w (w2n r6 - 1))``,
+  Cases \\ ASM_SIMP_TAC (srw_ss()) [mc_sub1_pre_def,mc_sub1_def]
   \\ Cases_on `n = 0` \\ FULL_SIMP_TAC std_ss [LET_DEF,GSYM word_sub_def]
   \\ `~(n < 1)` by DECIDE_TAC
   \\ ASM_SIMP_TAC std_ss [addressTheory.word_arith_lemma2]);
 
-val (x64_cmp2_def, _,
-     x64_cmp2_pre_def, _) =
-  tailrec_define "x64_cmp2" ``
+val (mc_cmp2_def, _,
+     mc_cmp2_pre_def, _) =
+  tailrec_define "mc_cmp2" ``
     (\(r0,r2,r10,r11).
       (let r1 = 0x1w
        in
@@ -1843,36 +1843,36 @@ val (x64_cmp2_def, _,
      word # 'a word + 'a word # 'a word # 'a word # 'a word # 'a word)
      # bool``;
 
-val x64_cmp2_thm = prove(
-  ``x64_cmp2_pre (r0,r2,r10,r11) /\
-    (x64_cmp2 (r0,r2,r10,r11) =
+val mc_cmp2_thm = prove(
+  ``mc_cmp2_pre (r0,r2,r10,r11) /\
+    (mc_cmp2 (r0,r2,r10,r11) =
       (r0,if mw_cmp [r10;r11] [r0;r2] = SOME T then 1w else 0w,
        r2,r10,r11))``,
   NTAC 5 (ONCE_REWRITE_TAC [mw_cmp_def])
-  \\ SIMP_TAC (srw_ss()) [x64_cmp2_def,x64_cmp2_pre_def,LET_DEF]
+  \\ SIMP_TAC (srw_ss()) [mc_cmp2_def,mc_cmp2_pre_def,LET_DEF]
   \\ Tactical.REVERSE (Cases_on `r2 = r11`)
   \\ FULL_SIMP_TAC std_ss [] THEN1 SRW_TAC [] []
   \\ Tactical.REVERSE (Cases_on `r0 = r10`)
   \\ FULL_SIMP_TAC std_ss [] THEN1 SRW_TAC [] []);
 
-val (x64_div_test_def, _,
-     x64_div_test_pre_def, _) =
-  tailrec_define "x64_div_test" ``
+val (mc_div_test_def, _,
+     mc_div_test_pre_def, _) =
+  tailrec_define "mc_div_test" ``
     (\(l,r6,r7,r8,r9,r10,r11).
-      (let cond = x64_cmp_mul2_pre (r6,r7,r8,r9,r10,r11) in
-       let (r0,r6,r7,r8,r9,r10,r11) = x64_cmp_mul2 (r6,r7,r8,r9,r10,r11)
+      (let cond = mc_cmp_mul2_pre (r6,r7,r8,r9,r10,r11) in
+       let (r0,r6,r7,r8,r9,r10,r11) = mc_cmp_mul2 (r6,r7,r8,r9,r10,r11)
        in
          if r0 = 0x0w then (INR (l,r6,r7,r8,r9,r10,r11),cond)
          else
-           (let r6 = x64_sub1 r6 in
+           (let r6 = mc_sub1 r6 in
             let r0 = r6 in
             let r1 = 0x0w in
             let r2 = r8 in
             let r3 = r1 in
-            let cond = cond /\ x64_single_mul_add_pre (r0,r1,r2,r3) in
-            let (r0,r1,r2,r3) = x64_single_mul_add (r0,r1,r2,r3) in
+            let cond = cond /\ mc_single_mul_add_pre (r0,r1,r2,r3) in
+            let (r0,r1,r2,r3) = mc_single_mul_add (r0,r1,r2,r3) in
             let r2 = r2 + 0x1w in
-            let (r0,r1,r2,r10,r11) = x64_cmp2 (r0,r2,r10,r11)
+            let (r0,r1,r2,r10,r11) = mc_cmp2 (r0,r2,r10,r11)
             in
               if r1 = 0x0w then (INR (l,r6,r7,r8,r9,r10,r11),cond)
               else (INL (l-1,r6,r7,r8,r9,r10,r11),cond /\ l <> 0n))))
@@ -1890,22 +1890,22 @@ val mw_add_0_1 = prove(
   SIMP_TAC (srw_ss()) [mw_add_def,HD,TL,single_add_def,b2w_def,
     LET_DEF,EVAL ``b2n F``,GSYM NOT_LESS,w2n_lt]);
 
-val x64_div_test_lemma = prove(
+val mc_div_test_lemma = prove(
   ``!q u1 u2 u3 v1 v2 l.
       w2n q <= l ==>
       ?l2.
-        x64_div_test_pre (l,q,v2,v1,u3,u2,u1) /\
-        (x64_div_test (l,q,v2,v1,u3,u2,u1) =
+        mc_div_test_pre (l,q,v2,v1,u3,u2,u1) /\
+        (mc_div_test (l,q,v2,v1,u3,u2,u1) =
            (l2,mw_div_test q u1 u2 u3 v1 v2,v2,v1,u3,u2,u1)) /\
         l <= l2 + w2n q``,
   HO_MATCH_MP_TAC mw_div_test_ind \\ rpt strip_tac
-  \\ ONCE_REWRITE_TAC [x64_div_test_def,x64_div_test_pre_def,mw_div_test_def]
-  \\ SIMP_TAC std_ss [x64_cmp_mul2_thm]
+  \\ ONCE_REWRITE_TAC [mc_div_test_def,mc_div_test_pre_def,mw_div_test_def]
+  \\ SIMP_TAC std_ss [mc_cmp_mul2_thm]
   \\ Cases_on `mw_cmp [u3; u2; u1] (mw_mul_by_single q [v2; v1]) = SOME T`
-  \\ ASM_SIMP_TAC std_ss [LET_DEF,GSYM one_neq_zero_word,x64_sub1_thm]
-  \\ FULL_SIMP_TAC std_ss [x64_single_mul_add_thm,GSYM single_mul_thm]
+  \\ ASM_SIMP_TAC std_ss [LET_DEF,GSYM one_neq_zero_word,mc_sub1_thm]
+  \\ FULL_SIMP_TAC std_ss [mc_single_mul_add_thm,GSYM single_mul_thm]
   \\ Cases_on `single_mul_add (n2w (w2n q - 1)) v1 0x0w 0x0w`
-  \\ FULL_SIMP_TAC std_ss [LET_DEF,x64_cmp2_thm]
+  \\ FULL_SIMP_TAC std_ss [LET_DEF,mc_cmp2_thm]
   \\ Q.MATCH_ASSUM_RENAME_TAC
        `single_mul_add (n2w (w2n q - 1)) v1 0x0w 0x0w = (q1,q2)`
   \\ FULL_SIMP_TAC std_ss [mw_add_0_1]
@@ -1924,23 +1924,23 @@ val x64_div_test_lemma = prove(
   \\ first_x_assum (qspec_then `l-1` mp_tac)
   \\ match_mp_tac IMP_IMP \\ conj_tac \\ fs []);
 
-val x64_div_test_thm = prove(
+val mc_div_test_thm = prove(
   ``!q u1 u2 u3 v1 (v2:'a word) l.
       dimword (:'a) <= l ==>
       ?l2.
-        x64_div_test_pre (l,q,v2,v1,u3,u2,u1) /\
-        (x64_div_test (l,q,v2,v1,u3,u2,u1) =
+        mc_div_test_pre (l,q,v2,v1,u3,u2,u1) /\
+        (mc_div_test (l,q,v2,v1,u3,u2,u1) =
            (l2,mw_div_test q u1 u2 u3 v1 v2,v2,v1,u3,u2,u1)) /\
         l <= l2 + dimword (:'a)``,
   rw [] \\ assume_tac (Q.SPEC `q` w2n_lt)
   \\ `w2n q <= l` by fs []
-  \\ imp_res_tac x64_div_test_lemma
+  \\ imp_res_tac mc_div_test_lemma
   \\ pop_assum (strip_assume_tac o SPEC_ALL)
   \\ fs []);
 
-val (x64_div_r1_def, _,
-     x64_div_r1_pre_def, _) =
-  tailrec_define "x64_div_r1" ``
+val (mc_div_r1_def, _,
+     mc_div_r1_pre_def, _) =
+  tailrec_define "mc_div_r1" ``
     (\(r0,r1,r2).
       if r2 <+ r1 then
         (let cond = single_div_pre r2 r0 r1 in
@@ -1951,51 +1951,51 @@ val (x64_div_r1_def, _,
     :'a word # 'a word # 'a word -> ('a word # 'a word # 'a word + 'a
     word # 'a word # 'a word) # bool``;
 
-val x64_div_r1_def = LIST_CONJ [x64_div_r1_def,x64_div_r1_pre_def]
+val mc_div_r1_def = LIST_CONJ [mc_div_r1_def,mc_div_r1_pre_def]
 
-val x64_div_r1_thm = prove(
-  ``x64_div_r1 (r0,r1,r2) =
+val mc_div_r1_thm = prove(
+  ``mc_div_r1 (r0,r1,r2) =
       if r2 <+ r1 then
         (FST (single_div r2 r0 r1),r1,SND (single_div r2 r0 r1))
       else (~0w,r1,r2)``,
-  SIMP_TAC (srw_ss()) [x64_div_r1_def,single_div_def,LET_DEF]);
+  SIMP_TAC (srw_ss()) [mc_div_r1_def,single_div_def,LET_DEF]);
 
-val (x64_div_guess_def, _,
-     x64_div_guess_pre_def, _) =
-  tailrec_define "x64_div_guess" ``
+val (mc_div_guess_def, _,
+     mc_div_guess_pre_def, _) =
+  tailrec_define "mc_div_guess" ``
     (\(l,r7,r8,r9,r10,r11).
       (let r0 = r10 in
        let r1 = r8 in
        let r2 = r11 in
-       let cond = x64_div_r1_pre (r0,r1,r2) in
-       let (r0,r1,r2) = x64_div_r1 (r0,r1,r2) in
+       let cond = mc_div_r1_pre (r0,r1,r2) in
+       let (r0,r1,r2) = mc_div_r1 (r0,r1,r2) in
        let r6 = r0 in
-       let cond = cond /\ x64_div_test_pre (l-1,r6,r7,r8,r9,r10,r11) /\ l <> 0 in
-       let (l,r6,r7,r8,r9,r10,r11) = x64_div_test (l-1,r6,r7,r8,r9,r10,r11)
+       let cond = cond /\ mc_div_test_pre (l-1,r6,r7,r8,r9,r10,r11) /\ l <> 0 in
+       let (l,r6,r7,r8,r9,r10,r11) = mc_div_test (l-1,r6,r7,r8,r9,r10,r11)
        in
          (INR (l,r6,r7,r8,r9,r10,r11),cond)))
     :num # 'a word # 'a word # 'a word # 'a word # 'a word ->
      (num # 'a word # 'a word # 'a word # 'a word # 'a word +
       num # 'a word # 'a word # 'a word # 'a word # 'a word # 'a word) # bool``;
 
-val x64_div_guess_thm = prove(
+val mc_div_guess_thm = prove(
   ``!u1 u2 u3 v1 v2:'a word.
       dimword (:'a) + 1 <= l ==>
       ?l2.
-        (x64_div_guess_pre (l,v2,v1,u3,u2,u1) <=>
+        (mc_div_guess_pre (l,v2,v1,u3,u2,u1) <=>
            (u1 <+ v1 ==> v1 <> 0w)) /\
-        (x64_div_guess (l,v2,v1,u3,u2,u1) =
+        (mc_div_guess (l,v2,v1,u3,u2,u1) =
            (l2,mw_div_guess (u1::u2::u3::us) (v1::v2::vs),v2,v1,u3,u2,u1)) /\
         l <= l2 + dimword (:'a) + 1``,
   rpt strip_tac
   \\ `dimword (:α) ≤ l - 1` by decide_tac
-  \\ imp_res_tac x64_div_test_thm
-  \\ SIMP_TAC (srw_ss()) [x64_div_guess_def,x64_div_guess_pre_def,
-       x64_div_test_thm, mw_div_guess_def,HD,TL,x64_div_r1_thm,LET_DEF]
-  \\ SIMP_TAC std_ss [x64_div_r1_def,LET_DEF,WORD_LO,single_div_pre_def]
+  \\ imp_res_tac mc_div_test_thm
+  \\ SIMP_TAC (srw_ss()) [mc_div_guess_def,mc_div_guess_pre_def,
+       mc_div_test_thm, mw_div_guess_def,HD,TL,mc_div_r1_thm,LET_DEF]
+  \\ SIMP_TAC std_ss [mc_div_r1_def,LET_DEF,WORD_LO,single_div_pre_def]
   \\ REPEAT STRIP_TAC
   \\ IF_CASES_TAC \\ fs []
-  \\ SEP_I_TAC "x64_div_test" \\ fs []
+  \\ SEP_I_TAC "mc_div_test" \\ fs []
   \\ FULL_SIMP_TAC (srw_ss()) [single_div_def]
   \\ FULL_SIMP_TAC std_ss [EVAL ``-1w:'a word``]
   \\ fs [word_2comp_def]
@@ -2026,9 +2026,9 @@ val x64_div_guess_thm = prove(
 
 *)
 
-val (x64_adj_cmp_def, _,
-     x64_adj_cmp_pre_def, _) =
-  tailrec_define "x64_adj_cmp" ``
+val (mc_adj_cmp_def, _,
+     mc_adj_cmp_pre_def, _) =
+  tailrec_define "mc_adj_cmp" ``
     (\(r0,r3,r8).
       if r0 = r3 then (INR (r0,r3,r8),T)
       else
@@ -2039,35 +2039,35 @@ val (x64_adj_cmp_def, _,
     :'a word # 'a word # 'a word -> ('a word # 'a word # 'a word + 'a
     word # 'a word # 'a word) # bool``;
 
-val (x64_adjust_aux_def, _,
-     x64_adjust_aux_pre_def, _) =
-  tailrec_define "x64_adjust_aux" ``
+val (mc_adjust_aux_def, _,
+     mc_adjust_aux_pre_def, _) =
+  tailrec_define "mc_adjust_aux" ``
     (\(l,r1,r6,r7,r8,r9,r10,r11,r12,ys,zs).
       if r9 = r11 then
         (let r0 = r12 in
          let cond = w2n r10 < LENGTH zs in
          let r3 = EL (w2n r10) zs in
          let r10 = r10 + 0x1w in
-         let (r0,r3,r8) = x64_adj_cmp (r0,r3,r8)
+         let (r0,r3,r8) = mc_adj_cmp (r0,r3,r8)
          in
            (INR (l,r6,r7,r8,r9,r10,r11,ys,zs),cond))
       else
         (let r0 = r6 in
          let cond = w2n r11 < LENGTH ys in
          let r2 = EL (w2n r11) ys in
-         let cond = cond /\ x64_single_mul_pre (r0,r1,r2) in
-         let (r0,r1,r2) = x64_single_mul (r0,r1,r2) in
+         let cond = cond /\ mc_single_mul_pre (r0,r1,r2) in
+         let (r0,r1,r2) = mc_single_mul (r0,r1,r2) in
          let r1 = r12 in
          let r12 = r2 in
          let r2 = r0 in
          let r0 = r7 in
-         let cond = cond /\ x64_single_mul_pre (r0,r1,r2) in
-         let (r0,r1,r2) = x64_single_mul (r0,r1,r2) in
+         let cond = cond /\ mc_single_mul_pre (r0,r1,r2) in
+         let (r0,r1,r2) = mc_single_mul (r0,r1,r2) in
          let r1 = r12 in
          let r12 = r2 in
          let cond = cond /\ w2n r10 < LENGTH zs in
          let r3 = EL (w2n r10) zs in
-         let (r0,r3,r8) = x64_adj_cmp (r0,r3,r8) in
+         let (r0,r3,r8) = mc_adj_cmp (r0,r3,r8) in
          let r11 = r11 + 0x1w in
          let r10 = r10 + 0x1w
          in
@@ -2079,17 +2079,17 @@ val (x64_adjust_aux_def, _,
     word # 'a word # 'a word # 'a word # 'a word list # 'a word list)
     # bool``;
 
-val (x64_div_adjust_def, _,
-     x64_div_adjust_pre_def, _) =
-  tailrec_define "x64_div_adjust" ``
+val (mc_div_adjust_def, _,
+     mc_div_adjust_pre_def, _) =
+  tailrec_define "mc_div_adjust" ``
     (\(l,r6,r7,r9,r10,ys,zs).
       (let r1 = 0x0w in
        let r8 = r1 in
        let r11 = r1 in
        let r12 = r1 in
-       let cond = x64_adjust_aux_pre (l-1,r1,r6,r7,r8,r9,r10,r11,r12,ys,zs) /\ l<>0 in
+       let cond = mc_adjust_aux_pre (l-1,r1,r6,r7,r8,r9,r10,r11,r12,ys,zs) /\ l<>0 in
        let (l,r6,r7,r8,r9,r10,r11,ys,zs) =
-             x64_adjust_aux (l-1,r1,r6,r7,r8,r9,r10,r11,r12,ys,zs)
+             mc_adjust_aux (l-1,r1,r6,r7,r8,r9,r10,r11,r12,ys,zs)
        in
          if r7 = 0x0w then (INR (l,r6,r7,r9,r10,r11,ys,zs),cond)
          else if r8 = 0x0w then (INR (l,r6,r7,r9,r10,r11,ys,zs),cond)
@@ -2099,11 +2099,11 @@ val (x64_div_adjust_def, _,
      word list # 'a word list + num # 'a word # 'a word # 'a word # 'a
      word # 'a word # 'a word list # 'a word list) # bool``;
 
-val x64_adj_cmp_thm = prove(
-  ``x64_adj_cmp_pre (r1,h,anything) /\
-    (x64_adj_cmp (r1,h,if res = SOME T then 0x1w else 0x0w) =
+val mc_adj_cmp_thm = prove(
+  ``mc_adj_cmp_pre (r1,h,anything) /\
+    (mc_adj_cmp (r1,h,if res = SOME T then 0x1w else 0x0w) =
       (r1,h,if mw_cmp_alt [h] [r1] res = SOME T then 0x1w else 0x0w))``,
-  SIMP_TAC std_ss [mw_cmp_alt_def,HD,TL,x64_adj_cmp_def,x64_adj_cmp_pre_def,LET_DEF]
+  SIMP_TAC std_ss [mw_cmp_alt_def,HD,TL,mc_adj_cmp_def,mc_adj_cmp_pre_def,LET_DEF]
   \\ Cases_on `r1 = h` \\ FULL_SIMP_TAC std_ss []
   \\ Cases_on `h <+ r1` \\ FULL_SIMP_TAC std_ss []);
 
@@ -2123,16 +2123,16 @@ val mw_cmp_alt_CONS = prove(
     mw_cmp_alt (z::zs) (q3::mw_mul_by_single2 r6 r7 ys q2 q4) res``,
   SIMP_TAC std_ss [mw_cmp_alt_def,TL,HD]);
 
-val x64_adjust_aux_thm = prove(
+val mc_adjust_aux_thm = prove(
   ``!(ys:'a word list) zs ys1 zs1 zs2 res r1 r12 l.
       (LENGTH zs = LENGTH ys + 1) /\ LENGTH (ys1 ++ ys) < dimword (:'a)
                                   /\ LENGTH (zs1 ++ zs) < dimword (:'a) /\
       LENGTH ys <= l ==>
       ?l2.
-        x64_adjust_aux_pre (l,r1,r6,r7,if res = SOME T then 1w else 0w,
+        mc_adjust_aux_pre (l,r1,r6,r7,if res = SOME T then 1w else 0w,
           n2w (LENGTH (ys1 ++ ys)), n2w (LENGTH zs1),n2w (LENGTH ys1),
           r12,ys1 ++ ys,zs1 ++ zs ++ zs2) /\
-        (x64_adjust_aux (l,r1,r6,r7,if res = SOME T then 1w else 0w,
+        (mc_adjust_aux (l,r1,r6,r7,if res = SOME T then 1w else 0w,
           n2w (LENGTH (ys1 ++ ys)), n2w (LENGTH zs1),n2w (LENGTH ys1),
           r12,ys1 ++ ys,zs1 ++ zs ++ zs2) =
           (l2,r6,r7,if mw_cmp_alt zs (mw_mul_by_single2 r6 r7 ys r1 r12) res = SOME T
@@ -2143,15 +2143,15 @@ val x64_adjust_aux_thm = prove(
    (SIMP_TAC std_ss [APPEND_NIL,mw_mul_by_single2_def,LENGTH]
     \\ Cases \\ SIMP_TAC std_ss [LENGTH]
     \\ Cases_on `t` \\ SIMP_TAC std_ss [LENGTH,ADD1]
-    \\ ONCE_REWRITE_TAC [x64_adjust_aux_def,x64_adjust_aux_pre_def]
+    \\ ONCE_REWRITE_TAC [mc_adjust_aux_def,mc_adjust_aux_pre_def]
     \\ SIMP_TAC std_ss [LET_DEF,LENGTH_APPEND,LENGTH]
     \\ NTAC 7 STRIP_TAC
     \\ `LENGTH zs1 < dimword (:'a)` by DECIDE_TAC
     \\ FULL_SIMP_TAC std_ss [APPEND,GSYM APPEND_ASSOC,w2n_n2w,
          rich_listTheory.EL_LENGTH_APPEND,NULL_DEF,HD]
-    \\ REWRITE_TAC [x64_adj_cmp_thm] \\ SIMP_TAC std_ss [word_add_n2w]
+    \\ REWRITE_TAC [mc_adj_cmp_thm] \\ SIMP_TAC std_ss [word_add_n2w]
     \\ DECIDE_TAC)
-  \\ ONCE_REWRITE_TAC [x64_adjust_aux_def,x64_adjust_aux_pre_def]
+  \\ ONCE_REWRITE_TAC [mc_adjust_aux_def,mc_adjust_aux_pre_def]
   \\ Cases_on `zs` \\ SIMP_TAC std_ss [LENGTH,ADD1] \\ rpt STRIP_TAC
   \\ Q.MATCH_ASSUM_RENAME_TAC `LENGTH (zs1 ++ z::zs) < dimword (:'a)`
   \\ POP_ASSUM MP_TAC
@@ -2161,8 +2161,8 @@ val x64_adjust_aux_thm = prove(
    (FULL_SIMP_TAC std_ss [LENGTH_APPEND]
     \\ `LENGTH ys1 < dimword(:'a)` by DECIDE_TAC
     \\ FULL_SIMP_TAC std_ss [n2w_11,LENGTH,ADD1])
-  \\ FULL_SIMP_TAC std_ss [word_add_n2w,x64_adj_cmp_thm,x64_single_mul_add_thm,
-        x64_single_mul_thm]
+  \\ FULL_SIMP_TAC std_ss [word_add_n2w,mc_adj_cmp_thm,mc_single_mul_add_thm,
+        mc_single_mul_thm]
   \\ `LENGTH zs1 < dimword (:'a) /\ LENGTH ys1 < dimword (:'a)` by
        (FULL_SIMP_TAC (srw_ss()) [LENGTH_APPEND,LENGTH] \\ DECIDE_TAC)
   \\ FULL_SIMP_TAC std_ss [w2n_n2w,EL_LENGTH,LET_DEF,mw_mul_by_single2_def]
@@ -2178,21 +2178,21 @@ val x64_adjust_aux_thm = prove(
   |> Q.SPECL [`ys`,`zs`,`[]`,`zs1`,`zs2`,`NONE`,`0w`,`0w`]
   |> SIMP_RULE std_ss [LENGTH,APPEND] |> GEN_ALL;
 
-val x64_div_adjust_thm = prove(
+val mc_div_adjust_thm = prove(
   ``(LENGTH zs = LENGTH ys + 1) /\ LENGTH (ys:'a word list) < dimword (:'a)
                                 /\ LENGTH (zs1 ++ zs) < dimword (:'a) /\
     LENGTH ys + 1 <= l ==>
     ?l2.
-      x64_div_adjust_pre (l,r6,r7,n2w (LENGTH ys),n2w (LENGTH zs1),
+      mc_div_adjust_pre (l,r6,r7,n2w (LENGTH ys),n2w (LENGTH zs1),
                           ys,zs1 ++ zs ++ zs2) /\
-      (x64_div_adjust (l,r6,r7,n2w (LENGTH ys),n2w (LENGTH zs1),
+      (mc_div_adjust (l,r6,r7,n2w (LENGTH ys),n2w (LENGTH zs1),
                        ys,zs1 ++ zs ++ zs2) =
         (l2,r6,mw_div_adjust r7 zs (FRONT (mw_mul_by_single r6 ys)),
          n2w (LENGTH ys),n2w (LENGTH (zs1 ++ zs)),n2w (LENGTH ys),
          ys,zs1 ++ zs ++ zs2)) /\
       l <= l2 + LENGTH ys + 1``,
-  SIMP_TAC std_ss [x64_div_adjust_def,x64_div_adjust_pre_def,LET_DEF]
-  \\ ASSUME_TAC x64_adjust_aux_thm \\ SEP_I_TAC "x64_adjust_aux"
+  SIMP_TAC std_ss [mc_div_adjust_def,mc_div_adjust_pre_def,LET_DEF]
+  \\ ASSUME_TAC mc_adjust_aux_thm \\ SEP_I_TAC "mc_adjust_aux"
   \\ STRIP_TAC \\ FULL_SIMP_TAC std_ss [mw_div_adjust_def] \\ fs []
   \\ SIMP_TAC std_ss [GSYM mw_mul_by_single2_thm]
   \\ `mw_cmp_alt zs (mw_mul_by_single2 r6 r7 ys 0x0w 0x0w) NONE =
@@ -2211,9 +2211,9 @@ val x64_div_adjust_thm = prove(
 
 (* mw_div -- mw_sub *)
 
-val (x64_div_sub_def, _,
-     x64_div_sub_pre_def, _) =
-  tailrec_define "x64_div_sub" ``
+val (mc_div_sub_def, _,
+     mc_div_sub_pre_def, _) =
+  tailrec_define "mc_div_sub" ``
     (\(r0,r3,r8).
       (let cond = ((r8 <> 0w) ==> (r8 = 1w)) in
        let (r3,r8) = single_sub_word r3 r0 r8 in
@@ -2221,29 +2221,29 @@ val (x64_div_sub_def, _,
     :'a word # 'a word # 'a word -> ('a word # 'a word # 'a word + 'a
     word # 'a word # 'a word) # bool``;
 
-val x64_div_sub_def = LIST_CONJ [x64_div_sub_def,x64_div_sub_pre_def]
+val mc_div_sub_def = LIST_CONJ [mc_div_sub_def,mc_div_sub_pre_def]
 
 val b2n_thm = prove(
   ``b2n = b2n``,
   FULL_SIMP_TAC std_ss [FUN_EQ_THM] \\ Cases \\ EVAL_TAC);
 
-val x64_div_sub_thm = prove(
-  ``x64_div_sub_pre (r0,r3,b2w c) /\
-    (x64_div_sub (r0,r3,b2w c) =
+val mc_div_sub_thm = prove(
+  ``mc_div_sub_pre (r0,r3,b2w c) /\
+    (mc_div_sub (r0,r3,b2w c) =
        let (r3,c) = single_sub r3 r0 c in
          (r0,r3,b2w c))``,
-  SIMP_TAC std_ss [single_sub_def,x64_div_sub_def,LET_DEF,single_sub_word_def]
+  SIMP_TAC std_ss [single_sub_def,mc_div_sub_def,LET_DEF,single_sub_word_def]
   \\ fs [] \\ rpt (pairarg_tac \\ fs []));
 
-val (x64_div_sub_loop_def, _,
-     x64_div_sub_loop_pre_def, _) =
-  tailrec_define "x64_div_sub_loop" ``
+val (mc_div_sub_loop_def, _,
+     mc_div_sub_loop_pre_def, _) =
+  tailrec_define "mc_div_sub_loop" ``
     (\(l,r1,r6,r7,r8,r9,r10,r11,r12,ys,zs).
       if r9 = r11 then
         (let r0 = r12 in
          let cond = w2n r10 < LENGTH zs in
          let r3 = EL (w2n r10) zs in
-         let (r0,r3,r8) = x64_div_sub (r0,r3,r8) in
+         let (r0,r3,r8) = mc_div_sub (r0,r3,r8) in
          let r1 = r3 in
          let zs = LUPDATE r1 (w2n r10) zs in
          let r10 = r10 + 0x1w
@@ -2253,19 +2253,19 @@ val (x64_div_sub_loop_def, _,
         (let r0 = r6 in
          let cond = w2n r11 < LENGTH ys in
          let r2 = EL (w2n r11) ys in
-         let cond = cond /\ x64_single_mul_pre (r0,r1,r2) in
-         let (r0,r1,r2) = x64_single_mul (r0,r1,r2) in
+         let cond = cond /\ mc_single_mul_pre (r0,r1,r2) in
+         let (r0,r1,r2) = mc_single_mul (r0,r1,r2) in
          let r1 = r12 in
          let r12 = r2 in
          let r2 = r0 in
          let r0 = r7 in
-         let cond = cond /\ x64_single_mul_pre (r0,r1,r2) in
-         let (r0,r1,r2) = x64_single_mul (r0,r1,r2) in
+         let cond = cond /\ mc_single_mul_pre (r0,r1,r2) in
+         let (r0,r1,r2) = mc_single_mul (r0,r1,r2) in
          let r1 = r12 in
          let r12 = r2 in
          let cond = cond /\ w2n r10 < LENGTH zs in
          let r3 = EL (w2n r10) zs in
-         let (r0,r3,r8) = x64_div_sub (r0,r3,r8) in
+         let (r0,r3,r8) = mc_div_sub (r0,r3,r8) in
          let r0 = r1 in
          let r1 = r3 in
          let zs = LUPDATE r1 (w2n r10) zs in
@@ -2286,16 +2286,16 @@ val LUPDATE_THM = prove(
     (LUPDATE q (LENGTH xs) (SNOC x xs ++ ys ++ zs) = SNOC q xs ++ ys ++ zs)``,
   SIMP_TAC std_ss [SNOC_APPEND,GSYM APPEND_ASSOC,APPEND,LUPDATE_LENGTH]);
 
-val x64_div_sub_loop_thm = prove(
+val mc_div_sub_loop_thm = prove(
   ``!(ys:'a word list) zs ys1 zs1 zs2 c r1 r12 l.
       (LENGTH zs = LENGTH ys + 1) /\ LENGTH (ys1 ++ ys) < dimword (:'a)
                                   /\ LENGTH (zs1 ++ zs) < dimword (:'a) /\
       LENGTH ys <= l ==>
       ?l2.
-        x64_div_sub_loop_pre (l,r1,r6,r7,b2w c,
+        mc_div_sub_loop_pre (l,r1,r6,r7,b2w c,
           n2w (LENGTH (ys1 ++ ys)), n2w (LENGTH zs1),n2w (LENGTH ys1),
           r12,ys1 ++ ys,zs1 ++ zs ++ zs2) /\
-        (x64_div_sub_loop (l,r1,r6,r7,b2w c,
+        (mc_div_sub_loop (l,r1,r6,r7,b2w c,
           n2w (LENGTH (ys1 ++ ys)), n2w (LENGTH zs1),n2w (LENGTH ys1),
           r12,ys1 ++ ys,zs1 ++ zs ++ zs2) =
           (l2,r6,r7,n2w (LENGTH (ys1 ++ ys)),n2w (LENGTH (zs1 ++ zs)),
@@ -2306,17 +2306,17 @@ val x64_div_sub_loop_thm = prove(
    (SIMP_TAC std_ss [APPEND_NIL,mw_mul_by_single2_def,LENGTH]
     \\ Cases \\ SIMP_TAC std_ss [LENGTH]
     \\ Cases_on `t` \\ SIMP_TAC std_ss [LENGTH,ADD1]
-    \\ ONCE_REWRITE_TAC [x64_div_sub_loop_def,x64_div_sub_loop_pre_def]
+    \\ ONCE_REWRITE_TAC [mc_div_sub_loop_def,mc_div_sub_loop_pre_def]
     \\ SIMP_TAC std_ss [LET_DEF,LENGTH_APPEND,LENGTH]
     \\ rpt STRIP_TAC
     \\ `LENGTH zs1 < dimword (:'a)` by DECIDE_TAC
     \\ FULL_SIMP_TAC std_ss [word_add_n2w,w2n_n2w,EL_LENGTH]
     \\ FULL_SIMP_TAC std_ss [LUPDATE_THM,APPEND_NIL,SNOC_INTRO]
-    \\ FULL_SIMP_TAC std_ss [SNOC_INTRO,x64_div_sub_thm]
+    \\ FULL_SIMP_TAC std_ss [SNOC_INTRO,mc_div_sub_thm]
     \\ FULL_SIMP_TAC std_ss [mw_sub_def,HD,TL]
     \\ Cases_on `single_sub h r12 c`
     \\ FULL_SIMP_TAC std_ss [LET_DEF,SNOC_INTRO,APPEND_NIL] \\ DECIDE_TAC)
-  \\ ONCE_REWRITE_TAC [x64_div_sub_loop_def,x64_div_sub_loop_pre_def]
+  \\ ONCE_REWRITE_TAC [mc_div_sub_loop_def,mc_div_sub_loop_pre_def]
   \\ Cases_on `zs` \\ SIMP_TAC std_ss [LENGTH,ADD1] \\ rpt STRIP_TAC
   \\ Q.MATCH_ASSUM_RENAME_TAC `LENGTH (zs1 ++ z::zs) < dimword (:'a)`
   \\ POP_ASSUM MP_TAC
@@ -2326,14 +2326,14 @@ val x64_div_sub_loop_thm = prove(
    (FULL_SIMP_TAC std_ss [LENGTH_APPEND]
     \\ `LENGTH ys1 < dimword(:'a)` by DECIDE_TAC
     \\ FULL_SIMP_TAC std_ss [n2w_11,LENGTH,ADD1])
-  \\ FULL_SIMP_TAC std_ss [word_add_n2w,x64_adj_cmp_thm,x64_single_mul_add_thm,
-        x64_single_mul_thm]
+  \\ FULL_SIMP_TAC std_ss [word_add_n2w,mc_adj_cmp_thm,mc_single_mul_add_thm,
+        mc_single_mul_thm]
   \\ `LENGTH zs1 < dimword (:'a) /\ LENGTH ys1 < dimword (:'a)` by
        (FULL_SIMP_TAC (srw_ss()) [LENGTH_APPEND,LENGTH] \\ DECIDE_TAC)
   \\ FULL_SIMP_TAC std_ss [w2n_n2w,EL_LENGTH,LET_DEF,mw_mul_by_single2_def]
   \\ `?q1 q2. single_mul_add r6 y r1 0x0w = (q1,q2)` by METIS_TAC [PAIR]
   \\ `?q3 q4. single_mul_add r7 q1 r12 0x0w = (q3,q4)` by METIS_TAC [PAIR]
-  \\ FULL_SIMP_TAC std_ss [SNOC_INTRO,x64_div_sub_thm]
+  \\ FULL_SIMP_TAC std_ss [SNOC_INTRO,mc_div_sub_thm]
   \\ FULL_SIMP_TAC std_ss [mw_sub_def,HD,TL]
   \\ Cases_on `single_sub z q3 c`
   \\ FULL_SIMP_TAC std_ss [LET_DEF]
@@ -2354,9 +2354,9 @@ val x64_div_sub_loop_thm = prove(
 
 (* mw_div -- mw_div_aux *)
 
-val (x64_div_loop_def, _,
-     x64_div_loop_pre_def, _) =
-  tailrec_define "x64_div_loop" ``
+val (mc_div_loop_def, _,
+     mc_div_loop_pre_def, _) =
+  tailrec_define "mc_div_loop" ``
     (\(l,r7:'a word,r9:'a word,r10:'a word,r11:'a word,
        r14:'a word,r15:'a word,ys:'a word list,zs:'a word list).
       if r10 = 0x0w then (INR (l,r7,r9,r10,r11,r14,r15,ys,zs),T)
@@ -2381,8 +2381,8 @@ val (x64_div_loop_def, _,
          let r9 = r2 in
          let r7 = r3 in
          let r8 = r6 in
-         let cond = cond /\ x64_div_guess_pre (l,r7,r8,r9,r10,r11) in
-         let (l,r6,r7,r8,r9,r10,r11) = x64_div_guess (l,r7,r8,r9,r10,r11) in
+         let cond = cond /\ mc_div_guess_pre (l,r7,r8,r9,r10,r11) in
+         let (l,r6,r7,r8,r9,r10,r11) = mc_div_guess (l,r7,r8,r9,r10,r11) in
          let r0 = r6 in
          let r6 = r14 in
          let r9 = r15 in
@@ -2391,8 +2391,8 @@ val (x64_div_loop_def, _,
          let r15 = r7 in
          let r14 = r8 in
          let r7 = r0 in
-         let cond = cond /\ x64_div_adjust_pre (l,r6,r7,r9,r10,ys,zs) in
-         let (l,r6,r7,r9,r10,r11,ys,zs) = x64_div_adjust (l,r6,r7,r9,r10,ys,zs) in
+         let cond = cond /\ mc_div_adjust_pre (l,r6,r7,r9,r10,ys,zs) in
+         let (l,r6,r7,r9,r10,r11,ys,zs) = mc_div_adjust (l,r6,r7,r9,r10,ys,zs) in
          let r10 = r10 - r9 in
          let r10 = r10 - 0x1w in
          let r1 = 0x0w in
@@ -2402,10 +2402,10 @@ val (x64_div_loop_def, _,
          let r12 = r1 in
          let cond =
                cond /\
-               x64_div_sub_loop_pre (l-1,r1,r6,r7,r8,r9,r10,r11,r12,ys,zs) /\ l <> 0
+               mc_div_sub_loop_pre (l-1,r1,r6,r7,r8,r9,r10,r11,r12,ys,zs) /\ l <> 0
          in
          let (l,r6,r7,r9,r10,r11,ys,zs) =
-               x64_div_sub_loop (l-1,r1,r6,r7,r8,r9,r10,r11,r12,ys,zs)
+               mc_div_sub_loop (l-1,r1,r6,r7,r8,r9,r10,r11,r12,ys,zs)
          in
          let r10 = r10 - 0x1w in
          let cond = cond /\ w2n r10 < LENGTH zs in
@@ -2415,16 +2415,16 @@ val (x64_div_loop_def, _,
          in
            (INL (l-1,r7,r9,r10,r11,r14,r15,ys,zs),cond /\ l <> 0)))``;
 
-val x64_div_loop_thm = prove(
+val mc_div_loop_thm = prove(
   ``!(zs1:'a word list) zs ys1 zs2 c r1 r12 l.
       (LENGTH zs = LENGTH ys) /\ LENGTH (zs1 ++ zs ++ zs2) < dimword (:'a) /\
       1 < LENGTH ys /\ LAST (FRONT (mw_mul_by_single d ys)) <> 0x0w /\
       LENGTH zs1 * (dimword (:'a) + 2 * LENGTH ys + 4) <= l ==>
       ?l2.
         let ys1 = (FRONT (mw_mul_by_single d ys)) in
-          x64_div_loop_pre (l,d,n2w (LENGTH ys),n2w (LENGTH zs1),n2w (LENGTH ys),
+          mc_div_loop_pre (l,d,n2w (LENGTH ys),n2w (LENGTH zs1),n2w (LENGTH ys),
             LAST ys1,LAST (BUTLAST ys1),ys,zs1 ++ zs ++ zs2) /\
-          (x64_div_loop (l,d,n2w (LENGTH ys),n2w (LENGTH zs1),n2w (LENGTH ys),
+          (mc_div_loop (l,d,n2w (LENGTH ys),n2w (LENGTH zs1),n2w (LENGTH ys),
             LAST ys1,LAST (BUTLAST ys1),ys,zs1 ++ zs ++ zs2) =
             (l2,d,n2w (LENGTH ys),0w,n2w (LENGTH ys),LAST ys1,LAST (BUTLAST ys1),ys,
              (let (qs,rs) = mw_div_aux zs1 zs ys1 in
@@ -2434,7 +2434,7 @@ val x64_div_loop_thm = prove(
   \\ SIMP_TAC std_ss [LET_DEF] \\ HO_MATCH_MP_TAC SNOC_INDUCT
   \\ STRIP_TAC THEN1 (SIMP_TAC std_ss
     [LENGTH,APPEND,Once mw_div_aux_def,APPEND_NIL,
-     Once x64_div_loop_def,Once x64_div_loop_pre_def,REVERSE_DEF])
+     Once mc_div_loop_def,Once mc_div_loop_pre_def,REVERSE_DEF])
   \\ NTAC 2 STRIP_TAC
   \\ ONCE_REWRITE_TAC [mw_div_aux_def] \\ NTAC 5 STRIP_TAC
   \\ SIMP_TAC std_ss [LAST_SNOC,FRONT_SNOC,rich_listTheory.NOT_SNOC_NIL]
@@ -2444,7 +2444,7 @@ val x64_div_loop_thm = prove(
   \\ Q.ABBREV_TAC `sub = (FST (mw_sub (x::zs) (mw_mul_by_single adj ys1) T))`
   \\ `?qs1 rs1. mw_div_aux zs1 (FRONT sub) ys1 = (qs1,rs1)` by METIS_TAC [PAIR]
   \\ FULL_SIMP_TAC std_ss []
-  \\ ONCE_REWRITE_TAC [x64_div_loop_def,x64_div_loop_pre_def]
+  \\ ONCE_REWRITE_TAC [mc_div_loop_def,mc_div_loop_pre_def]
   \\ FULL_SIMP_TAC std_ss [n2w_11,LENGTH_APPEND]
   \\ IMP_RES_TAC (DECIDE ``n + m + k < d ==> 0 < d /\ n < d:num``)
   \\ FULL_SIMP_TAC std_ss [n2w_11,LENGTH_APPEND]
@@ -2498,10 +2498,10 @@ val x64_div_loop_thm = prove(
          LENGTH,ADD1,SNOC_APPEND] \\ SIMP_TAC std_ss [GSYM APPEND_ASSOC,APPEND]
     \\ SIMP_TAC std_ss [EL_LENGTH,DECIDE ``n+1+1+1-3 = n:num``])
   \\ FULL_SIMP_TAC std_ss []
-  \\ ASSUME_TAC (x64_div_guess_thm |> GEN_ALL)
+  \\ ASSUME_TAC (mc_div_guess_thm |> GEN_ALL)
   \\ `dimword (:α) + 1 ≤ l` by
         (fs [LENGTH_APPEND,LEFT_ADD_DISTRIB] \\ NO_TAC)
-  \\ SEP_I_TAC "x64_div_guess" \\ FULL_SIMP_TAC std_ss []
+  \\ SEP_I_TAC "mc_div_guess" \\ FULL_SIMP_TAC std_ss []
   \\ REV_FULL_SIMP_TAC std_ss []
   \\ POP_ASSUM (MP_TAC o Q.SPECL [`REVERSE (FRONT (FRONT ys1))`,
       `REVERSE (FRONT (FRONT (FRONT (x::zs))))`])
@@ -2542,12 +2542,12 @@ val x64_div_loop_thm = prove(
   \\ NTAC 2 (qpat_x_assum `_ <= _` mp_tac)
   \\ NTAC 6 (POP_ASSUM (K ALL_TAC))
   \\ rpt strip_tac
-  \\ ASSUME_TAC (GEN_ALL x64_div_adjust_thm)
-  \\ SEP_I_TAC "x64_div_adjust" \\ POP_ASSUM MP_TAC
+  \\ ASSUME_TAC (GEN_ALL mc_div_adjust_thm)
+  \\ SEP_I_TAC "mc_div_adjust" \\ POP_ASSUM MP_TAC
   \\ MATCH_MP_TAC IMP_IMP \\ STRIP_TAC THEN1 (fs [])
   \\ STRIP_TAC \\ ASM_SIMP_TAC std_ss [word_add_n2w,word_arith_lemma2]
-  \\ ASSUME_TAC (GEN_ALL x64_div_sub_loop_thm)
-  \\ SEP_I_TAC "x64_div_sub_loop" \\ POP_ASSUM MP_TAC
+  \\ ASSUME_TAC (GEN_ALL mc_div_sub_loop_thm)
+  \\ SEP_I_TAC "mc_div_sub_loop" \\ POP_ASSUM MP_TAC
   \\ MATCH_MP_TAC IMP_IMP \\ STRIP_TAC
   THEN1 (fs [LEFT_ADD_DISTRIB,RIGHT_ADD_DISTRIB])
   \\ STRIP_TAC \\ ASM_SIMP_TAC std_ss [word_add_n2w,word_arith_lemma2]
@@ -2573,7 +2573,7 @@ val x64_div_loop_thm = prove(
   \\ FULL_SIMP_TAC std_ss []
   \\ SIMP_TAC std_ss [SNOC_APPEND,GSYM APPEND_ASSOC,APPEND]
   \\ FULL_SIMP_TAC std_ss [APPEND_ASSOC,APPEND]
-  \\ SEP_I_TAC "x64_div_loop" \\ POP_ASSUM MP_TAC
+  \\ SEP_I_TAC "mc_div_loop" \\ POP_ASSUM MP_TAC
   \\ MATCH_MP_TAC IMP_IMP \\ STRIP_TAC THEN1
    (`(LENGTH (FRONT sub) = LENGTH ys)` by ALL_TAC THEN1
       (Q.UNABBREV_TAC `sub`
@@ -2595,9 +2595,9 @@ val x64_div_loop_thm = prove(
 
 (* mw_div -- mul_by_single *)
 
-val (x64_mul_by_single_def, _,
-     x64_mul_by_single_pre_def, _) =
-  tailrec_define "x64_mul_by_single" ``
+val (mc_mul_by_single_def, _,
+     mc_mul_by_single_pre_def, _) =
+  tailrec_define "mc_mul_by_single" ``
     (\(l,r1,r8,r9,r10,r11,xs,zs).
       if r9 = r11 then
         (let cond = w2n r10 < LENGTH zs in
@@ -2610,8 +2610,8 @@ val (x64_mul_by_single_def, _,
          let r2 = EL (w2n r11) xs in
          let r0 = r8 in
          let r3 = 0x0w in
-         let cond = cond /\ x64_single_mul_add_pre (r0,r1,r2,r3) in
-         let (r0,r1,r2,r3) = x64_single_mul_add (r0,r1,r2,r3) in
+         let cond = cond /\ mc_single_mul_add_pre (r0,r1,r2,r3) in
+         let (r0,r1,r2,r3) = mc_single_mul_add (r0,r1,r2,r3) in
          let cond = cond /\ w2n r10 < LENGTH zs in
          let zs = LUPDATE r0 (w2n r10) zs in
          let r1 = r2 in
@@ -2624,27 +2624,27 @@ val (x64_mul_by_single_def, _,
      word # 'a word # 'a word list # 'a word list + num # 'a word # 'a
      word # 'a word # 'a word # 'a word list # 'a word list) # bool``;
 
-val x64_mul_by_single_thm = prove(
+val mc_mul_by_single_thm = prove(
   ``!(xs:'a word list) xs1 x zs k zs1 zs2 z2 l.
       LENGTH (xs1++xs) < dimword (:'a) /\ (LENGTH zs = LENGTH xs) /\
       LENGTH (zs1++zs) < dimword (:'a) /\ LENGTH xs <= l ==>
       ?r1 l2.
-        x64_mul_by_single_pre (l,k,x,n2w (LENGTH (xs1++xs)),n2w (LENGTH zs1),
+        mc_mul_by_single_pre (l,k,x,n2w (LENGTH (xs1++xs)),n2w (LENGTH zs1),
                           n2w (LENGTH xs1),xs1++xs,zs1++zs++z2::zs2) /\
-        (x64_mul_by_single (l,k,x,n2w (LENGTH (xs1++xs)),n2w (LENGTH zs1),
+        (mc_mul_by_single (l,k,x,n2w (LENGTH (xs1++xs)),n2w (LENGTH zs1),
                        n2w (LENGTH xs1),xs1++xs,zs1++zs++z2::zs2) =
            (l2,r1,x,n2w (LENGTH (xs1++xs)),n2w (LENGTH (zs1++zs)+1),xs1++xs,
             zs1++(mw_mul_pass x xs (MAP (K 0w) xs) k)++zs2)) /\
         l <= l2 + LENGTH xs``,
   Induct \\ Cases_on `zs`
   \\ FULL_SIMP_TAC std_ss [LENGTH,APPEND_NIL,mw_mul_pass_def,ADD1]
-  \\ ONCE_REWRITE_TAC [x64_mul_by_single_def,x64_mul_by_single_pre_def]
+  \\ ONCE_REWRITE_TAC [mc_mul_by_single_def,mc_mul_by_single_pre_def]
   \\ FULL_SIMP_TAC std_ss [LET_DEF,n2w_11,w2n_n2w,LUPDATE_LENGTH]
   \\ FULL_SIMP_TAC std_ss [GSYM APPEND_ASSOC,APPEND,word_add_n2w,LENGTH_APPEND]
   \\ FULL_SIMP_TAC std_ss [LENGTH,MAP,HD,TL]
   \\ REPEAT STRIP_TAC
   \\ IMP_RES_TAC (DECIDE ``m+n<k ==> m < k /\ n<k:num``)
-  \\ FULL_SIMP_TAC std_ss [ADD1,x64_single_mul_add_thm]
+  \\ FULL_SIMP_TAC std_ss [ADD1,mc_single_mul_add_thm]
   \\ FULL_SIMP_TAC std_ss [rich_listTheory.EL_LENGTH_APPEND,LUPDATE_LENGTH,NULL,HD]
   \\ Cases_on `single_mul_add x h' k 0w` \\ FULL_SIMP_TAC std_ss [LET_DEF,TL]
   \\ ONCE_REWRITE_TAC [SNOC_INTRO |> Q.INST [`xs2`|->`[]`] |> REWRITE_RULE [APPEND_NIL]]
@@ -2653,7 +2653,7 @@ val x64_mul_by_single_thm = prove(
       ((LENGTH zs1 + 1) = LENGTH (SNOC q zs1))` by ALL_TAC
   THEN1 (FULL_SIMP_TAC std_ss [LENGTH_SNOC] \\ DECIDE_TAC)
   \\ FULL_SIMP_TAC std_ss []
-  \\ SEP_I_TAC "x64_mul_by_single" \\ POP_ASSUM MP_TAC
+  \\ SEP_I_TAC "mc_mul_by_single" \\ POP_ASSUM MP_TAC
   \\ MATCH_MP_TAC IMP_IMP \\ STRIP_TAC
   THEN1 (fs [])
   \\ REPEAT STRIP_TAC \\ FULL_SIMP_TAC std_ss []
@@ -2665,9 +2665,9 @@ val x64_mul_by_single_thm = prove(
 
 (* mw_div -- mul_by_single, top two from ys *)
 
-val (x64_top_two_def, _,
-     x64_top_two_pre_def, _) =
-  tailrec_define "x64_top_two" ``
+val (mc_top_two_def, _,
+     mc_top_two_pre_def, _) =
+  tailrec_define "mc_top_two" ``
     (\(l,r0,r1,r3,r8,r9,r11,ys).
       if r9 = r11 then (let r1 = r3 in (INR (l,r0,r1,r8,r9,r11,ys),T))
       else
@@ -2675,8 +2675,8 @@ val (x64_top_two_def, _,
          let cond = w2n r11 < LENGTH ys in
          let r2 = EL (w2n r11) ys in
          let r0 = r8 in
-         let cond = cond /\ x64_single_mul_pre (r0,r1,r2) in
-         let (r0,r1,r2) = x64_single_mul (r0,r1,r2) in
+         let cond = cond /\ mc_single_mul_pre (r0,r1,r2) in
+         let (r0,r1,r2) = mc_single_mul (r0,r1,r2) in
          let r1 = r2 in
          let r11 = r11 + 0x1w
          in
@@ -2686,34 +2686,34 @@ val (x64_top_two_def, _,
      word # 'a word # 'a word list + num # 'a word # 'a word # 'a word
      # 'a word # 'a word # 'a word list) # bool``;
 
-val x64_top_two_thm = prove(
+val mc_top_two_thm = prove(
   ``!(ys:'a word list) x k1 k2 k3 ys1 l.
       LENGTH (ys1 ++ ys) < dimword (:'a) /\ LENGTH ys <= l ==>
       ?l2.
-        x64_top_two_pre (l,k2,k1,k3,
+        mc_top_two_pre (l,k2,k1,k3,
                          x,n2w (LENGTH (ys1++ys)),n2w (LENGTH ys1),ys1++ys) /\
-        (x64_top_two (l,k2,k1,k3,
+        (mc_top_two (l,k2,k1,k3,
                       x,n2w (LENGTH (ys1++ys)),n2w (LENGTH ys1),ys1++ys) =
                  (l2,FST (SND (mw_mul_pass_top x ys (k1,k2,k3))),
                   SND (SND (mw_mul_pass_top x ys (k1,k2,k3))),x,
                   n2w (LENGTH (ys1++ys)),n2w (LENGTH (ys1++ys)),ys1++ys)) /\
         l <= l2 + LENGTH ys``,
   Induct \\ FULL_SIMP_TAC std_ss [APPEND,APPEND_NIL]
-  \\ ONCE_REWRITE_TAC [x64_top_two_def,x64_top_two_pre_def]
+  \\ ONCE_REWRITE_TAC [mc_top_two_def,mc_top_two_pre_def]
   \\ FULL_SIMP_TAC std_ss [LET_DEF,n2w_11,mw_mul_pass_top_def]
   \\ rpt STRIP_TAC
   \\ `LENGTH ys1 < dimword (:'a) /\
       LENGTH (ys1 ++ h::ys) <> LENGTH ys1` by
         (FULL_SIMP_TAC std_ss [LENGTH_APPEND,LENGTH] \\ DECIDE_TAC)
   \\ FULL_SIMP_TAC std_ss [w2n_n2w,EL_LENGTH]
-  \\ FULL_SIMP_TAC std_ss [x64_single_mul_thm]
+  \\ FULL_SIMP_TAC std_ss [mc_single_mul_thm]
   \\ Cases_on `single_mul_add x h k1 0w`
   \\ FULL_SIMP_TAC std_ss [LET_DEF,SNOC_INTRO]
   \\ `(LENGTH ys1 + 1) = (LENGTH (SNOC h ys1))` by ALL_TAC THEN1
        FULL_SIMP_TAC (srw_ss()) [word_add_n2w,ADD1]
   \\ FULL_SIMP_TAC std_ss [word_add_n2w]
   \\ `LENGTH ys <= l-1` by fs []
-  \\ res_tac \\ SEP_I_TAC "x64_top_two"
+  \\ res_tac \\ SEP_I_TAC "mc_top_two"
   \\ rfs [])
   |> Q.SPECL [`ys`,`x`,`0w`,`0w`,`0w`,`[]`] |> DISCH ``1 < LENGTH (ys:'a word list)``
   |> SIMP_RULE std_ss [APPEND_NIL,APPEND,LENGTH,mw_mul_pass_top_thm]
@@ -2721,9 +2721,9 @@ val x64_top_two_thm = prove(
 
 (* mw_div -- copy result down *)
 
-val (x64_copy_down_def, _,
-     x64_copy_down_pre_def, _) =
-  tailrec_define "x64_copy_down" ``
+val (mc_copy_down_def, _,
+     mc_copy_down_pre_def, _) =
+  tailrec_define "mc_copy_down" ``
     (\(l,r8,r10,r11,zs).
       if r8 = 0x0w then (INR (l,zs),T)
       else
@@ -2739,19 +2739,19 @@ val (x64_copy_down_def, _,
     :num # 'a word # 'a word # 'a word # 'a word list -> (num # 'a
     word # 'a word # 'a word # 'a word list + num # 'a word list) # bool``;
 
-val x64_copy_down_thm = prove(
+val mc_copy_down_thm = prove(
   ``!(zs0:'a word list) zs1 zs2 zs3 l.
       LENGTH (zs0 ++ zs1 ++ zs2) < dimword (:'a) /\ zs1 <> [] /\
       LENGTH zs2 <= l ==>
       ?zs4 l2.
-        x64_copy_down_pre (l,n2w (LENGTH zs2),
+        mc_copy_down_pre (l,n2w (LENGTH zs2),
           n2w (LENGTH (zs0 ++ zs1)),n2w (LENGTH zs0),zs0 ++ zs1 ++ zs2 ++ zs3) /\
-        (x64_copy_down (l,n2w (LENGTH zs2),
+        (mc_copy_down (l,n2w (LENGTH zs2),
           n2w (LENGTH (zs0 ++ zs1)),n2w (LENGTH zs0),zs0 ++ zs1 ++ zs2 ++ zs3) =
            (l2,zs0 ++ zs2 ++ zs4)) /\ (LENGTH zs4 = LENGTH zs1 + LENGTH zs3) /\
         l <= l2 + LENGTH zs2``,
   Induct_on `zs2`
-  \\ ONCE_REWRITE_TAC [x64_copy_down_def,x64_copy_down_pre_def]
+  \\ ONCE_REWRITE_TAC [mc_copy_down_def,mc_copy_down_pre_def]
   \\ FULL_SIMP_TAC std_ss [LENGTH,APPEND_NIL]
   \\ FULL_SIMP_TAC std_ss [APPEND_11,GSYM APPEND_ASSOC,LENGTH_APPEND]
   \\ REPEAT STRIP_TAC
@@ -2780,9 +2780,9 @@ val x64_copy_down_thm = prove(
 
 (* mw_div -- copy xs into zs *)
 
-val (x64_copy_over_def, _,
-     x64_copy_over_pre_def, _) =
-  tailrec_define "x64_copy_over" ``
+val (mc_copy_over_def, _,
+     mc_copy_over_pre_def, _) =
+  tailrec_define "mc_copy_over" ``
     (\(l,r10,xs,zs).
       if r10 = 0x0w then (INR (l,xs,zs),T)
       else
@@ -2796,41 +2796,41 @@ val (x64_copy_over_def, _,
     :num # 'a word # 'a word list # 'a word list -> (num # 'a word #
     'a word list # 'a word list + num # 'a word list # 'a word list) # bool``;
 
-val x64_copy_over_thm = prove(
+val mc_copy_over_thm = prove(
   ``!(xs0:'a word list) zs0 xs zs l.
       (LENGTH zs0 = LENGTH xs0) /\
       LENGTH (zs0++zs) < dimword (:'a) /\
       LENGTH xs0 <= l ==>
       ?l2.
-        x64_copy_over_pre (l,n2w (LENGTH xs0),xs0 ++ xs,zs0 ++ zs) /\
-        (x64_copy_over (l,n2w (LENGTH xs0),xs0 ++ xs,zs0 ++ zs) =
+        mc_copy_over_pre (l,n2w (LENGTH xs0),xs0 ++ xs,zs0 ++ zs) /\
+        (mc_copy_over (l,n2w (LENGTH xs0),xs0 ++ xs,zs0 ++ zs) =
            (l2,xs0 ++ xs,xs0 ++ zs)) /\
         l <= l2 + LENGTH xs0``,
   HO_MATCH_MP_TAC SNOC_INDUCT \\ STRIP_TAC THEN1
-   (ONCE_REWRITE_TAC [x64_copy_over_def,x64_copy_over_pre_def]
+   (ONCE_REWRITE_TAC [mc_copy_over_def,mc_copy_over_pre_def]
     \\ SIMP_TAC std_ss [LENGTH,LENGTH_NIL,APPEND])
   \\ rpt STRIP_TAC
   \\ `(zs0 = []) \/ ?x l. zs0 = SNOC x l` by METIS_TAC [SNOC_CASES]
   \\ FULL_SIMP_TAC std_ss [LENGTH,ADD1,LENGTH_SNOC]
   \\ `LENGTH xs0 + 1 < dimword (:'a) /\ LENGTH xs0 < dimword (:'a)` by ALL_TAC
   THEN1 (FULL_SIMP_TAC std_ss [LENGTH_SNOC,LENGTH_APPEND] \\ DECIDE_TAC)
-  \\ ONCE_REWRITE_TAC [x64_copy_over_def,x64_copy_over_pre_def]
+  \\ ONCE_REWRITE_TAC [mc_copy_over_def,mc_copy_over_pre_def]
   \\ FULL_SIMP_TAC std_ss [n2w_11,ZERO_LT_dimword]
   \\ FULL_SIMP_TAC std_ss [GSYM word_add_n2w,WORD_ADD_SUB,LET_DEF]
   \\ FULL_SIMP_TAC std_ss [w2n_n2w,EL_LENGTH,SNOC_APPEND]
   \\ Q.PAT_X_ASSUM `LENGTH l' = LENGTH xs0` (ASSUME_TAC o GSYM)
   \\ ASM_SIMP_TAC std_ss [LUPDATE_LENGTH,APPEND,GSYM APPEND_ASSOC]
   \\ FULL_SIMP_TAC std_ss [LENGTH,LENGTH_APPEND]
-  \\ SEP_I_TAC "x64_copy_over"
+  \\ SEP_I_TAC "mc_copy_over"
   \\ pop_assum mp_tac
   \\ match_mp_tac IMP_IMP \\ conj_tac THEN1 fs []
   \\ strip_tac \\ fs [])
 
 (* mw_div -- top-level function *)
 
-val (x64_div_def, _,
-     x64_div_pre_def, _) =
-  tailrec_define "x64_div" ``
+val (mc_div_def, _,
+     mc_div_pre_def, _) =
+  tailrec_define "mc_div" ``
     (\(l,r0,r1,r3,xs,ys,zs).
       if r0 <+ r1 then
         (let r6 = r0
@@ -2841,11 +2841,11 @@ val (x64_div_def, _,
              (let r11 = r0 in
               let r10 = r1 in
               let r0 = 0x0w in
-              let cond = x64_mul_zero_pre (l-1,r0,r10,zs) /\ l <> 0 in
-              let (l,r10,zs) = x64_mul_zero (l-1,r0,r10,zs) in
+              let cond = mc_mul_zero_pre (l-1,r0,r10,zs) /\ l <> 0 in
+              let (l,r10,zs) = mc_mul_zero (l-1,r0,r10,zs) in
               let r10 = r11 in
-              let cond = cond /\ x64_copy_over_pre (l-1,r10,xs,zs) /\ l <> 0 in
-              let (l,xs,zs) = x64_copy_over (l-1,r10,xs,zs) in
+              let cond = cond /\ mc_copy_over_pre (l-1,r10,xs,zs) /\ l <> 0 in
+              let (l,xs,zs) = mc_copy_over (l-1,r10,xs,zs) in
               let r0 = r1
               in
                 (INR (l,r0,r3,r6,xs,ys,zs),cond)))
@@ -2857,8 +2857,8 @@ val (x64_div_def, _,
          let r9 = EL (w2n r10) ys in
          let r10 = r0 in
          let r8 = r0 in
-         let cond = cond /\ x64_simple_div_pre (l-1,r2,r9,r10,xs,zs) /\ l <> 0 in
-         let (l,r2,r9,r10,xs,zs) = x64_simple_div (l-1,r2,r9,r10,xs,zs) in
+         let cond = cond /\ mc_simple_div_pre (l-1,r2,r9,r10,xs,zs) /\ l <> 0 in
+         let (l,r2,r9,r10,xs,zs) = mc_simple_div (l-1,r2,r9,r10,xs,zs) in
          let r6 = 0x0w in
          let r0 = r8 in
          let r3 = r14
@@ -2884,16 +2884,16 @@ val (x64_div_def, _,
          let cond = w2n r10 < LENGTH ys in
          let r1 = EL (w2n r10) ys in
          let r2 = 0x1w in
-         let cond = cond /\ x64_calc_d_pre (l-1,r1,r2) /\ l <> 0 in
-         let (l,r2) = x64_calc_d (l-1,r1,r2) in
+         let cond = cond /\ mc_calc_d_pre (l-1,r1,r2) /\ l <> 0 in
+         let (l,r2) = mc_calc_d (l-1,r1,r2) in
          let r1 = 0x0w in
          let r8 = r2 in
          let r10 = r1 in
          let r11 = r1 in
-         let cond = cond /\ x64_mul_by_single_pre (l-1,r1,r8,r9,r10,r11,xs,zs) /\ l<>0
+         let cond = cond /\ mc_mul_by_single_pre (l-1,r1,r8,r9,r10,r11,xs,zs) /\ l<>0
          in
          let (l,r1,r8,r9,r10,xs,zs) =
-               x64_mul_by_single (l-1,r1,r8,r9,r10,r11,xs,zs)
+               mc_mul_by_single (l-1,r1,r8,r9,r10,r11,xs,zs)
          in
          let r1 = 0x0w in
          let cond = cond /\ w2n r10 < LENGTH zs in
@@ -2903,8 +2903,8 @@ val (x64_div_def, _,
          let r3 = r0 in
          let r11 = r0 in
          let r9 = r7 in
-         let cond = cond /\ x64_top_two_pre (l-1,r0,r1,r3,r8,r9,r11,ys) /\ l <> 0 in
-         let (l,r0,r1,r8,r9,r11,ys) = x64_top_two (l-1,r0,r1,r3,r8,r9,r11,ys) in
+         let cond = cond /\ mc_top_two_pre (l-1,r0,r1,r3,r8,r9,r11,ys) /\ l <> 0 in
+         let (l,r0,r1,r8,r9,r11,ys) = mc_top_two (l-1,r0,r1,r3,r8,r9,r11,ys) in
          let r7 = r8 in
          let r11 = r9 in
          let r10 = r19 in
@@ -2913,22 +2913,22 @@ val (x64_div_def, _,
          let r14 = r0 in
          let r15 = r1 in
          let r17 = r10 in
-         let cond = cond /\ x64_div_loop_pre (l-1,r7,r9,r10,r11,r14,r15,ys,zs) /\ l<>0 in
+         let cond = cond /\ mc_div_loop_pre (l-1,r7,r9,r10,r11,r14,r15,ys,zs) /\ l<>0 in
          let (l,r7,r9,r10,r11,r14,r15,ys,zs) =
-               x64_div_loop (l-1,r7,r9,r10,r11,r14,r15,ys,zs)
+               mc_div_loop (l-1,r7,r9,r10,r11,r14,r15,ys,zs)
          in
          let r8 = r17 in
          let r11 = r9 in
          let r10 = r9 in
          let r9 = r7 in
          let r2 = 0x0w in
-         let cond = cond /\ x64_simple_div1_pre (l-1,r2,r9,r10,zs) /\ l <> 0 in
-         let (l,r2,r9,r10,zs) = x64_simple_div1 (l-1,r2,r9,r10,zs) in
+         let cond = cond /\ mc_simple_div1_pre (l-1,r2,r9,r10,zs) /\ l <> 0 in
+         let (l,r2,r9,r10,zs) = mc_simple_div1 (l-1,r2,r9,r10,zs) in
          let r9 = r11 in
          let r10 = r9 in
          let r7 = r8 in
-         let cond = cond /\ x64_fix_pre (l-1,r8,r10,zs) /\ l <> 0 in
-         let (l,r8,r10,zs) = x64_fix (l-1,r8,r10,zs) in
+         let cond = cond /\ mc_fix_pre (l-1,r8,r10,zs) /\ l <> 0 in
+         let (l,r8,r10,zs) = mc_fix (l-1,r8,r10,zs) in
          let r6 = r10 in
          let r10 = r9 in
          let r3 = r18 in
@@ -2936,8 +2936,8 @@ val (x64_div_def, _,
          in
            if r3 = 0x0w then
              (let r11 = 0x0w in
-              let cond = cond /\ x64_copy_down_pre (l-1,r8,r10,r11,zs) /\ l<>0 in
-              let (l,zs) = x64_copy_down (l-1,r8,r10,r11,zs) in
+              let cond = cond /\ mc_copy_down_pre (l-1,r8,r10,r11,zs) /\ l<>0 in
+              let (l,zs) = mc_copy_down (l-1,r8,r10,r11,zs) in
               let r0 = r7
               in
                 (INR (l,r0,r3,r6,xs,ys,zs),cond))
@@ -2960,26 +2960,26 @@ val MAP_K_0 = prove(
   ``!xs. MAP (\x. 0x0w) xs = REPLICATE (LENGTH xs) 0x0w``,
   Induct \\ SRW_TAC [] [REPLICATE]);
 
-val x64_div_max_def = Define `
-  x64_div_max (xs:'a word list) (ys:'a word list) (zs:'a word list) =
+val mc_div_max_def = Define `
+  mc_div_max (xs:'a word list) (ys:'a word list) (zs:'a word list) =
     2 * LENGTH ys + 2 * LENGTH zs + 5 + dimindex (:α) +
     LENGTH xs * (dimword (:α) + 2 * LENGTH ys + 4)`;
 
-val x64_div_thm = prove(
+val mc_div_thm = prove(
   ``(ys:'a word list) <> [] /\ mw_ok xs /\ mw_ok ys /\
     LENGTH xs + LENGTH ys <= LENGTH zs /\
     LENGTH zs < dimword (:'a) /\ ((res,mod,T) = mw_div xs ys) /\
-    x64_div_max xs ys zs <= l ==>
+    mc_div_max xs ys zs <= l ==>
     ?zs2 l2.
-      x64_div_pre (l,n2w (LENGTH xs),n2w (LENGTH ys),r3,xs,ys,zs) /\
-      (x64_div (l,n2w (LENGTH xs),n2w (LENGTH ys),r3,xs,ys,zs) =
+      mc_div_pre (l,n2w (LENGTH xs),n2w (LENGTH ys),r3,xs,ys,zs) /\
+      (mc_div (l,n2w (LENGTH xs),n2w (LENGTH ys),r3,xs,ys,zs) =
          (l2,n2w (LENGTH (if r3 = 0w then res else mod)),r3,
           n2w (LENGTH (mw_fix mod)),xs,ys,
           (if r3 = 0w then res else mod) ++ zs2)) /\
       (LENGTH zs = LENGTH ((if r3 = 0w then res else mod) ++ zs2)) /\
       ((r3 = 0w) ==> LENGTH zs2 <> 0) /\ LENGTH (mw_fix mod) < dimword (:'a) /\
-      l <= l2 + x64_div_max xs ys zs``,
-  REWRITE_TAC [x64_div_max_def]
+      l <= l2 + mc_div_max xs ys zs``,
+  REWRITE_TAC [mc_div_max_def]
   \\ SIMP_TAC std_ss [mw_div_def,LET_DEF] \\ STRIP_TAC
   \\ `LENGTH xs < dimword (:'a) /\ LENGTH ys < dimword (:'a)` by DECIDE_TAC
   \\ IMP_RES_TAC mw_ok_mw_fix_ID \\ FULL_SIMP_TAC std_ss []
@@ -2988,30 +2988,30 @@ val x64_div_thm = prove(
    (Cases_on `r3 = 0w` \\ FULL_SIMP_TAC std_ss [] THEN1
      (Q.EXISTS_TAC `zs`
       \\ FULL_SIMP_TAC std_ss [LENGTH,LENGTH_APPEND,APPEND]
-      \\ ASM_SIMP_TAC std_ss [x64_div_def,x64_div_pre_def,LET_DEF,WORD_LO,
+      \\ ASM_SIMP_TAC std_ss [mc_div_def,mc_div_pre_def,LET_DEF,WORD_LO,
            w2n_n2w, mw_ok_mw_fix_ID,n2w_11,ZERO_LT_dimword,LENGTH_NIL,
            mw_fix_REPLICATE] \\ FULL_SIMP_TAC std_ss [LENGTH,GSYM LENGTH_NIL]
       \\ DECIDE_TAC)
-    \\ ASM_SIMP_TAC std_ss [x64_div_def,x64_div_pre_def,LET_DEF,WORD_LO,
+    \\ ASM_SIMP_TAC std_ss [mc_div_def,mc_div_pre_def,LET_DEF,WORD_LO,
            w2n_n2w, mw_ok_mw_fix_ID,n2w_11,ZERO_LT_dimword,LENGTH_NIL]
     \\ `?zs1 zs2. (zs = zs1 ++ zs2) /\ (LENGTH zs1 = LENGTH ys)` by ALL_TAC
     THEN1 (MATCH_MP_TAC LESS_EQ_LENGTH \\ DECIDE_TAC)
     \\ POP_ASSUM (ASSUME_TAC o GSYM)
     \\ FULL_SIMP_TAC std_ss []
     \\ `LENGTH zs1 ≤ l − 1` by fs []
-    \\ ASSUME_TAC x64_mul_zero_thm \\ SEP_I_TAC "x64_mul_zero"
+    \\ ASSUME_TAC mc_mul_zero_thm \\ SEP_I_TAC "mc_mul_zero"
     \\ POP_ASSUM MP_TAC \\ FULL_SIMP_TAC std_ss []
     \\ STRIP_TAC \\ FULL_SIMP_TAC std_ss []
     \\ `?zs3 zs4. (zs1 = zs3 ++ zs4) /\ (LENGTH zs3 = LENGTH xs)` by ALL_TAC
     THEN1 (MATCH_MP_TAC LESS_EQ_LENGTH \\ DECIDE_TAC)
     \\ FULL_SIMP_TAC std_ss [MAP_APPEND,GSYM APPEND_ASSOC]
-    \\ ASSUME_TAC (x64_copy_over_thm |>
+    \\ ASSUME_TAC (mc_copy_over_thm |>
           Q.SPECL [`xs`,`MAP (\x.0w) (zs3:'a word list)`,`[]`,
                    `MAP (\x.0w) (zs4:'a word list) ++ zs2`,
                    `l − 1 − LENGTH (xs ++ zs4:'a word list)-1`]
           |> SIMP_RULE std_ss [LENGTH_MAP,APPEND_NIL,LENGTH_APPEND] |> GEN_ALL)
     \\ FULL_SIMP_TAC std_ss [LENGTH_APPEND,MAP_APPEND,APPEND_ASSOC]
-    \\ SEP_I_TAC "x64_copy_over" \\ POP_ASSUM MP_TAC
+    \\ SEP_I_TAC "mc_copy_over" \\ POP_ASSUM MP_TAC
     \\ MATCH_MP_TAC IMP_IMP \\ STRIP_TAC
     THEN1 (fs [])
     \\ STRIP_TAC \\ FULL_SIMP_TAC std_ss []
@@ -3025,13 +3025,13 @@ val x64_div_thm = prove(
    (`?qs r c. mw_simple_div 0x0w (REVERSE xs) (HD ys) = (qs,r,c)` by METIS_TAC [PAIR]
     \\ FULL_SIMP_TAC std_ss [LENGTH_REVERSE]
     \\ `0 < dimword (:'a)` by DECIDE_TAC
-    \\ ASM_SIMP_TAC std_ss [x64_div_def,x64_div_pre_def,LET_DEF,WORD_LO,w2n_n2w,EL]
+    \\ ASM_SIMP_TAC std_ss [mc_div_def,mc_div_pre_def,LET_DEF,WORD_LO,w2n_n2w,EL]
     \\ `?zs1 zs2. (zs = zs1 ++ zs2) /\ (LENGTH zs1 = LENGTH xs)` by
          (MATCH_MP_TAC LESS_EQ_LENGTH \\ DECIDE_TAC)
     \\ FULL_SIMP_TAC std_ss []
-    \\ ASSUME_TAC (x64_simple_div_thm |> Q.SPECL [`xs`,`[]`] |> GEN_ALL
+    \\ ASSUME_TAC (mc_simple_div_thm |> Q.SPECL [`xs`,`[]`] |> GEN_ALL
         |> SIMP_RULE std_ss [APPEND_NIL])
-    \\ SEP_I_TAC "x64_simple_div" \\ POP_ASSUM MP_TAC
+    \\ SEP_I_TAC "mc_simple_div" \\ POP_ASSUM MP_TAC
     \\ `LENGTH xs ≤ l − 1` by fs []
     \\ FULL_SIMP_TAC std_ss [] \\ STRIP_TAC
     \\ `(LENGTH xs) = (LENGTH qs)` by
@@ -3066,15 +3066,15 @@ val x64_div_thm = prove(
   \\ `LENGTH ys <> 0` by FULL_SIMP_TAC std_ss [LENGTH_NIL]
   \\ `0 < dimword (:'a) /\ LENGTH ys - 1 < dimword (:'a)` by DECIDE_TAC
   \\ `1 < dimword (:'a) /\ ~(LENGTH ys < 1) /\ 0 < LENGTH ys` by DECIDE_TAC
-  \\ ASM_SIMP_TAC std_ss [x64_div_def,x64_div_pre_def,LET_DEF,WORD_LO,
+  \\ ASM_SIMP_TAC std_ss [mc_div_def,mc_div_pre_def,LET_DEF,WORD_LO,
        w2n_n2w,n2w_11,word_arith_lemma2]
   \\ `(LAST ys <> 0w) /\ (EL (LENGTH ys - 1) ys = LAST ys)` by ALL_TAC THEN1
    (FULL_SIMP_TAC std_ss [mw_ok_def]
     \\ `(ys = []) \/ ?y ys2. ys = SNOC y ys2` by METIS_TAC [SNOC_CASES]
     \\ FULL_SIMP_TAC std_ss [LENGTH_SNOC,LAST_SNOC]
     \\ FULL_SIMP_TAC std_ss [EL_LENGTH,SNOC_APPEND])
-  \\ assume_tac x64_calc_d_thm
-  \\ SEP_I_TAC "x64_calc_d"
+  \\ assume_tac mc_calc_d_thm
+  \\ SEP_I_TAC "mc_calc_d"
   \\ pop_assum mp_tac
   \\ match_mp_tac IMP_IMP
   \\ conj_tac THEN1 (fs [] \\ Cases_on `LAST ys` \\ fs [])
@@ -3084,8 +3084,8 @@ val x64_div_thm = prove(
   \\ FULL_SIMP_TAC std_ss []
   \\ Cases_on `zs2` \\ FULL_SIMP_TAC std_ss [LENGTH,LENGTH_APPEND]
   THEN1 (`F` by DECIDE_TAC)
-  \\ ASSUME_TAC x64_mul_by_single_thm
-  \\ SEP_I_TAC "x64_mul_by_single"
+  \\ ASSUME_TAC mc_mul_by_single_thm
+  \\ SEP_I_TAC "mc_mul_by_single"
   \\ POP_ASSUM MP_TAC
   \\ match_mp_tac IMP_IMP
   \\ conj_tac THEN1 fs []
@@ -3104,8 +3104,8 @@ val x64_div_thm = prove(
     \\ Q.UNABBREV_TAC `xs1`
     \\ FULL_SIMP_TAC std_ss [GSYM APPEND_ASSOC, APPEND])
   \\ FULL_SIMP_TAC std_ss [] \\ POP_ASSUM (K ALL_TAC)
-  \\ (x64_top_two_thm |> GEN_ALL |> MP_CANON |> ASSUME_TAC)
-  \\ SEP_I_TAC "x64_top_two" \\ POP_ASSUM MP_TAC
+  \\ (mc_top_two_thm |> GEN_ALL |> MP_CANON |> ASSUME_TAC)
+  \\ SEP_I_TAC "mc_top_two" \\ POP_ASSUM MP_TAC
   \\ MATCH_MP_TAC IMP_IMP \\ STRIP_TAC THEN1 fs []
   \\ STRIP_TAC \\ FULL_SIMP_TAC std_ss []
   \\ FULL_SIMP_TAC std_ss [HD,TL]
@@ -3125,13 +3125,13 @@ val x64_div_thm = prove(
   \\ POP_ASSUM (ASSUME_TAC o GSYM) \\ FULL_SIMP_TAC std_ss [LENGTH_APPEND]
   \\ FULL_SIMP_TAC std_ss [BUTLASTN_LENGTH_APPEND,LASTN_LENGTH_APPEND]
   \\ POP_ASSUM (ASSUME_TAC o GSYM) \\ FULL_SIMP_TAC std_ss [LENGTH_APPEND]
-  \\ ASSUME_TAC (x64_div_loop_thm |> SIMP_RULE std_ss [LET_DEF] |> GEN_ALL)
+  \\ ASSUME_TAC (mc_div_loop_thm |> SIMP_RULE std_ss [LET_DEF] |> GEN_ALL)
   \\ `-1w * n2w (LENGTH ys) + n2w (LENGTH xs) + 2w =
       n2w (LENGTH ts1):'a word` by
          (qpat_x_assum `_ = n2w (LENGTH ts1)` (assume_tac o GSYM)
           \\ full_simp_tac std_ss [WORD_SUB_INTRO] \\ NO_TAC)
   \\ FULL_SIMP_TAC std_ss []
-  \\ SEP_I_TAC "x64_div_loop" \\ POP_ASSUM MP_TAC
+  \\ SEP_I_TAC "mc_div_loop" \\ POP_ASSUM MP_TAC
   \\ MATCH_MP_TAC IMP_IMP \\ STRIP_TAC THEN1
    (FULL_SIMP_TAC std_ss [LENGTH_APPEND] \\ fs []
     \\ rpt conj_tac \\ unabbrev_all_tac
@@ -3153,8 +3153,8 @@ val x64_div_thm = prove(
   \\ FULL_SIMP_TAC std_ss []
   \\ Q.PAT_X_ASSUM `LENGTH rs1 = LENGTH ys` (ASSUME_TAC o GSYM)
   \\ FULL_SIMP_TAC std_ss [GSYM APPEND_ASSOC]
-  \\ ASSUME_TAC x64_simple_div1_thm
-  \\ SEP_I_TAC "x64_simple_div1" \\ POP_ASSUM MP_TAC
+  \\ ASSUME_TAC mc_simple_div1_thm
+  \\ SEP_I_TAC "mc_simple_div1" \\ POP_ASSUM MP_TAC
   \\ `?x1 x2 x3. mw_simple_div 0x0w (REVERSE rs1) d = (x1,x2,x3)` by METIS_TAC [PAIR]
   \\ FULL_SIMP_TAC std_ss []
   \\ match_mp_tac IMP_IMP \\ conj_tac
@@ -3170,7 +3170,7 @@ val x64_div_thm = prove(
   \\ IMP_RES_TAC LENGTH_mw_simple_div
   \\ FULL_SIMP_TAC std_ss [LENGTH_REVERSE]
   \\ qpat_abbrev_tac `l5 = _ − 1 − LENGTH x1 − 1n`
-  \\ (x64_fix_thm |> Q.SPECL [`REVERSE x1`,`REVERSE qs1 ++ zs2`,
+  \\ (mc_fix_thm |> Q.SPECL [`REVERSE x1`,`REVERSE qs1 ++ zs2`,
         `n2w (LENGTH (ts1:'a word list))`,`l5`] |> MP_TAC)
   \\ MATCH_MP_TAC IMP_IMP \\ STRIP_TAC
   THEN1 (fs []
@@ -3206,7 +3206,7 @@ val x64_div_thm = prove(
     \\ fs [LEFT_ADD_DISTRIB,RIGHT_ADD_DISTRIB]
     \\ unabbrev_all_tac \\ fs [])
   \\ Q.MATCH_ASSUM_RENAME_TAC `l5 ≤ l6 + LENGTH x1`
-  \\ MP_TAC (x64_copy_down_thm |> Q.SPECL [`tt`,`REVERSE qs1`,`zs2`,`l6-1`])
+  \\ MP_TAC (mc_copy_down_thm |> Q.SPECL [`tt`,`REVERSE qs1`,`zs2`,`l6-1`])
   \\ MATCH_MP_TAC IMP_IMP \\ STRIP_TAC THEN1
    (fs [GSYM LENGTH_NIL]
     \\ Cases_on `LENGTH x1` \\ fs []
@@ -3235,9 +3235,9 @@ val x64_div_thm = prove(
 
 (* mwi_div -- addv zs [] c *)
 
-val (x64_add1_def, _,
-     x64_add1_pre_def, _) =
-  tailrec_define "x64_add1" ``
+val (mc_add1_def, _,
+     mc_add1_pre_def, _) =
+  tailrec_define "mc_add1" ``
     (\(l,r2,r10,r11,zs).
       if r10 = r11 then
         (let r0 = 0x1w in
@@ -3265,9 +3265,9 @@ val (x64_add1_def, _,
     word # 'a word # 'a word # 'a word list + num # 'a word # 'a word
     list) # bool``;
 
-val (x64_add1_call_def, _,
-     x64_add1_call_pre_def, _) =
-  tailrec_define "x64_add1_call" ``
+val (mc_add1_call_def, _,
+     mc_add1_call_pre_def, _) =
+  tailrec_define "mc_add1_call" ``
     (\(l,r2,r6,r11,zs).
       if r2 = 0x0w then (INR (l,r11,zs),T)
       else if r6 = 0x0w then (INR (l,r11,zs),T)
@@ -3275,22 +3275,22 @@ val (x64_add1_call_def, _,
         (let r2 = 0x0w in
          let r10 = r2 in
          let r2 = ~r2 in
-         let cond = x64_add1_pre (l-1,r2,r10,r11,zs) /\ l<>0 in
-         let (l,r11,zs) = x64_add1 (l-1,r2,r10,r11,zs)
+         let cond = mc_add1_pre (l-1,r2,r10,r11,zs) /\ l<>0 in
+         let (l,r11,zs) = mc_add1 (l-1,r2,r10,r11,zs)
          in
            (INR (l,r11,zs),cond)))
     :num # 'a word # 'a word # 'a word # 'a word list -> (num # 'a
     word # 'a word # 'a word # 'a word list + num # 'a word # 'a word
     list) # bool``;
 
-val x64_add1_thm = prove(
+val mc_add1_thm = prove(
   ``!(zs:'a word list) zs1 l.
       LENGTH (zs1 ++ zs) + 1 < dimword (:'a) /\ zs2 <> [] /\
       LENGTH zs <= l ==>
       ?rest l2.
-        x64_add1_pre (l,~0w,n2w (LENGTH zs1),n2w (LENGTH (zs1 ++ zs)),
+        mc_add1_pre (l,~0w,n2w (LENGTH zs1),n2w (LENGTH (zs1 ++ zs)),
                       zs1 ++ zs ++ zs2) /\
-        (x64_add1 (l,~0w,n2w (LENGTH zs1),n2w (LENGTH (zs1 ++ zs)),
+        (mc_add1 (l,~0w,n2w (LENGTH zs1),n2w (LENGTH (zs1 ++ zs)),
                    zs1 ++ zs ++ zs2) =
          (l2,n2w (LENGTH (zs1 ++ mw_addv zs [] T)),
              zs1 ++ mw_addv zs [] T ++ rest)) /\
@@ -3302,7 +3302,7 @@ val x64_add1_thm = prove(
   \\ FULL_SIMP_TAC std_ss [LENGTH,ADD1]
   \\ Induct
   \\ SIMP_TAC std_ss [mw_addv_NIL,LENGTH_APPEND,APPEND,APPEND_NIL,LENGTH]
-  \\ ONCE_REWRITE_TAC [x64_add1_def,x64_add1_pre_def] \\ REPEAT STRIP_TAC
+  \\ ONCE_REWRITE_TAC [mc_add1_def,mc_add1_pre_def] \\ REPEAT STRIP_TAC
   \\ `LENGTH zs1 < dimword (:'a)` by DECIDE_TAC
   \\ FULL_SIMP_TAC std_ss [LET_DEF,w2n_n2w,LENGTH_APPEND,LENGTH,
          word_add_n2w,n2w_11,LUPDATE_LENGTH]
@@ -3325,9 +3325,9 @@ val x64_add1_thm = prove(
 
 (* mwi_div -- subtraction *)
 
-val (x64_div_sub_aux1_def, _,
-     x64_div_sub_aux1_pre_def, _) =
-  tailrec_define "x64_div_sub_aux1" ``
+val (mc_div_sub_aux1_def, _,
+     mc_div_sub_aux1_pre_def, _) =
+  tailrec_define "mc_div_sub_aux1" ``
     (\(l,r1:'a word,r4:'a word,r8:'a word,r9:'a word,r10:'a word,ys,zs).
       if r1 = 0x1w then
         (let r1 = 0x0w:'a word
@@ -3346,15 +3346,15 @@ val (x64_div_sub_aux1_def, _,
          in
            (INL (l-1,r1,r4,r8,r9,r10,ys,zs),cond /\ l<>0n)))``;
 
-val (x64_div_sub_aux_def, _,
-     x64_div_sub_aux_pre_def, _) =
-  tailrec_define "x64_div_sub_aux" ``
+val (mc_div_sub_aux_def, _,
+     mc_div_sub_aux_pre_def, _) =
+  tailrec_define "mc_div_sub_aux" ``
     (\(l,r1,r8,r9,ys,zs).
       (let r10 = 0x0w in
        let r1 = r1 + 0x1w in
        let r4 = 1w in
-       let cond = x64_div_sub_aux1_pre (l-1,r1,r4,r8,r9,r10,ys,zs) /\ l<>0 in
-       let (l,r1,r4,r8,r9,r10,ys,zs) = x64_div_sub_aux1 (l-1,r1,r4,r8,r9,r10,ys,zs)
+       let cond = mc_div_sub_aux1_pre (l-1,r1,r4,r8,r9,r10,ys,zs) /\ l<>0 in
+       let (l,r1,r4,r8,r9,r10,ys,zs) = mc_div_sub_aux1 (l-1,r1,r4,r8,r9,r10,ys,zs)
        in
          (INR (l,r1,r4,r8,r9,r10,ys,zs),cond)))
     :num # 'a word # 'a word # 'a word # 'a word list # 'a word list
@@ -3362,16 +3362,16 @@ val (x64_div_sub_aux_def, _,
     list + num # 'a word # 'a word # 'a word # 'a word # 'a word # 'a
     word list # 'a word list) # bool``;
 
-val x64_div_sub_aux_def =
-  LIST_CONJ [x64_div_sub_aux_def,x64_div_sub_aux_pre_def,
-             x64_div_sub_aux1_def,x64_div_sub_aux1_pre_def]
+val mc_div_sub_aux_def =
+  LIST_CONJ [mc_div_sub_aux_def,mc_div_sub_aux_pre_def,
+             mc_div_sub_aux1_def,mc_div_sub_aux1_pre_def]
 
-val (x64_div_sub_def, _,
-     x64_div_sub_pre_def, _) =
-  tailrec_define "x64_div_sub" ``
+val (mc_div_sub_def, _,
+     mc_div_sub_pre_def, _) =
+  tailrec_define "mc_div_sub" ``
     (\(l,r1,r8,r9,ys,zs).
-      (let cond = x64_div_sub_aux_pre (l,r1,r8,r9,ys,zs) in
-       let (l,r1,r4,r8,r9,r10,ys,zs) = x64_div_sub_aux (l,r1,r8,r9,ys,zs)
+      (let cond = mc_div_sub_aux_pre (l,r1,r8,r9,ys,zs) in
+       let (l,r1,r4,r8,r9,r10,ys,zs) = mc_div_sub_aux (l,r1,r8,r9,ys,zs)
        in
          (INR (l,r1,r8,r9,r10,ys,zs),cond)))
     :num # 'a word # 'a word # 'a word # 'a word list # 'a word list
@@ -3379,12 +3379,12 @@ val (x64_div_sub_def, _,
      list + num # 'a word # 'a word # 'a word # 'a word # 'a word list
      # 'a word list) # bool``;
 
-val x64_div_sub_def =
-  LIST_CONJ [x64_div_sub_def,x64_div_sub_pre_def]
+val mc_div_sub_def =
+  LIST_CONJ [mc_div_sub_def,mc_div_sub_pre_def]
 
-val (x64_div_sub_call_def, _,
-     x64_div_sub_call_pre_def, _) =
-  tailrec_define "x64_div_sub_call" ``
+val (mc_div_sub_call_def, _,
+     mc_div_sub_call_pre_def, _) =
+  tailrec_define "mc_div_sub_call" ``
     (\(l,r1,r2,r6,ys,zs).
       if r2 = 0x0w then (INR (l,r6,ys,zs),T)
       else if r6 = 0x0w then (INR (l,r6,ys,zs),T)
@@ -3392,11 +3392,11 @@ val (x64_div_sub_call_def, _,
         (let r8 = r6 in
          let r9 = r6 in
          let r3 = r1 in
-         let cond = x64_div_sub_pre (l,r1,r8,r9,ys,zs) in
-         let (l,r1,r8,r9,r10,ys,zs) = x64_div_sub (l,r1,r8,r9,ys,zs) in
+         let cond = mc_div_sub_pre (l,r1,r8,r9,ys,zs) in
+         let (l,r1,r8,r9,r10,ys,zs) = mc_div_sub (l,r1,r8,r9,ys,zs) in
          let r10 = r3 in
-         let cond = cond /\ x64_fix_pre (l-1,r8,r10,zs) /\ l<>0 in
-         let (l,r8,r10,zs) = x64_fix (l-1,r8,r10,zs) in
+         let cond = cond /\ mc_fix_pre (l-1,r8,r10,zs) /\ l<>0 in
+         let (l,r8,r10,zs) = mc_fix (l-1,r8,r10,zs) in
          let r6 = r10
          in
            (INR (l,r6,ys,zs),cond)))
@@ -3404,24 +3404,24 @@ val (x64_div_sub_call_def, _,
      (num # 'a word # 'a word # 'a word # 'a word list # 'a word list +
       num # 'a word # 'a word list # 'a word list) # bool``;
 
-val x64_div_sub_aux_thm = prove(
+val mc_div_sub_aux_thm = prove(
   ``!(ys:'a word list) zs ys1 zs1 ys2 zs2 c r8 r9 l.
       (LENGTH zs1 = LENGTH ys1) /\ (LENGTH zs = LENGTH ys) /\
       LENGTH (zs1 ++ zs) + 1 < dimword (:'a) /\ LENGTH ys <= l ==>
       ?r8' r9' z_af' z_of' z_pf' z_sf' z_zf' l2.
-        x64_div_sub_aux1_pre (l,n2w (LENGTH zs + 1),b2w c,r8,
+        mc_div_sub_aux1_pre (l,n2w (LENGTH zs + 1),b2w c,r8,
            r9,n2w (LENGTH zs1),ys1 ++ ys ++ ys2,zs1 ++ zs ++ zs2) /\
-        (x64_div_sub_aux1 (l,n2w (LENGTH zs + 1),b2w c,r8,
+        (mc_div_sub_aux1 (l,n2w (LENGTH zs + 1),b2w c,r8,
            r9,n2w (LENGTH zs1),ys1 ++ ys ++ ys2,zs1 ++ zs ++ zs2) =
           (l2,0w,b2w (SND (mw_sub ys zs c)),r8',r9',n2w (LENGTH (zs1++zs)),
            ys1 ++ ys ++ ys2,zs1 ++ FST (mw_sub ys zs c) ++ zs2)) /\
         l <= l2 + LENGTH ys``,
   Induct THEN1
    (FULL_SIMP_TAC (srw_ss()) [LENGTH,LENGTH_NIL,mw_sub_def]
-    \\ ONCE_REWRITE_TAC [x64_div_sub_aux_def]
+    \\ ONCE_REWRITE_TAC [mc_div_sub_aux_def]
     \\ FULL_SIMP_TAC (srw_ss()) [LENGTH,LENGTH_NIL,mw_sub_def,LET_DEF])
   \\ Cases_on `zs` \\ FULL_SIMP_TAC std_ss [LENGTH,ADD1]
-  \\ ONCE_REWRITE_TAC [x64_div_sub_aux_def]
+  \\ ONCE_REWRITE_TAC [mc_div_sub_aux_def]
   \\ FULL_SIMP_TAC std_ss [LET_DEF,ADD1,n2w_w2n,w2n_n2w,
        single_sub_word_thm]
   \\ REPEAT STRIP_TAC \\ FULL_SIMP_TAC std_ss [LENGTH,LENGTH_APPEND]
@@ -3438,7 +3438,7 @@ val x64_div_sub_aux_thm = prove(
   \\ `LENGTH zs1 + 1 = LENGTH (SNOC h' ys1)` by
         FULL_SIMP_TAC std_ss [LENGTH_SNOC,ADD1]
   \\ FULL_SIMP_TAC std_ss []
-  \\ SEP_I_TAC "x64_div_sub_aux1" \\ POP_ASSUM MP_TAC
+  \\ SEP_I_TAC "mc_div_sub_aux1" \\ POP_ASSUM MP_TAC
   \\ MATCH_MP_TAC IMP_IMP \\ STRIP_TAC
   THEN1 (fs [])
   \\ STRIP_TAC \\ ASM_SIMP_TAC std_ss []
@@ -3452,28 +3452,28 @@ val x64_div_sub_aux_thm = prove(
   |> Q.SPECL [`ys`,`zs`,`[]`,`[]`,`ys2`,`zs2`,`T`]
   |> SIMP_RULE std_ss [APPEND,LENGTH,EVAL ``b2w T``] |> GEN_ALL;
 
-val x64_div_sub_thm = prove(
+val mc_div_sub_thm = prove(
   ``(LENGTH (zs:'a word list) = LENGTH ys) /\ LENGTH zs + 1 < dimword (:'a) /\
     LENGTH ys + 1 <= l ==>
     ?r8' r9' l2.
-      x64_div_sub_pre (l,n2w (LENGTH ys),r8,r9,ys ++ ys2,zs ++ zs2) /\
-      (x64_div_sub (l,n2w (LENGTH ys),r8,r9,ys ++ ys2,zs ++ zs2) =
+      mc_div_sub_pre (l,n2w (LENGTH ys),r8,r9,ys ++ ys2,zs ++ zs2) /\
+      (mc_div_sub (l,n2w (LENGTH ys),r8,r9,ys ++ ys2,zs ++ zs2) =
         (l2,0x0w,r8',r9',n2w (LENGTH ys),ys ++ ys2,
          FST (mw_sub ys zs T) ++ zs2)) /\
       l <= l2 + LENGTH ys + 1``,
-  SIMP_TAC std_ss [x64_div_sub_def]
-  \\ ONCE_REWRITE_TAC [x64_div_sub_aux_def]
+  SIMP_TAC std_ss [mc_div_sub_def]
+  \\ ONCE_REWRITE_TAC [mc_div_sub_aux_def]
   \\ SIMP_TAC std_ss [LET_DEF,WORD_SUB_RZERO,word_add_n2w]
-  \\ REPEAT STRIP_TAC \\ ASSUME_TAC x64_div_sub_aux_thm
-  \\ SEP_I_TAC "x64_div_sub_aux1" \\ POP_ASSUM MP_TAC
+  \\ REPEAT STRIP_TAC \\ ASSUME_TAC mc_div_sub_aux_thm
+  \\ SEP_I_TAC "mc_div_sub_aux1" \\ POP_ASSUM MP_TAC
   \\ FULL_SIMP_TAC std_ss [] \\ STRIP_TAC \\ FULL_SIMP_TAC std_ss []
   \\ fs [] \\ rfs []);
 
 (* mwi_div -- integer division *)
 
-val (x64_idiv_mod_header_def, _,
-     x64_idiv_mod_header_pre_def, _) =
-  tailrec_define "x64_idiv_mod_header" ``
+val (mc_idiv_mod_header_def, _,
+     mc_idiv_mod_header_pre_def, _) =
+  tailrec_define "mc_idiv_mod_header" ``
     (\(r6,r11).
       if r6 = 0x0w then (INR r6,T)
       else
@@ -3483,21 +3483,21 @@ val (x64_idiv_mod_header_def, _,
            else (let r6 = r6 + 0x1w in (INR r6,T))))
     :'a word # 'a word -> ('a word # 'a word + 'a word) # bool``;
 
-val x64_idiv_mod_header_thm = prove(
+val mc_idiv_mod_header_thm = prove(
   ``LENGTH (xs:'a word list) < dimword (:'a) ==>
-    (x64_idiv_mod_header (n2w (LENGTH xs),x64_header (t,ys)) =
-     x64_header (xs <> [] /\ t,xs))``,
-  SIMP_TAC std_ss [x64_idiv_mod_header_def,x64_header_sign,n2w_11,
-    ZERO_LT_dimword,LENGTH_NIL,LET_DEF,x64_header_def,word_lsl_n2w]
+    (mc_idiv_mod_header (n2w (LENGTH xs),mc_header (t,ys)) =
+     mc_header (xs <> [] /\ t,xs))``,
+  SIMP_TAC std_ss [mc_idiv_mod_header_def,mc_header_sign,n2w_11,
+    ZERO_LT_dimword,LENGTH_NIL,LET_DEF,mc_header_def,word_lsl_n2w]
   \\ rw[] \\ fs[] \\ rw[]
   THEN_LT USE_SG_THEN (fn th => metis_tac[th]) 1 2
   \\ Cases_on`xs` \\ fs[]
   \\ `dimindex(:'a) = 1` by fs[DIMINDEX_GT_0]
   \\ fs[dimword_def]);
 
-val (x64_idiv_def, _,
-     x64_idiv_pre_def, _) =
-  tailrec_define "x64_idiv" ``
+val (mc_idiv_def, _,
+     mc_idiv_pre_def, _) =
+  tailrec_define "mc_idiv" ``
     (\(l,r3,r10,r11,xs,ys,zs).
       (let r0 = r10 >>> 1 in
        let r1 = r11 >>> 1 in
@@ -3505,20 +3505,20 @@ val (x64_idiv_def, _,
        let r10 = r10 && 0x1w in
        let r20 = r10 in
        let r21 = r11 in
-       let cond = x64_div_pre (l,r0,r1,r3,xs,ys,zs) in
-       let (l,r0,r3,r6,xs,ys,zs) = x64_div (l,r0,r1,r3,xs,ys,zs) in
+       let cond = mc_div_pre (l,r0,r1,r3,xs,ys,zs) in
+       let (l,r0,r3,r6,xs,ys,zs) = mc_div (l,r0,r1,r3,xs,ys,zs) in
        let r11 = r21
        in
          if r3 = 0x0w then
            (let r10 = r0 in
             let r8 = r10 in
-            let cond = cond /\ x64_fix_pre (l-1,r8,r10,zs) /\ l<>0 in
-            let (l,r8,r10,zs) = x64_fix (l-1,r8,r10,zs) in
+            let cond = cond /\ mc_fix_pre (l-1,r8,r10,zs) /\ l<>0 in
+            let (l,r8,r10,zs) = mc_fix (l-1,r8,r10,zs) in
             let r11 = r10 in
             let r2 = r20 in
             let r3 = r2 in
-            let cond = cond /\ x64_add1_call_pre (l,r2,r6,r11,zs) in
-            let (l,r11,zs) = x64_add1_call (l,r2,r6,r11,zs)
+            let cond = cond /\ mc_add1_call_pre (l,r2,r6,r11,zs) in
+            let (l,r11,zs) = mc_add1_call (l,r2,r6,r11,zs)
             in
               if r11 = 0x0w then (INR (l,r11,xs,ys,zs),cond)
               else
@@ -3530,9 +3530,9 @@ val (x64_idiv_def, _,
            (let r2 = r20 in
             let r1 = r11 in
             let r1 = r1 >>> 1 in
-            let cond = cond /\ x64_div_sub_call_pre (l,r1,r2,r6,ys,zs) in
-            let (l,r6,ys,zs) = x64_div_sub_call (l,r1,r2,r6,ys,zs) in
-            let r6 = x64_idiv_mod_header (r6,r11) in
+            let cond = cond /\ mc_div_sub_call_pre (l,r1,r2,r6,ys,zs) in
+            let (l,r6,ys,zs) = mc_div_sub_call (l,r1,r2,r6,ys,zs) in
+            let r6 = mc_idiv_mod_header (r6,r11) in
             let r11 = r6
             in
               (INR (l,r11,xs,ys,zs),cond))))
@@ -3541,10 +3541,10 @@ val (x64_idiv_def, _,
      # 'a word list # 'a word list + num # 'a word # 'a word list # 'a
      word list # 'a word list) # bool``;
 
-val x64_header_XOR = prove(
-  ``!s t. ((x64_header (s,xs) ?? x64_header (t,ys)) && 0x1w:'a word) =
+val mc_header_XOR = prove(
+  ``!s t. ((mc_header (s,xs) ?? mc_header (t,ys)) && 0x1w:'a word) =
           (b2w (s <> t)):'a word``,
-  SIMP_TAC std_ss [WORD_RIGHT_AND_OVER_XOR,x64_header_AND_1]
+  SIMP_TAC std_ss [WORD_RIGHT_AND_OVER_XOR,mc_header_AND_1]
   \\ Cases \\ Cases \\ rw[b2w_def,b2n_def]);
 
 val b2w_EQ_0w = prove(
@@ -3555,45 +3555,45 @@ val mwi_divmod_alt_def = Define `
   mwi_divmod_alt w s_xs t_ys =
     if w = 0w then mwi_div s_xs t_ys else mwi_mod s_xs t_ys`;
 
-val x64_idiv_thm = prove(
+val mc_idiv_thm = prove(
   ``LENGTH (xs:'a word list) + LENGTH ys <= LENGTH zs /\
     LENGTH zs < dimword (:'a) DIV 2 /\
     mw_ok xs /\ mw_ok ys /\ ys <> [] /\
-    x64_div_max xs ys zs + 2 * LENGTH zs + 2 <= l ==>
+    mc_div_max xs ys zs + 2 * LENGTH zs + 2 <= l ==>
     ?zs1 l2.
-      x64_idiv_pre (l,r3,x64_header (s,xs),x64_header (t,ys),xs,ys,zs) /\
-      (x64_idiv (l,r3,x64_header (s,xs),x64_header (t,ys),xs,ys,zs) =
-        (l2,x64_header ((mwi_divmod_alt r3 (s,xs) (t,ys))),xs,ys,
+      mc_idiv_pre (l,r3,mc_header (s,xs),mc_header (t,ys),xs,ys,zs) /\
+      (mc_idiv (l,r3,mc_header (s,xs),mc_header (t,ys),xs,ys,zs) =
+        (l2,mc_header ((mwi_divmod_alt r3 (s,xs) (t,ys))),xs,ys,
          SND ((mwi_divmod_alt r3 (s,xs) (t,ys)))++zs1)) /\
       (LENGTH (SND ((mwi_divmod_alt r3 (s,xs) (t,ys)))++zs1) = LENGTH zs) /\
-      l <= l2 + x64_div_max xs ys zs + 2 * LENGTH zs + 2``,
-  FULL_SIMP_TAC std_ss [x64_idiv_def,x64_idiv_pre_def,LET_DEF]
-  \\ FULL_SIMP_TAC std_ss [x64_header_EQ,mwi_mul_def,x64_length]
-  \\ STRIP_TAC \\ FULL_SIMP_TAC std_ss [x64_header_XOR]
+      l <= l2 + mc_div_max xs ys zs + 2 * LENGTH zs + 2``,
+  FULL_SIMP_TAC std_ss [mc_idiv_def,mc_idiv_pre_def,LET_DEF]
+  \\ FULL_SIMP_TAC std_ss [mc_header_EQ,mwi_mul_def,mc_length]
+  \\ STRIP_TAC \\ FULL_SIMP_TAC std_ss [mc_header_XOR]
   \\ `LENGTH xs < dimword (:'a) DIV 2 /\ LENGTH ys < dimword (:'a) DIV 2` by DECIDE_TAC
   \\ `LENGTH zs < dimword (:'a)` by (FULL_SIMP_TAC (srw_ss()) [X_LT_DIV] \\ DECIDE_TAC)
-  \\ IMP_RES_TAC x64_length \\ FULL_SIMP_TAC std_ss []
+  \\ IMP_RES_TAC mc_length \\ FULL_SIMP_TAC std_ss []
   \\ `mw2n ys <> 0` by ALL_TAC THEN1
    (SIMP_TAC std_ss [GSYM mw_fix_NIL]
     \\ FULL_SIMP_TAC std_ss [mw_ok_mw_fix_ID])
   \\ `?res mod c. (mw_div xs ys = (res,mod,c))` by METIS_TAC [PAIR]
   \\ `c /\ (LENGTH mod = LENGTH ys)` by METIS_TAC [mw_div_thm,mw_ok_mw_fix_ID]
   \\ FULL_SIMP_TAC std_ss []
-  \\ ASSUME_TAC (x64_div_thm |> GEN_ALL)
-  \\ SEP_I_TAC "x64_div"
+  \\ ASSUME_TAC (mc_div_thm |> GEN_ALL)
+  \\ SEP_I_TAC "mc_div"
   \\ POP_ASSUM MP_TAC
-  \\ `x64_div_max xs ys zs ≤ l` by fs []
+  \\ `mc_div_max xs ys zs ≤ l` by fs []
   \\ FULL_SIMP_TAC std_ss [] \\ STRIP_TAC
   \\ FULL_SIMP_TAC std_ss []
   \\ NTAC 4 (POP_ASSUM MP_TAC) \\ NTAC 2 (POP_ASSUM (K ALL_TAC))
   \\ REPEAT STRIP_TAC
   \\ FULL_SIMP_TAC std_ss [LENGTH_APPEND]
   \\ Cases_on `r3 <> 0w` \\ FULL_SIMP_TAC std_ss [mwi_divmod_alt_def] THEN1
-   (FULL_SIMP_TAC std_ss [x64_div_sub_call_def,x64_div_sub_call_pre_def]
+   (FULL_SIMP_TAC std_ss [mc_div_sub_call_def,mc_div_sub_call_pre_def]
     \\ FULL_SIMP_TAC std_ss [TL,mwi_mod_def,mwi_divmod_def,LET_DEF,HD,NOT_CONS_NIL,
-         x64_header_XOR]
+         mc_header_XOR]
     \\ Cases_on `s = t` \\ FULL_SIMP_TAC std_ss [EVAL ``b2w F``] THEN1
-     (FULL_SIMP_TAC std_ss [x64_idiv_mod_header_thm]
+     (FULL_SIMP_TAC std_ss [mc_idiv_mod_header_thm]
       \\ ASSUME_TAC (Q.ISPEC `mod:'a word list` (GSYM mw_fix_thm))
       \\ POP_ASSUM (fn th => SIMP_TAC std_ss [Once th])
       \\ SIMP_TAC std_ss [GSYM APPEND_ASSOC,APPEND_11]
@@ -3602,13 +3602,13 @@ val x64_idiv_thm = prove(
       \\ DECIDE_TAC)
     \\ Cases_on `mw_fix mod = []`
     \\ FULL_SIMP_TAC std_ss [LENGTH,APPEND,LENGTH_APPEND]
-    THEN1 (SIMP_TAC std_ss [x64_idiv_mod_header_def] \\ fs [] \\ EVAL_TAC \\ simp[])
+    THEN1 (SIMP_TAC std_ss [mc_idiv_mod_header_def] \\ fs [] \\ EVAL_TAC \\ simp[])
     \\ FULL_SIMP_TAC std_ss [EVAL ``b2w T = 0x0w:'a word``,n2w_11,ZERO_LT_dimword]
     \\ FULL_SIMP_TAC std_ss [LENGTH_NIL]
     \\ Cases_on`1 MOD dimword(:'a) = 0` \\ fs[]
-    \\ (x64_div_sub_thm |> Q.INST [`ys2`|->`[]`]
+    \\ (mc_div_sub_thm |> Q.INST [`ys2`|->`[]`]
         |> SIMP_RULE std_ss [APPEND_NIL] |> GEN_ALL |> ASSUME_TAC)
-    \\ SEP_I_TAC "x64_div_sub" \\ POP_ASSUM MP_TAC
+    \\ SEP_I_TAC "mc_div_sub" \\ POP_ASSUM MP_TAC
     \\ MATCH_MP_TAC IMP_IMP \\ STRIP_TAC
     THEN1 (FULL_SIMP_TAC std_ss [GSYM LENGTH_NIL,X_LT_DIV] \\ fs [])
     \\ STRIP_TAC \\ FULL_SIMP_TAC std_ss []
@@ -3616,8 +3616,8 @@ val x64_idiv_thm = prove(
      (Cases_on `mw_sub ys mod T` \\ IMP_RES_TAC LENGTH_mw_sub
       \\ FULL_SIMP_TAC std_ss [])
     \\ ASM_SIMP_TAC std_ss []
-    \\ ASSUME_TAC x64_fix_thm
-    \\ SEP_I_TAC "x64_fix"
+    \\ ASSUME_TAC mc_fix_thm
+    \\ SEP_I_TAC "mc_fix"
     \\ pop_assum mp_tac
     \\ match_mp_tac IMP_IMP \\ strip_tac THEN1 fs []
     \\ strip_tac \\ FULL_SIMP_TAC std_ss []
@@ -3628,7 +3628,7 @@ val x64_idiv_thm = prove(
     \\ `LENGTH (mw_subv ys mod) <= LENGTH ys` by ALL_TAC
     THEN1 (MATCH_MP_TAC LENGTH_mw_subv \\ FULL_SIMP_TAC std_ss [])
     \\ `LENGTH (mw_subv ys mod) < dimword (:'a)` by DECIDE_TAC
-    \\ ASM_SIMP_TAC std_ss [x64_idiv_mod_header_thm]
+    \\ ASM_SIMP_TAC std_ss [mc_idiv_mod_header_thm]
     \\ FULL_SIMP_TAC std_ss [GSYM APPEND_ASSOC,APPEND_11]
     \\ FULL_SIMP_TAC std_ss [LENGTH_APPEND,LENGTH_REPLICATE]
     \\ SIMP_TAC std_ss [mw_subv_def]
@@ -3636,19 +3636,19 @@ val x64_idiv_thm = prove(
           by FULL_SIMP_TAC std_ss [LENGTH_mw_fix] \\ fs [])
   \\ `LENGTH res < dimword (:'a)` by DECIDE_TAC
   \\ FULL_SIMP_TAC std_ss [mwi_div_def]
-  \\ MP_TAC (x64_fix_thm |> Q.SPECL
+  \\ MP_TAC (mc_fix_thm |> Q.SPECL
        [`res`,`zs2`,`n2w (LENGTH (res:'a word list))`,`l2-1`])
   \\ match_mp_tac IMP_IMP \\ conj_tac THEN1 fs []
   \\ FULL_SIMP_TAC std_ss [] \\ STRIP_TAC \\ FULL_SIMP_TAC std_ss [HD,TL]
   \\ pop_assum mp_tac
   \\ NTAC 2 (POP_ASSUM (K ALL_TAC)) \\ strip_tac
-  \\ FULL_SIMP_TAC std_ss [x64_add1_call_def,x64_add1_call_pre_def,
+  \\ FULL_SIMP_TAC std_ss [mc_add1_call_def,mc_add1_call_pre_def,
                            LET_DEF,mwi_divmod_def,b2w_EQ_0w]
   \\ `LENGTH (mw_fix res) <= LENGTH res` by
         FULL_SIMP_TAC std_ss [LENGTH_mw_fix]
   \\ `LENGTH (mw_fix res) < dimword (:'a)` by DECIDE_TAC
   \\ Cases_on `s = t` \\ FULL_SIMP_TAC std_ss [n2w_11,ZERO_LT_dimword] THEN1
-   (SIMP_TAC (srw_ss()) [word_lsl_n2w,b2w_def,b2n_def,x64_header_def]
+   (SIMP_TAC (srw_ss()) [word_lsl_n2w,b2w_def,b2n_def,mc_header_def]
     \\ Cases_on`dimindex(:'a) < 2` \\ fs[X_LT_DIV,LEFT_ADD_DISTRIB]
     >- (
       `dimindex(:'a) = 1` by fs[DIMINDEX_GT_0]
@@ -3662,35 +3662,35 @@ val x64_idiv_thm = prove(
    (Cases_on `mw_fix res = []` \\ FULL_SIMP_TAC std_ss []
     \\ FULL_SIMP_TAC std_ss [GSYM APPEND_ASSOC,APPEND_11,
          LENGTH_APPEND,LENGTH_REPLICATE]
-    \\ SIMP_TAC (srw_ss()) [word_lsl_n2w,b2w_def,b2n_def,x64_header_def]
+    \\ SIMP_TAC (srw_ss()) [word_lsl_n2w,b2w_def,b2n_def,mc_header_def]
     \\ rw[]
     \\ `dimindex(:'a) = 1` by fs[DIMINDEX_GT_0]
     \\ fs[dimword_def])
   \\ SIMP_TAC std_ss [GSYM APPEND_ASSOC]
   \\ Q.ABBREV_TAC `ts1 = REPLICATE (LENGTH res - LENGTH (mw_fix res)) 0x0w ++ zs2`
-  \\ ASSUME_TAC (x64_add1_thm |> GEN_ALL)
-  \\ SEP_I_TAC "x64_add1" \\ POP_ASSUM MP_TAC
+  \\ ASSUME_TAC (mc_add1_thm |> GEN_ALL)
+  \\ SEP_I_TAC "mc_add1" \\ POP_ASSUM MP_TAC
   \\ MATCH_MP_TAC IMP_IMP \\ STRIP_TAC THEN1
     (Q.UNABBREV_TAC `ts1`
      \\ FULL_SIMP_TAC std_ss [n2w_11,ZERO_LT_dimword,GSYM LENGTH_NIL,
-          LENGTH_REPLICATE,x64_header_def,LENGTH,APPEND,word_add_n2w,LENGTH_APPEND]
+          LENGTH_REPLICATE,mc_header_def,LENGTH,APPEND,word_add_n2w,LENGTH_APPEND]
      \\ DECIDE_TAC)
   \\ STRIP_TAC \\ FULL_SIMP_TAC std_ss [NOT_CONS_NIL]
   \\ FULL_SIMP_TAC std_ss [n2w_11,ZERO_LT_dimword,LENGTH_NIL]
   \\ Cases_on `mw_addv (mw_fix res) [] T = []`
   \\ FULL_SIMP_TAC std_ss [n2w_11,ZERO_LT_dimword,LENGTH_NIL,
-       x64_header_def,LENGTH,APPEND,word_add_n2w,LENGTH_APPEND]
+       mc_header_def,LENGTH,APPEND,word_add_n2w,LENGTH_APPEND]
   THEN1 (Q.UNABBREV_TAC `ts1`
     \\ FULL_SIMP_TAC std_ss [n2w_11,ZERO_LT_dimword,LENGTH_NIL,LENGTH_REPLICATE,
-         x64_header_def,LENGTH,APPEND,word_add_n2w,LENGTH_APPEND]
+         mc_header_def,LENGTH,APPEND,word_add_n2w,LENGTH_APPEND]
     \\ DECIDE_TAC)
   \\ FULL_SIMP_TAC std_ss [n2w_11,ZERO_LT_dimword,LENGTH_NIL,LENGTH_REPLICATE,
-         x64_header_def,LENGTH,APPEND,word_add_n2w,LENGTH_APPEND,APPEND_11]
+         mc_header_def,LENGTH,APPEND,word_add_n2w,LENGTH_APPEND,APPEND_11]
   \\ FULL_SIMP_TAC std_ss [b2w_def,b2n_def]
   \\ SIMP_TAC (srw_ss()) [word_lsl_n2w,word_add_n2w]
   \\ Q.UNABBREV_TAC `ts1`
   \\ FULL_SIMP_TAC std_ss [n2w_11,ZERO_LT_dimword,LENGTH_NIL,LENGTH_REPLICATE,
-         x64_header_def,LENGTH,APPEND,word_add_n2w,LENGTH_APPEND]
+         mc_header_def,LENGTH,APPEND,word_add_n2w,LENGTH_APPEND]
   \\ rw[]
   >- (
     `dimindex(:'a) = 1` by fs[DIMINDEX_GT_0]
@@ -3701,20 +3701,20 @@ val x64_idiv_thm = prove(
 
 (* int to decimal conversion *)
 
-val (x64_to_dec_def, _,
-     x64_to_dec_pre_def, _) =
-  tailrec_define "x64_to_dec" ``
+val (mc_to_dec_def, _,
+     mc_to_dec_pre_def, _) =
+  tailrec_define "mc_to_dec" ``
     (\(r9,r10,zs,ss).
       (let r2 = 0x0w in
        let r11 = r10 in
-       let cond = x64_simple_div1_pre (r2,r9,r10,zs) in
-       let (r2,r9,r10,zs) = x64_simple_div1 (r2,r9,r10,zs) in
+       let cond = mc_simple_div1_pre (r2,r9,r10,zs) in
+       let (r2,r9,r10,zs) = mc_simple_div1 (r2,r9,r10,zs) in
        let r2 = r2 + 0x30w in
        let ss = r2::ss in
        let r8 = r10 in
        let r10 = r11 in
-       let cond = cond /\ x64_fix_pre (r8,r10,zs) in
-       let (r8,r10,zs) = x64_fix (r8,r10,zs)
+       let cond = cond /\ mc_fix_pre (r8,r10,zs) in
+       let (r8,r10,zs) = mc_fix (r8,r10,zs)
        in
          if r10 = 0x0w then (INR (zs,ss),cond)
          else (INL (r9,r10,zs,ss),cond)))
@@ -3722,19 +3722,19 @@ val (x64_to_dec_def, _,
      word # 'a word list # 'a word list + 'a word list # 'a word list)
      # bool``;
 
-val (x64_int_to_dec_def, _,
-     x64_int_to_dec_pre_def, _) =
-  tailrec_define "x64_int_to_dec" ``
+val (mc_int_to_dec_def, _,
+     mc_int_to_dec_pre_def, _) =
+  tailrec_define "mc_int_to_dec" ``
     (\(r10,xs,zs,ss).
       (let r1 = r10 in
        let r10 = r10 >>> 1 in
-       let cond = x64_copy_over_pre (r10,xs,zs) in
-       let (xs,zs) = x64_copy_over (r10,xs,zs) in
+       let cond = mc_copy_over_pre (r10,xs,zs) in
+       let (xs,zs) = mc_copy_over (r10,xs,zs) in
        let r10 = r1 in
        let r10 = r10 >>> 1 in
        let r9 = 0xAw in
-       let cond = cond /\ x64_to_dec_pre (r9,r10,zs,ss) in
-       let (zs,ss) = x64_to_dec (r9,r10,zs,ss)
+       let cond = cond /\ mc_to_dec_pre (r9,r10,zs,ss) in
+       let (zs,ss) = mc_to_dec (r9,r10,zs,ss)
        in
          if r1 && 0x1w = 0x0w then (INR (xs,zs,ss),cond)
          else (let r2 = 0x7Ew in let ss = r2::ss in (INR (xs,zs,ss),cond))))
@@ -3742,12 +3742,12 @@ val (x64_int_to_dec_def, _,
      # 'a word list # 'a word list # 'a word list + 'a word list # 'a
      word list # 'a word list) # bool``;
 
-val x64_to_dec_thm = prove(
+val mc_to_dec_thm = prove(
   ``!(xs:'a word list) ys zs ss.
       LENGTH xs < dimword (:'a) /\ (mw_to_dec xs = (ys,T)) ==>
       ?zs1.
-        x64_to_dec_pre (10w,n2w (LENGTH xs),xs++zs,ss) /\
-        (x64_to_dec (10w,n2w (LENGTH xs),xs++zs,ss) = (zs1,ys ++ ss)) /\
+        mc_to_dec_pre (10w,n2w (LENGTH xs),xs++zs,ss) /\
+        (mc_to_dec (10w,n2w (LENGTH xs),xs++zs,ss) = (zs1,ys ++ ss)) /\
         (LENGTH zs1 = LENGTH xs + LENGTH zs)``,
   HO_MATCH_MP_TAC mw_to_dec_ind \\ REPEAT STRIP_TAC \\ POP_ASSUM MP_TAC
   \\ SIMP_TAC std_ss [Once mw_to_dec_def]
@@ -3755,16 +3755,16 @@ val x64_to_dec_thm = prove(
   \\ `?qs r c1. mw_simple_div 0x0w (REVERSE xs) 0xAw = (qs,r,c1)` by METIS_TAC [PAIR]
   \\ `?res c2. mw_to_dec (mw_fix (REVERSE qs)) = (res,c2)` by METIS_TAC [PAIR]
   \\ FULL_SIMP_TAC std_ss [LET_DEF]
-  \\ ONCE_REWRITE_TAC [x64_to_dec_def,x64_to_dec_pre_def]
+  \\ ONCE_REWRITE_TAC [mc_to_dec_def,mc_to_dec_pre_def]
   \\ SIMP_TAC std_ss [LET_DEF]
   \\ ONCE_REWRITE_TAC [EQ_SYM_EQ] \\ STRIP_TAC
   \\ `c1` by ALL_TAC \\ FULL_SIMP_TAC std_ss []
   THEN1 (Cases_on `LENGTH (mw_fix (REVERSE qs)) = 0` \\ FULL_SIMP_TAC std_ss [])
   \\ SIMP_TAC std_ss [Once EQ_SYM_EQ]
-  \\ IMP_RES_TAC x64_simple_div1_thm
+  \\ IMP_RES_TAC mc_simple_div1_thm
   \\ FULL_SIMP_TAC std_ss []
   \\ IMP_RES_TAC LENGTH_mw_simple_div
-  \\ MP_TAC (x64_fix_thm |> Q.SPECL [`REVERSE qs`,`zs`,`0w`])
+  \\ MP_TAC (mc_fix_thm |> Q.SPECL [`REVERSE qs`,`zs`,`0w`])
   \\ FULL_SIMP_TAC std_ss [LENGTH_REVERSE] \\ STRIP_TAC
   \\ `LENGTH (mw_fix (REVERSE qs)) <= LENGTH (REVERSE qs)` by
         METIS_TAC [LENGTH_mw_fix]
@@ -3775,39 +3775,39 @@ val x64_to_dec_thm = prove(
   \\ Cases_on `mw_fix (REVERSE qs) = []` \\ FULL_SIMP_TAC std_ss [LENGTH]
   THEN1 (SIMP_TAC std_ss [LENGTH_REPLICATE,LENGTH_APPEND] \\ EVAL_TAC)
   \\ FULL_SIMP_TAC std_ss [GSYM APPEND_ASSOC]
-  \\ SEP_I_TAC "x64_to_dec"
+  \\ SEP_I_TAC "mc_to_dec"
   \\ FULL_SIMP_TAC std_ss []
   \\ SIMP_TAC std_ss [LENGTH_REPLICATE,LENGTH_APPEND,REVERSE_APPEND,REVERSE_DEF]
   \\ FULL_SIMP_TAC std_ss [APPEND]
   \\ FULL_SIMP_TAC std_ss [LENGTH_REVERSE] \\ DECIDE_TAC);
 
-val x64_int_to_dec_thm = prove(
+val mc_int_to_dec_thm = prove(
   ``(mwi_to_dec (s,xs) = (res,T)) /\ LENGTH zs < dimword (:'a) DIV 2 /\
     LENGTH (xs:'a word list) <= LENGTH zs ==>
     ?zs1.
-      (x64_int_to_dec_pre (x64_header(s,xs),xs,zs,ss)) /\
-      (x64_int_to_dec (x64_header(s,xs),xs,zs,ss) = (xs,zs1,res ++ ss)) /\
+      (mc_int_to_dec_pre (mc_header(s,xs),xs,zs,ss)) /\
+      (mc_int_to_dec (mc_header(s,xs),xs,zs,ss) = (xs,zs1,res ++ ss)) /\
       (LENGTH zs1 = LENGTH zs)``,
   SIMP_TAC std_ss [Once EQ_SYM_EQ]
-  \\ SIMP_TAC std_ss [x64_int_to_dec_def,x64_int_to_dec_pre_def,LET_DEF] \\ STRIP_TAC
+  \\ SIMP_TAC std_ss [mc_int_to_dec_def,mc_int_to_dec_pre_def,LET_DEF] \\ STRIP_TAC
   \\ `LENGTH xs < dimword (:'a) DIV 2` by DECIDE_TAC
-  \\ ASM_SIMP_TAC std_ss [x64_length]
+  \\ ASM_SIMP_TAC std_ss [mc_length]
   \\ IMP_RES_TAC LESS_EQ_LENGTH
   \\ FULL_SIMP_TAC std_ss []
-  \\ ASSUME_TAC (x64_copy_over_thm |> Q.SPECL [`xs0`,`zs0`,`[]`] |> GEN_ALL)
+  \\ ASSUME_TAC (mc_copy_over_thm |> Q.SPECL [`xs0`,`zs0`,`[]`] |> GEN_ALL)
   \\ FULL_SIMP_TAC std_ss [APPEND_NIL]
   \\ `LENGTH xs + LENGTH xs2 < dimword (:'a)` by
         (FULL_SIMP_TAC (srw_ss()) [X_LT_DIV] \\ DECIDE_TAC)
-  \\ SEP_I_TAC "x64_copy_over"
+  \\ SEP_I_TAC "mc_copy_over"
   \\ POP_ASSUM MP_TAC \\ FULL_SIMP_TAC std_ss [LENGTH_APPEND]
   \\ STRIP_TAC \\ FULL_SIMP_TAC std_ss []
   \\ FULL_SIMP_TAC std_ss [mwi_to_dec_def,LET_DEF]
   \\ Cases_on `mw_to_dec xs` \\ FULL_SIMP_TAC std_ss []
   \\ POP_ASSUM MP_TAC \\ FULL_SIMP_TAC std_ss [] \\ STRIP_TAC
   \\ `LENGTH xs < dimword (:'a)` by DECIDE_TAC
-  \\ IMP_RES_TAC x64_to_dec_thm
+  \\ IMP_RES_TAC mc_to_dec_thm
   \\ POP_ASSUM (STRIP_ASSUME_TAC o Q.SPECL [`xs2`,`ss`])
-  \\ FULL_SIMP_TAC std_ss [x64_header_sign]
+  \\ FULL_SIMP_TAC std_ss [mc_header_sign]
   \\ Cases_on `s` \\ FULL_SIMP_TAC std_ss [APPEND]);
 
 *)
@@ -3824,17 +3824,17 @@ val int_op_rep_def = Define `
   (int_op_rep Mod = 6w) /\
   (int_op_rep Dec = 7w:'a word)`;
 
-val (x64_isub_flip_def, _,
-     x64_isub_flip_pre_def, _) =
-  tailrec_define "x64_isub_flip" ``
+val (mc_isub_flip_def, _,
+     mc_isub_flip_pre_def, _) =
+  tailrec_define "mc_isub_flip" ``
     (\(r1,r3).
       if r3 = 0x0w then (INR (r1,r3),T)
       else (let r1 = r1 ?? 0x1w in (INR (r1,r3),T)))
     :'a word # 'a word -> ('a word # 'a word + 'a word # 'a word) # bool``;
 
-val (x64_icmp_res_def, _,
-     x64_icmp_res_pre_def, _) =
-  tailrec_define "x64_icmp_res" ``
+val (mc_icmp_res_def, _,
+     mc_icmp_res_pre_def, _) =
+  tailrec_define "mc_icmp_res" ``
     (\(r10,r3).
       if r3 = 0x2w then
         if r10 = 0x1w then (let r10 = 0x1w in (INR r10,T))
@@ -3843,13 +3843,13 @@ val (x64_icmp_res_def, _,
       else (let r10 = 0x0w in (INR r10,T)))
     :'a word # 'a word -> ('a word # 'a word + 'a word) # bool``;
 
-val (x64_full_cmp_def, _,
-     x64_full_cmp_pre_def, _) =
-  tailrec_define "x64_full_cmp" ``
+val (mc_full_cmp_def, _,
+     mc_full_cmp_pre_def, _) =
+  tailrec_define "mc_full_cmp" ``
     (\(l,r3,r10,r11,xs,ys,zs).
-      (let cond = x64_icompare_pre (l,r10,r11,xs,ys) in
-       let (l,r10,xs,ys) = x64_icompare (l,r10,r11,xs,ys) in
-       let r10 = x64_icmp_res (r10,r3)
+      (let cond = mc_icompare_pre (l,r10,r11,xs,ys) in
+       let (l,r10,xs,ys) = mc_icompare (l,r10,r11,xs,ys) in
+       let r10 = mc_icmp_res (r10,r3)
        in
          if r10 = 0x0w then (INR (l,r10,xs,ys,zs),cond)
          else
@@ -3869,30 +3869,30 @@ val NumABS_LEMMA = prove(
   ``(Num (ABS (0:int)) = 0:num) /\ (Num (ABS (1:int)) = 1:num)``,
   intLib.COOPER_TAC);
 
-val x64_full_cmp_lt = prove(
-  ``((x64_header (s,xs) = 0x0w) <=> (xs = [])) /\ mw_ok xs /\
-    ((x64_header (t,ys) = 0x0w) <=> (ys = [])) /\ mw_ok ys /\
+val mc_full_cmp_lt = prove(
+  ``((mc_header (s,xs) = 0x0w) <=> (xs = [])) /\ mw_ok xs /\
+    ((mc_header (t,ys) = 0x0w) <=> (ys = [])) /\ mw_ok ys /\
     LENGTH (xs:'a word list) < dimword (:'a) DIV 2 /\
     LENGTH ys < dimword (:'a) DIV 2 /\
     LENGTH xs + LENGTH ys < LENGTH zs /\ LENGTH zs < dimword (:'a) DIV 2 /\
     LENGTH xs + 1 <= l ==>
     ?zs1 l2.
-      x64_full_cmp_pre (l,2w,x64_header (s,xs),x64_header (t,ys),xs,ys,zs) /\
-      (x64_full_cmp (l,2w,x64_header (s,xs),x64_header (t,ys),xs,ys,zs) =
-       (l2,x64_header (mwi_op Lt (s,xs) (t,ys)),xs,ys,
+      mc_full_cmp_pre (l,2w,mc_header (s,xs),mc_header (t,ys),xs,ys,zs) /\
+      (mc_full_cmp (l,2w,mc_header (s,xs),mc_header (t,ys),xs,ys,zs) =
+       (l2,mc_header (mwi_op Lt (s,xs) (t,ys)),xs,ys,
         SND (mwi_op Lt (s,xs) (t,ys)) ++ zs1)) /\
       (LENGTH (SND (mwi_op Lt (s,xs) (t,ys)) ++ zs1) = LENGTH zs) /\
       l <= l2 + LENGTH xs + 1``,
-  SIMP_TAC std_ss [x64_full_cmp_def,x64_full_cmp_pre_def,LET_DEF] \\ STRIP_TAC
-  \\ MP_TAC x64_icompare_thm \\ FULL_SIMP_TAC std_ss []
+  SIMP_TAC std_ss [mc_full_cmp_def,mc_full_cmp_pre_def,LET_DEF] \\ STRIP_TAC
+  \\ MP_TAC mc_icompare_thm \\ FULL_SIMP_TAC std_ss []
   \\ STRIP_TAC \\ FULL_SIMP_TAC std_ss [mwi_op_def] \\ SIMP_TAC std_ss [mwi_lt_def]
   \\ Cases_on `mwi_compare (s,xs) (t,ys)`
-  \\ FULL_SIMP_TAC (srw_ss()) [cmp2w_def,x64_icmp_res_def,n2w_11,LET_DEF]
+  \\ FULL_SIMP_TAC (srw_ss()) [cmp2w_def,mc_icmp_res_def,n2w_11,LET_DEF]
   THEN1 (Q.EXISTS_TAC `zs` \\ SIMP_TAC std_ss []
     \\ SIMP_TAC std_ss [i2mw_def,NumABS_LEMMA,EVAL ``n2mw 0``] \\ EVAL_TAC
     \\ fs[])
   \\ REV (Cases_on `x`)
-  \\ FULL_SIMP_TAC (srw_ss()) [cmp2w_def,x64_icmp_res_def,n2w_11,LET_DEF]
+  \\ FULL_SIMP_TAC (srw_ss()) [cmp2w_def,mc_icmp_res_def,n2w_11,LET_DEF]
   THEN1 (Q.EXISTS_TAC `zs` \\ SIMP_TAC std_ss []
     \\ SIMP_TAC std_ss [i2mw_def,NumABS_LEMMA,EVAL ``n2mw 0``] \\ EVAL_TAC
     \\ IF_CASES_TAC \\ fs[]
@@ -3904,25 +3904,25 @@ val x64_full_cmp_lt = prove(
   \\ SIMP_TAC std_ss [i2mw_def,NumABS_LEMMA,EVAL ``n2mw 0``,n2mw_1]
   \\ EVAL_TAC \\ FULL_SIMP_TAC std_ss [ADD1] \\ fs[]);
 
-val x64_full_cmp_eq = prove(
-  ``((x64_header (s,xs) = 0x0w) <=> (xs = [])) /\ mw_ok xs /\
-    ((x64_header (t,ys) = 0x0w) <=> (ys = [])) /\ mw_ok ys /\
+val mc_full_cmp_eq = prove(
+  ``((mc_header (s,xs) = 0x0w) <=> (xs = [])) /\ mw_ok xs /\
+    ((mc_header (t,ys) = 0x0w) <=> (ys = [])) /\ mw_ok ys /\
     LENGTH (xs:'a word list) < dimword (:'a) DIV 2 /\
     LENGTH ys < dimword (:'a) DIV 2 /\
     LENGTH xs + LENGTH ys < LENGTH zs /\ LENGTH zs < dimword (:'a) DIV 2 /\
     LENGTH xs + 1 <= l ==>
     ?zs1 l2.
-      x64_full_cmp_pre (l,3w,x64_header (s,xs),x64_header (t,ys),xs,ys,zs) /\
-      (x64_full_cmp (l,3w,x64_header (s,xs),x64_header (t,ys),xs,ys,zs) =
-       (l2,x64_header (mwi_op Eq (s,xs) (t,ys)),xs,ys,
+      mc_full_cmp_pre (l,3w,mc_header (s,xs),mc_header (t,ys),xs,ys,zs) /\
+      (mc_full_cmp (l,3w,mc_header (s,xs),mc_header (t,ys),xs,ys,zs) =
+       (l2,mc_header (mwi_op Eq (s,xs) (t,ys)),xs,ys,
         SND (mwi_op Eq (s,xs) (t,ys)) ++ zs1)) /\
       (LENGTH (SND (mwi_op Eq (s,xs) (t,ys)) ++ zs1) = LENGTH zs) /\
       l <= l2 + LENGTH xs + 1``,
-  SIMP_TAC std_ss [x64_full_cmp_def,x64_full_cmp_pre_def,LET_DEF] \\ STRIP_TAC
-  \\ MP_TAC x64_icompare_thm \\ FULL_SIMP_TAC std_ss []
+  SIMP_TAC std_ss [mc_full_cmp_def,mc_full_cmp_pre_def,LET_DEF] \\ STRIP_TAC
+  \\ MP_TAC mc_icompare_thm \\ FULL_SIMP_TAC std_ss []
   \\ STRIP_TAC \\ FULL_SIMP_TAC std_ss [mwi_op_def] \\ SIMP_TAC std_ss [mwi_eq_def]
   \\ REV (Cases_on `mwi_compare (s,xs) (t,ys)`) THEN1
-   (FULL_SIMP_TAC (srw_ss()) [cmp2w_def,x64_icmp_res_def,n2w_11,LET_DEF]
+   (FULL_SIMP_TAC (srw_ss()) [cmp2w_def,mc_icmp_res_def,n2w_11,LET_DEF]
     \\ Q.EXISTS_TAC `zs` \\ SIMP_TAC std_ss []
     \\ SIMP_TAC std_ss [i2mw_def,NumABS_LEMMA,EVAL ``n2mw 0``] \\ fs[]
     \\ Cases_on`3 < dimword(:'a)` \\ fs[]
@@ -3934,7 +3934,7 @@ val x64_full_cmp_eq = prove(
     \\ `dimword(:'a) = 2` by ( fs[dimword_def,X_LT_DIV] )
     \\ fs[])
   \\ SIMP_TAC std_ss [cmp2w_def]
-  \\ FULL_SIMP_TAC (srw_ss()) [cmp2w_def,x64_icmp_res_def,n2w_11,LET_DEF]
+  \\ FULL_SIMP_TAC (srw_ss()) [cmp2w_def,mc_icmp_res_def,n2w_11,LET_DEF]
   \\ Cases_on `zs` \\ FULL_SIMP_TAC std_ss [LENGTH]
   \\ Q.EXISTS_TAC `t'` \\ FULL_SIMP_TAC std_ss [LUPDATE_def]
   \\ SIMP_TAC std_ss [i2mw_def,NumABS_LEMMA,EVAL ``n2mw 0``]
@@ -3943,45 +3943,45 @@ val x64_full_cmp_eq = prove(
   \\ `dimword(:'a) = 2` by ( fs[dimword_def,X_LT_DIV] )
   \\ fs[]);
 
-val (x64_iop_def, _,
-     x64_iop_pre_def, _) =
-  tailrec_define "x64_iop" ``
+val (mc_iop_def, _,
+     mc_iop_pre_def, _) =
+  tailrec_define "mc_iop" ``
     (\(l,r0,r1,r3,xs,ys,zs).
       if r3 <+ 0x2w then
-        (let (r1,r3) = x64_isub_flip (r1,r3) in
+        (let (r1,r3) = mc_isub_flip (r1,r3) in
          let r2 = r1 in
          let r1 = r0 in
-         let cond = x64_iadd_pre (l,r1,r2,xs,ys,zs) in
-         let (l,r10,xs,ys,zs) = x64_iadd (l,r1,r2,xs,ys,zs)
+         let cond = mc_iadd_pre (l,r1,r2,xs,ys,zs) in
+         let (l,r10,xs,ys,zs) = mc_iadd (l,r1,r2,xs,ys,zs)
          in
            (INR (l,r10,xs,ys,zs),cond))
   (*  else if r3 <+ 0x4w then
         (let r10 = r0 in
          let r11 = r1 in
-         let cond = x64_full_cmp_pre (r3,r10,r11,xs,ys,zs) in
-         let (r10,xs,ys,zs) = x64_full_cmp (r3,r10,r11,xs,ys,zs)
+         let cond = mc_full_cmp_pre (r3,r10,r11,xs,ys,zs) in
+         let (r10,xs,ys,zs) = mc_full_cmp (r3,r10,r11,xs,ys,zs)
          in
            (INR (r10,xs,ys,zs,ss),cond))  *)
       else if r3 = 0x4w then
         (let r2 = r1 in
          let r1 = r0 in
-         let cond = x64_imul_pre (l,r1,r2,xs,ys,zs) in
-         let (l,r10,xs,ys,zs) = x64_imul (l,r1,r2,xs,ys,zs)
+         let cond = mc_imul_pre (l,r1,r2,xs,ys,zs) in
+         let (l,r10,xs,ys,zs) = mc_imul (l,r1,r2,xs,ys,zs)
          in
            (INR (l,r10,xs,ys,zs),cond))
       else (* if r3 <+ 0x7w then *)
         (let r3 = r3 - 0x5w in
          let r10 = r0 in
          let r11 = r1 in
-         let cond = x64_idiv_pre (l,r3,r10,r11,xs,ys,zs) in
-         let (l,r11,xs,ys,zs) = x64_idiv (l,r3,r10,r11,xs,ys,zs) in
+         let cond = mc_idiv_pre (l,r3,r10,r11,xs,ys,zs) in
+         let (l,r11,xs,ys,zs) = mc_idiv (l,r3,r10,r11,xs,ys,zs) in
          let r10 = r11
          in
            (INR (l,r10,xs,ys,zs),cond)))
   (*  else
         (let r10 = r0 in
-         let cond = x64_int_to_dec_pre (r10,xs,zs,ss) in
-         let (xs,zs,ss) = x64_int_to_dec (r10,xs,zs,ss) in
+         let cond = mc_int_to_dec_pre (r10,xs,zs,ss) in
+         let (xs,zs,ss) = mc_int_to_dec (r10,xs,zs,ss) in
          let r10 = 0x0w
          in
            (INR (r10,xs,ys,zs,ss),cond)) *)
@@ -3990,9 +3990,9 @@ val (x64_iop_def, _,
      # 'a word list # 'a word list + num # 'a word # 'a word list # 'a
      word list # 'a word list) # bool``;
 
-val x64_header_XOR_1 = prove(
-  ``x64_header (s,xs) ?? 1w = x64_header (~s,xs)``,
-  simp[x64_header_def,GSYM word_mul_n2w]
+val mc_header_XOR_1 = prove(
+  ``mc_header (s,xs) ?? 1w = mc_header (~s,xs)``,
+  simp[mc_header_def,GSYM word_mul_n2w]
   \\ Q.SPEC_TAC(`n2w(LENGTH xs):'a word`,`w`)
   \\ gen_tac
   \\ qspecl_then[`w`,`1`]mp_tac (GSYM WORD_MUL_LSL)
@@ -4001,24 +4001,24 @@ val x64_header_XOR_1 = prove(
   \\ FIRST (map match_mp_tac [xor_one_add_one,add_one_xor_one])
   \\ rw[word_lsl_def,fcpTheory.FCP_BETA] );
 
-val x64_iop_thm = store_thm("x64_iop_thm",
+val mc_iop_thm = store_thm("mc_iop_thm",
   ``3 < dimindex(:'a) ==>
-    ((x64_header (s,xs) = 0x0w) <=> (xs = [])) /\ mw_ok xs /\
-    ((x64_header (t,ys) = 0x0w) <=> (ys = [])) /\ mw_ok ys /\
+    ((mc_header (s,xs) = 0x0w) <=> (xs = [])) /\ mw_ok xs /\
+    ((mc_header (t,ys) = 0x0w) <=> (ys = [])) /\ mw_ok ys /\
     LENGTH (xs:'a word list) + LENGTH ys < LENGTH zs /\
     LENGTH zs < dimword (:'a) DIV 2 /\
     iop <> Lt /\ iop <> Eq /\ iop <> Dec /\
     (((iop = Div) \/ (iop = Mod)) ==> ys <> []) /\
-    x64_div_max xs ys zs + 2 * LENGTH zs + 2 <= l ==>
+    mc_div_max xs ys zs + 2 * LENGTH zs + 2 <= l ==>
     ?zs1 l2.
-      x64_iop_pre (l,x64_header (s,xs),x64_header (t,ys),int_op_rep iop,
+      mc_iop_pre (l,mc_header (s,xs),mc_header (t,ys),int_op_rep iop,
                    xs,ys,zs) /\
-      (x64_iop (l,x64_header (s,xs),x64_header (t,ys),int_op_rep iop,
+      (mc_iop (l,mc_header (s,xs),mc_header (t,ys),int_op_rep iop,
                 xs,ys,zs) =
-       (l2,x64_header (mwi_op iop (s,xs) (t,ys)),xs,ys,
+       (l2,mc_header (mwi_op iop (s,xs) (t,ys)),xs,ys,
         SND (mwi_op iop (s,xs) (t,ys)) ++ zs1)) /\
       (LENGTH (SND (mwi_op iop (s,xs) (t,ys)) ++ zs1) = LENGTH zs) /\
-      l <= l2 + x64_div_max xs ys zs + 2 * LENGTH zs + 2``,
+      l <= l2 + mc_div_max xs ys zs + 2 * LENGTH zs + 2``,
   strip_tac \\
  `10 < dimword(:'a)`
   by (
@@ -4027,36 +4027,36 @@ val x64_iop_thm = store_thm("x64_iop_thm",
   Cases_on `iop` \\ SIMP_TAC std_ss [int_op_rep_def] \\ REPEAT STRIP_TAC
   \\ `LENGTH xs < dimword (:'a) DIV 2 /\ LENGTH ys < dimword (:'a) DIV 2` by DECIDE_TAC
   \\ `LENGTH xs + LENGTH ys <= LENGTH zs` by DECIDE_TAC
-  \\ SIMP_TAC std_ss [x64_iop_def,x64_iop_pre_def,WORD_LO]
-  \\ SIMP_TAC (srw_ss()) [w2n_n2w,LET_DEF,x64_isub_flip_def]
+  \\ SIMP_TAC std_ss [mc_iop_def,mc_iop_pre_def,WORD_LO]
+  \\ SIMP_TAC (srw_ss()) [w2n_n2w,LET_DEF,mc_isub_flip_def]
   THEN1 (
     reverse IF_CASES_TAC \\ rfs[]
-    \\ MP_TAC x64_iadd_thm \\ fs[]
-    \\ match_mp_tac IMP_IMP \\ conj_tac THEN1 fs [x64_div_max_def]
+    \\ MP_TAC mc_iadd_thm \\ fs[]
+    \\ match_mp_tac IMP_IMP \\ conj_tac THEN1 fs [mc_div_max_def]
     \\ STRIP_TAC \\ FULL_SIMP_TAC std_ss [mwi_op_def]
-    \\ fs[] \\ fs [x64_div_max_def])
+    \\ fs[] \\ fs [mc_div_max_def])
   THEN1 (
     reverse IF_CASES_TAC \\ rfs[]
-    \\ MP_TAC (x64_iadd_thm |> Q.INST [`t`|->`~t`])
-    \\ fs[x64_header_XOR_1]
-    \\ match_mp_tac IMP_IMP \\ conj_tac THEN1 fs [x64_div_max_def]
+    \\ MP_TAC (mc_iadd_thm |> Q.INST [`t`|->`~t`])
+    \\ fs[mc_header_XOR_1]
+    \\ match_mp_tac IMP_IMP \\ conj_tac THEN1 fs [mc_div_max_def]
     \\ STRIP_TAC \\ FULL_SIMP_TAC std_ss [mwi_op_def,mwi_sub_def]
-    \\ fs[] \\ fs [x64_div_max_def])
+    \\ fs[] \\ fs [mc_div_max_def])
   THEN1 (
     IF_CASES_TAC \\ rfs[]
-    \\ MP_TAC x64_imul_thm \\ fs[]
-    \\ match_mp_tac IMP_IMP \\ conj_tac THEN1 fs [x64_div_max_def]
+    \\ MP_TAC mc_imul_thm \\ fs[]
+    \\ match_mp_tac IMP_IMP \\ conj_tac THEN1 fs [mc_div_max_def]
     \\ STRIP_TAC \\ FULL_SIMP_TAC std_ss [mwi_op_def]
     \\ FULL_SIMP_TAC (srw_ss()) []
-    \\ fs[] \\ fs [x64_div_max_def])
+    \\ fs[] \\ fs [mc_div_max_def])
   THEN1 (
     IF_CASES_TAC \\ rfs[]
-    \\ MP_TAC (x64_idiv_thm |> Q.INST [`r3`|->`0w`]) \\ fs[]
+    \\ MP_TAC (mc_idiv_thm |> Q.INST [`r3`|->`0w`]) \\ fs[]
     \\ STRIP_TAC \\ FULL_SIMP_TAC std_ss [mwi_op_def]
     \\ FULL_SIMP_TAC (srw_ss()) [mwi_divmod_alt_def])
   THEN1 (
     IF_CASES_TAC \\ rfs[]
-    \\ MP_TAC (x64_idiv_thm |> Q.INST [`r3`|->`1w`]) \\ fs[]
+    \\ MP_TAC (mc_idiv_thm |> Q.INST [`r3`|->`1w`]) \\ fs[]
     \\ STRIP_TAC \\ FULL_SIMP_TAC std_ss [mwi_op_def]
     \\ fs[mwi_divmod_alt_def] ));
 
